coq_ssprove/src/ChoiceEquality.v
@@ -1,12 +1,27 @@
+From Coq Require Import ZArith List.
 From Crypt Require Import choice_type Package.
 Import PackageNotation.
 From Crypt Require Import pkg_interpreter.
+From extructures Require Import ord fset fmap.
+Require Import Hacspec_Lib_Comparable.
 
-Class ChoiceEquality := {
-    T :> Type ;
-    ct :> choice_type ;
-    ChoiceEq : choice.Choice.sort (chElement ct) = T ;
+Require Import LocationUtility.
+Require Import Coq.Logic.FunctionalExtensionality.
+
+(* Set Printing Universes. *)
+
+Monomorphic Class ChoiceEquality := {
+    T : Type@{choice.Choice.type.u0} ;
+    ct : choice_type ;
+    ChoiceEq : @eq Type@{choice.Choice.type.u0} (choice.Choice.sort (chElement ct)) T ;
   }.
+(* Monomorphic Class ChoiceEquality@{a} := { *)
+(*     T : Type@{a} ; *)
+(*     ct : choice_type ; *)
+(*     ChoiceEq : @eq Type@{a} (choice.Choice.sort (chElement ct)) T ; *)
+(*   }. *)
+Print ChoiceEquality.
+
 
 Global Coercion T : ChoiceEquality >-> Sortclass.
 Global Coercion ct : ChoiceEquality >-> choice_type.
@@ -23,9 +38,71 @@ Proof (fun ce => rew_opp_r id (@ChoiceEq ce)).
 Theorem T_ct_id : forall {ce : ChoiceEquality} t, T_ct (ct_T t) = t.
 Proof (fun ce => rew_opp_l id (@ChoiceEq ce)).
 
-
 Global Coercion ct_T : choice.Choice.sort >-> T.
 Global Coercion T_ct : T >-> choice.Choice.sort.
+
+Lemma ChoiceEquality_ct_EqP : forall ce1 ce2, ce1 = ce2 <-> @ct ce1 = @ct ce2.
+Proof.
+  split ; intros.
+  - rewrite H.
+    reflexivity.
+  - destruct ce1 as [T1 ct1 CE1].
+    destruct ce2 as [T2 ct2 CE2].
+    cbn in *.
+    subst.
+    reflexivity.
+Qed.
+    
+Definition ChoiceEquality_leq (t1 t2 : ChoiceEquality) :=
+    choice_type_leq t1 t2.
+
+Lemma ChoiceEquality_leqP : Ord.axioms ChoiceEquality_leq.
+Proof.
+  unfold ChoiceEquality_leq.
+  destruct choice_type_leqP.
+  split.
+  - intros ?. apply H.
+  - intros ? ? ? ? ?. apply (H0 y x z) ; assumption.
+  - intros ? ? ?.
+    apply ChoiceEquality_ct_EqP.
+    apply H1. assumption.
+  - intros ? ?. apply H2.
+Qed.
+
+(* Locate OrdMixin. *)
+(* Definition ChoiceEquality_ordMixin := OrdMixin ChoiceEquality_leqP. *)
+(* Canonical ChoiceEquality_ordType : Ord.type. *)
+(* Proof. *)
+(*   pose ChoiceEquality. *)
+(*   Set Printing Universes. *)
+(*   pose ChoiceEquality_ordMixin. *)
+(*   pose (@Ord.pack T0). *)  
+(*   Constrait (extructures.ord. < Hacspec.ChoiceEquality.a). *)  
+(*   specialize (t T0). *)  
+(*   pose (OrdType ChoiceEquality ChoiceEquality_ordMixin). *)  
+(* (* Constraint ChoiceEquality.a < {extructures.ord.93}. *) *)  
+(*   Eval hnf in OrdType ChoiceEquality ChoiceEquality_ordMixin. *)
+
+Program Instance prod_ChoiceEquality (a b : ChoiceEquality) : ChoiceEquality :=
+  {| T := (@T a) * (@T b) ; ct := (@ct a) × (@ct b); |}.
+Next Obligation.
+  intros.
+  do 2 rewrite ChoiceEq.
+  reflexivity.
+Defined.
+
+Notation "A '× B" := (prod_ChoiceEquality A B) (at level 79, left associativity) : hacspec_scope.
+
+Open Scope hacspec_scope.
+
+Definition fst_CE {A B} (p : A '× B) : A := let '(f,s) := p in f.
+Definition snd_CE {A B} (p : A '× B) : B := let '(f,s) := p in s.  
+
+(* Notation "A '× B" := (prod A B) (at level 79, left associativity) : hacspec_scope. *)
+
+Instance nat_ChoiceEquality : ChoiceEquality := {| T := nat ; ct := 'nat ; ChoiceEq := ltac:(reflexivity) |}.
+Instance bool_ChoiceEquality : ChoiceEquality := {| T := bool ; ct := 'bool ; ChoiceEq := ltac:(reflexivity) |}.
+Instance unit_ChoiceEquality : ChoiceEquality := {| T := unit ; ct := 'unit ; ChoiceEq := ltac:(reflexivity) |}.
 
 Definition lift_to_code {ce : ChoiceEquality} {L I} (x : @T ce) : code L I (@ct ce) :=
   {code ret (T_ct x)}.
@@ -36,3 +113,704 @@ Proof.
   apply (ct_T s).
   contradiction.
 Defined.
+
+
+Definition pre_to_post (P : precond) {A} : postcond A A :=
+  fun '(a, h₀) '(b, h₁) => a = b /\ P (h₀ , h₁).  
+
+Definition true_precond : precond := fun _ => True.
+
+Class both L I (A : ChoiceEquality) :=
+  {
+    is_pure : A ;
+    is_state : code L I (@ct A) ;
+    code_eq_proof_statement :
+    ⊢ ⦃ true_precond ⦄
+          is_state ≈ lift_to_code (L := L) (I := I) (is_pure)
+      ⦃ pre_to_post true_precond ⦄
+  }.
+Coercion is_pure : both >-> T.
+Coercion is_state : both >-> code.
+
+Program Definition lift_to_both {ce : ChoiceEquality} {L I} (x : @T ce) : both L I ce :=
+  {| is_pure := x ; is_state := @lift_to_code ce L I x |}.
+Next Obligation. intros. apply r_ret. intros. split ; reflexivity. Qed.
+
+
+
+(* Ltac ssprove_valid_location := *)
+(*   try repeat (try (apply eqtype.predU1l ; reflexivity) ; try apply eqtype.predU1r). *)
+
+Ltac ssprove_valid_location :=
+  repeat
+    (try reflexivity ;
+     try (rewrite fset_cons ;
+          apply (ssrbool.introT (fsetU1P _ _ _)) ;
+          try (left ; reflexivity) ;
+          right)).
+
+
+Ltac ssprove_valid_program :=
+  try (apply prog_valid) ;
+  try (apply valid_scheme ; apply prog_valid).
+
+Ltac destruct_choice_type_prod :=
+  try match goal with
+  | H : choice.Choice.sort (chElement (loc_type ?p)) |- _ =>
+      unfold p in H ;
+      unfold loc_type in H ;
+      unfold projT1 in H
+  end ;
+  repeat match goal with
+  | H : @T (prod_ChoiceEquality _ _) |- _ =>
+      destruct H
+  end ;
+  repeat match goal with
+  | H : choice.Choice.sort
+         (chElement
+            (@ct
+               (prod_ChoiceEquality _ _))) |- _ =>
+      destruct H
+  end ;
+  repeat match goal with
+         | H : prod _ _ |- _ => destruct H
+         end.
+
+Ltac ssprove_valid_2 :=
+  (* destruct_choice_type_prod ; *)
+  ssprove_valid ;
+  ssprove_valid_program ;
+  ssprove_valid_location.
+
+Check ct.
+
+Theorem single_mem : forall m, 
+Datatypes.is_true
+    (@ssrbool.in_mem
+       (Ord.sort (@tag_ordType choice_type_ordType (fun _ : choice_type => nat_ordType)))
+       m
+       (@ssrbool.mem
+          (Ord.sort
+             (@tag_ordType choice_type_ordType (fun _ : choice_type => nat_ordType)))
+          (fset_predType
+             (@tag_ordType choice_type_ordType (fun _ : choice_type => nat_ordType)))
+          (@fset (@tag_ordType choice_type_ordType (fun _ : choice_type => nat_ordType))
+             (@cons (@sigT choice_type (fun _ : choice_type => nat)) m
+                    (@nil (@sigT choice_type (fun _ : choice_type => nat))))))).
+Proof.
+  intros.
+  rewrite <- (@fset1E (@tag_ordType choice_type_ordType (fun _ : choice_type => nat_ordType))).
+  rewrite (ssrbool.introT (fset1P _ _)) ; reflexivity.
+Qed.
+  
+(* Notation "ct( x , y , .. , z )" := (pair_ChoiceEquality .. (pair_ChoiceEquality x y) .. z) : hacspec_scope. *)
+
+
+
+(* Locate "=.?". *)
+
+(* Definition le_is_ord_leq2 : forall (s s0 : Location), *)
+(*     eqb (ssrfun.tagged s) (ssrfun.tagged s0) = false ->  *)
+(*     eqtype.eq_op (ssrfun.tag s) (ssrfun.tag s0) = false -> *)
+(*     s <.? s0 = (s <= s0)%ord. *)
+(* Proof. *)
+(*   intros s s0. *)
+(*   unfold "<.?" , location_comparable , eq_dec_lt_Comparable , location_ltb , "<?". *)
+(*   unfold eqtype.tagged_as, ssrfun.tagged , ssrfun.tag , ".π1" , ".π2". *)
+(*   intros e H. *)
+(*   destruct s , s0. *)
+
+(*   replace (((x; n) <= (x0; n0))%ord) with (x < x0)%ord. *)
+(*   2 : {     *)
+(*     cbn. *)
+(*     unfold tag_leq. *)
+(*     cbn. *)
+(*     cbn in H. *)
+(*     replace (choice_type_test x x0) with false by apply H. *)
+(*     cbn. *)
+(*     rewrite Bool.orb_false_r. *)
+(*     reflexivity. *)
+(*   }   *)
+
+  
+  
+(*   replace (eqtype.eq_op (ssrfun.tag (x; n)) (ssrfun.tag (x0; n0))) with false. *)
+  
+(*   rewrite le_is_ord_leq by apply e. *)
+
+  
+  
+(*   generalize dependent n. *)
+(*   induction n0 ; intros. *)
+(*   * destruct s ; easy. *)
+(*   * destruct s. reflexivity. *)
+(*     (* unfold Nat.leb ; fold Nat.leb. *) *)
+(*     cbn. *)
+(*     cbn in IHs0. *)
+(*     rewrite IHs0. *)
+(*     reflexivity. *)
+(*     assumption. *)
+(* Qed. *)
+
+
+Ltac ssprove_valid_location' :=
+  apply loc_compute ; repeat (try (left ; reflexivity) ; right) ; try reflexivity.
+
+(* Fixpoint uniqb {A} `{EqDec A} (s : list A) := *)
+(*   match s with *)
+(*   | cons x s' => andb (negb (Inb x s')) (uniqb s') *)
+(*   | _ => true *)
+(*   end. *)
+
+(* Theorem uniq_is_bool : forall (l : list (tag_ordType (I:=choice_type_ordType) (fun _ : choice_type => nat_ordType))), seq.uniq l = uniqb l. *)
+(* Proof. *)
+(*   cbn ; intros. *)
+(*   induction l. *)
+(*   - reflexivity. *)
+(*   - cbn. *)
+(*     f_equal. *)
+(*     + f_equal. *)
+(*       rewrite loc_compute_b. *)
+(*       reflexivity. *)
+(*     + exact IHl. *)
+(* Qed.         *)
+    
+(* Theorem simplify_fset : forall l, *)
+(*     is_true *)
+(*     (path.sorted leb l) -> *)
+(*     is_true (uniqb l) -> *)
+(*     (@FSet.fsval (@tag_ordType choice_type_ordType (fun _ : choice_type => nat_ordType)) *)
+(*        (@fset _ *)
+(*               l)) = (l). *)
+(*   intros l is_sorted  is_unique. *)
+(*   unfold fset ; rewrite ssreflect.locked_withE. *)
+(*   cbn. *)
+(*   rewrite <- uniq_is_bool in is_unique. *)
+(*   rewrite seq.undup_id by assumption. *)
+(*   rewrite path.sorted_sort. *)
+(*   - reflexivity. *)
+(*   - destruct (tag_leqP (I:=choice_type_ordType) (fun _ : choice_type => nat_ordType)) as [ _ trans _ _ ]. *)
+(*     apply trans. *)
+(*   - rewrite location_lebP. *)
+(*     assumption.   *)
+(* Qed. *)
+
+(* Theorem simplify_sorted_fset : forall l, *)
+(*     is_true (uniqb l) -> *)
+(*     (FSet.fsval (fset (path.sort (leb : Location -> Location -> bool) l))) *)
+(*     = (path.sort (leb : Location -> Location -> bool) l). *)
+(* Proof. *)
+(*   intros. *)
+(*   apply simplify_fset. *)
+(*   apply path.sort_sorted ; pose location_lebP ; cbn ; cbn in e ; rewrite <- e ; apply Ord.leq_total. *)
+(*   rewrite <- uniq_is_bool. *)
+(*   rewrite path.sort_uniq. *)
+(*   rewrite uniq_is_bool. *)
+(*   apply H. *)
+(* Qed. *)
+  
+Theorem tag_leq_simplify :
+  forall (a b : Location),
+    is_true (ssrfun.tag a <= ssrfun.tag b)%ord ->
+    is_true (ssrfun.tagged a <= ssrfun.tagged b)%ord ->
+    is_true (tag_leq (I:=choice_type_ordType) (T_:=fun _ : choice_type => nat_ordType) a b).
+Proof.
+  intros [] [].
+  
+  unfold tag_leq.
+  unfold eqtype.tagged_as, ssrfun.tagged , ssrfun.tag , projT1 , projT2.
+
+  intro.
+  rewrite Ord.leq_eqVlt in H.
+  rewrite is_true_split_or in H.
+  destruct H.
+  - apply Couplings.reflection_nonsense in H ; subst.
+    
+    rewrite Ord.ltxx.
+    rewrite Bool.orb_false_l.
+    rewrite eqtype.eq_refl.
+    rewrite Bool.andb_true_l.
+    
+    destruct eqtype.eqP.
+    + unfold eq_rect_r , eq_rect ; destruct eq_sym.
+      trivial.
+    + contradiction.
+  - rewrite H ; clear H.
+    reflexivity.    
+Qed.
+  
+Theorem tag_leq_inverse :
+  forall a b,
+    tag_leq (I:=choice_type_ordType) (T_:=fun _ : choice_type => nat_ordType) a b
+    =
+      (negb (tag_leq (I:=choice_type_ordType) (T_:=fun _ : choice_type => nat_ordType)
+                    b a) ||
+           eqtype.eq_op (ssrfun.tag a) (ssrfun.tag b) &&
+        eqtype.eq_op (ssrfun.tagged a) (ssrfun.tagged b))%bool.
+Proof.
+  intros [a b] [c d].
+  unfold tag_leq.
+  
+  rewrite Bool.negb_orb.
+  rewrite Bool.negb_andb.
+  rewrite Bool.andb_orb_distrib_r.
+
+  unfold eqtype.tagged_as.
+  unfold ssrfun.tagged , ssrfun.tag , projT1 , projT2.
+  rewrite <- Bool.orb_assoc.
+  
+  f_equal.
+  - rewrite <- Bool.negb_orb.    
+    rewrite <- Bool.orb_comm.
+    rewrite <- Ord.leq_eqVlt.
+    rewrite <- Ord.ltNge.
+    reflexivity.
+  - destruct (eqtype.eq_op a c) eqn:a_eq_c.
+    + apply Couplings.reflection_nonsense in a_eq_c.
+      subst.
+      do 2 rewrite Bool.andb_true_l.
+
+      destruct eqtype.eqP. 2: contradiction.
+      
+      unfold eq_rect_r , eq_rect.
+      destruct eq_sym.
+
+      rewrite Ord.leq_eqVlt.
+      rewrite Bool.orb_comm.
+
+      f_equal.
+      rewrite <- Ord.ltNge.
+      rewrite Ord.ltxx.
+      reflexivity.
+    + do 2 rewrite Bool.andb_false_l.
+      rewrite Bool.orb_false_r.
+      symmetry.
+
+      destruct eqtype.eqP.
+      { subst. rewrite eqtype.eq_refl in a_eq_c. discriminate a_eq_c. }
+
+      rewrite Ord.eq_leq by reflexivity.
+      rewrite Bool.andb_false_r.
+      reflexivity.
+Qed.
+
+(* rewrite list_incl_sort with (leb := location_ltb_simple) ;  *)
+Ltac incl_compute :=
+  now (apply list_incl_expand ; (now repeat (split ; [ repeat ((left ; reflexivity) || (right)) | ]))).
+  (* now (apply list_incl_compute ; cbn ; repeat rewrite ssrnat.eqnE ; repeat rewrite eqtype.eq_refl ; repeat rewrite choice_type_test_refl ; cbn ; reflexivity). *)
+
+(* Ltac valid_sorted_incl := *)
+(*   rewrite simplify_sorted_fset by reflexivity  *)
+(*   ; rewrite simplify_sorted_fset by reflexivity *)
+(*   ; apply list_incl_sort_order_ignorant_compute with (leb1 := location_ltb_simple) *)
+(*   ; cbn *)
+(*   ; incl_compute. *)
+
+Ltac valid_program :=
+  apply prog_valid
+  || (apply valid_scheme ; apply prog_valid)
+  || (eapply (valid_injectLocations_b) ; [ | apply prog_valid ] ; apply -> list_incl_remove_fset ; incl_compute).
+
+
+Definition heap_ignore_post fset {A} : postcond A A :=
+  pre_to_post (heap_ignore fset).
+
+Theorem heap_ignore_refl :
+  forall {fset} h, heap_ignore fset (h, h).
+Proof.
+  intros fset h ℓ ?.
+  reflexivity.
+Qed.
+
+Theorem heap_ignore_post_refl :
+  forall {fset A} (x : A * heap), heap_ignore_post fset x x.
+Proof.
+  intros fset A [].
+  split. reflexivity.
+  apply heap_ignore_refl.
+Qed.
+
+Lemma heap_ignore_weaken :
+  forall fset fset', is_true (fsubset fset fset') ->
+  forall x, heap_ignore fset x -> heap_ignore fset' x.
+Proof.
+  intros.
+  destruct x as [h h0].
+  pose (INV'_heap_ignore fset fset' fset0).
+  rewrite fsetU0 in i.
+  unfold INV' in i.
+  specialize (i H h h0).
+  destruct i as [? _].
+  intros l ?.
+  specialize (H1 H0 l H2 ltac:(easy)).
+  rewrite H1.
+  reflexivity.
+Qed.
+
+Lemma rpost_heap_ignore_weaken :
+  forall {A} fset fset', is_true (fsubset fset fset') ->
+  forall (x y : raw_code A),
+    ⊢ ⦃ (fun '(h0, h1) => heap_ignore fset (h0, h1)) ⦄
+        x ≈ y
+      ⦃ heap_ignore_post fset ⦄ ->
+    ⊢ ⦃ (fun '(h0, h1) => heap_ignore fset (h0, h1)) ⦄
+        x ≈ y
+        ⦃ heap_ignore_post fset' ⦄.
+Proof.
+  intros.
+  (* eapply rpre_weaken_rule. *)
+  eapply rpost_weaken_rule.
+  apply H0.
+
+  intros [] [] []. subst.
+  split. reflexivity.
+  apply (heap_ignore_weaken fset) ; assumption.
+Qed.
+
+
+Lemma rpre_heap_ignore_weaken :
+  forall {A} fset fset', is_true (fsubset fset fset') ->
+  forall (x y : raw_code A),
+    ⊢ ⦃ (fun '(h0, h1) => heap_ignore fset' (h0, h1)) ⦄
+        x ≈ y
+      ⦃ heap_ignore_post fset ⦄ ->
+    ⊢ ⦃ (fun '(h0, h1) => heap_ignore fset (h0, h1)) ⦄
+        x ≈ y
+        ⦃ heap_ignore_post fset ⦄.
+Proof.
+  intros.
+  eapply rpre_weaken_rule.
+  (* eapply rpost_weaken_rule. *)
+  apply H0.
+
+  intros. cbn.
+  apply (heap_ignore_weaken fset fset') ; assumption.
+Qed.
+
+(* Theorem bind_both {A B : ChoiceEquality} {fset' fset : {fset Location}}  `{b : @both fset A} *)
+(*         (k : choice.Choice.sort A -> raw_code B) : *)
+(*   List.incl fset fset' -> *)
+(*   forall fset_head fset_tail, *)
+(*     ⊢ ⦃ (fun '(h₀, h₁) => heap_ignore (fset_head :|: fset' :|: fset_tail) (h₀ , h₁)) ⦄ *)
+(*         (@bind A B is_state k) *)
+(*         ≈ *)
+(*         (@bind A B (lift_to_code (L := fset) (I := [interface]) is_pure) k) *)
+(*     ⦃ heap_ignore_post (fset_head :|: fset' :|: fset_tail) ⦄. *)
+(* Proof. *)
+(*   intros f_subset fset_head fset_tail. *)
+(*   apply list_incl_fsubset in f_subset. *)
+
+
+(*   assert (subset_eq : fset' = fset :|: (fset' :\: fset)). *)
+(*   { *)
+(*     apply (ssrbool.elimT fsetUidPr) in f_subset. *)
+(*     rewrite fsetUDr. *)
+(*     rewrite f_subset. *)
+(*     rewrite fsetDv. *)
+(*     rewrite fsetD0. *)
+(*     reflexivity. *)
+(*   } *)
+
+(*   rewrite subset_eq. *)
+(*   rewrite (fsetUC fset (fset' :\: fset)).     *)
+(*   rewrite fsetUA.   *)
+    
+(*   eapply (r_bind (is_state) ((lift_to_code (L := fset) (I := [interface]) is_pure)) k k). *)
+
+(*   apply code_eq_proof_statement. *)
+
+(*   (* intros. *) *)
+
+(*   exists fset_head, fset_tail. *)
+(*   split. *)
+(*   - intros. *)
+  
+  
+(*   apply rpre_hypothesis_rule. *)
+(*   intros ? ? []. *)
+(*   subst. *)
+
+(*   eapply rpost_weaken_rule. *)
+(*   - eapply rpre_weaken_rule. *)
+(*     + apply rreflexivity_rule. *)
+(*     + intros ? ? []. subst. *)
+(*       admit. *)
+(*   - intros [] [] ?. *)
+(*     inversion_clear H. *)
+(*     apply heap_ignore_post_refl. *)
+(* Admitted. *)
+
+(* Ltac bind_both_function := *)
+(*   match goal with *)
+(*   | [ |- context [ ⊢ ⦃ ?P ⦄ (@bind _ _ (_ (_ ?code_fun) ) ?k) ≈ _ ⦃ ?Q ⦄ ]] => *)
+(*       apply (@bind_both _ _ _ Q (code_eq_proof_statement code_fun) k) *)
+(*   end. *)
+
+Theorem bind_rewrite : forall A B x f, @bind A B (ret x) f = f x.
+Proof.
+  intros.
+  unfold bind.
+  reflexivity.
+Qed.
+(* Proof ltac:(unfold bind ; reflexivity). *)
+
+Ltac clear_bind :=
+  rewrite bind_rewrite
+  (* || *)
+  (* bind_both_function *).
+
+Theorem r_bind_eq : forall {B C : ChoiceEquality} (y : B) (g : choice.Choice.sort B  -> raw_code C), (temp ← ret y ;; g temp) = g y.
+Proof. reflexivity. Qed.
+
+Theorem r_bind_trans :
+  forall {B C : ChoiceEquality}
+    (f g : choice.Choice.sort B -> raw_code C) (x : raw_code B) (y : B),
+  forall (P P_mid : precond) (Q : postcond (choice.Choice.sort C) (choice.Choice.sort C)),
+  forall (H_x_is_y : ⊢ ⦃ P ⦄ x ≈ ret (T_ct y) ⦃ pre_to_post P_mid ⦄),
+    (forall a, ⊢ ⦃ P_mid ⦄ f a  ≈ g a ⦃ Q ⦄) ->
+    ⊢ ⦃ P ⦄ temp ← x ;; f temp ≈ g (T_ct y) ⦃ Q ⦄.
+Proof.
+  intros.
+  (* apply list_incl_fsubset in H_incl. *)
+
+  replace (g y) with (temp ← ret y ;; g temp) by reflexivity.
+
+  (* destruct H_P_Q as [fset_head [fset_tail [H_P [H_P_mid H_Q]]]]. *)
+  (* cbn in fset_head , fset_tail.  *)
+
+  (* set (P_mid := fun _ _ => _) in H_x_is_y. *)
+  
+  eapply r_bind with (mid := pre_to_post P_mid).
+  apply H_x_is_y.
+
+  intros.
+  eapply rpre_hypothesis_rule.
+  intros ? ? []. subst.
+  eapply rpre_weaken_rule.
+  2: { intros ? ? []. subst. apply H1. }
+  clear H1.
+
+  apply H.
+Qed.
+
+Lemma heap_ignore_remove_set_heap :
+  forall {fset} {s₀ s₁ : heap} {ℓ v},
+  is_true (ssrbool.in_mem ℓ (ssrbool.mem fset)) ->
+  heap_ignore (fset) (s₀, s₁) ->
+  heap_ignore (fset) (set_heap s₀ ℓ v, s₁).
+Proof.
+  intros.
+  unfold heap_ignore.
+  intros.
+  unfold heap_ignore in H0.  
+  specialize (H0 ℓ0 ltac:(assumption)).
+  rewrite <- H0.
+  rewrite <- get_heap_set_heap.
+  reflexivity.
+
+  destruct (@eqtype.eq_op
+          (@eqtype.tag_eqType choice_type_eqType
+                              (fun _ : choice_type => ssrnat.nat_eqType)) ℓ0 ℓ) eqn:ℓ_eq.
+  - apply (ssrbool.elimT eqtype.eqP) in ℓ_eq.
+    subst.
+    exfalso.
+    apply (ssrbool.elimT ssrbool.negP) in H.
+    + apply H.
+    + assumption.
+  - reflexivity.
+Qed.
+
+Lemma isolate_mem_section :
+  forall (fset : {fset Location}) ℓ  fset_head fset_tail,
+    is_true (ssrbool.in_mem ℓ (ssrbool.mem fset)) ->
+    is_true (ssrbool.in_mem ℓ (ssrbool.mem (fset_head :|: fset :|: fset_tail))).
+Proof.
+  intros.
+  apply loc_compute. apply in_split_fset_cat ; left ; apply in_split_fset_cat ; right.
+  apply loc_compute. apply H.
+Qed.  
+  
+Ltac solve_heap_ignore_remove_set_heap :=
+  apply (heap_ignore_remove_set_heap) ; [ apply isolate_mem_section ; apply loc_compute ; apply -> in_remove_fset ; cbn ; repeat (left ; reflexivity || right || reflexivity) | assumption ].
+
+Theorem r_bind_trans_both : forall {B C : ChoiceEquality} {L I} {f g : choice.Choice.sort B -> raw_code C} (b : both L I B),
+  forall (P : precond) (Q : postcond _ _),
+    (forall a, ⊢ ⦃ true_precond ⦄ f a  ≈ g a ⦃ Q ⦄) -> 
+    ⊢ ⦃ P ⦄ temp ← @is_state L I B b ;; f temp ≈ g (is_pure) ⦃ Q ⦄.
+Proof.
+  intros.
+  eapply r_bind_trans with (P_mid := true_precond).
+
+  eapply rpre_weaken_rule.    
+  apply code_eq_proof_statement.
+  reflexivity.
+
+  intros.
+  apply H.
+Qed.
+
+Ltac solve_post_from_pre :=
+  let H := fresh in
+  intros ? ? H
+  ; split
+  ; [reflexivity | ]
+  ; ( assumption
+      || (apply restore_set_lhs in H
+         ; [ assumption
+           | intros ? ?
+             ; solve_heap_ignore_remove_set_heap ] )).
+
+Corollary better_r_put_lhs : forall {A B : choice.Choice.type} (ℓ : Location)
+       (v : choice.Choice.sort (Value (projT1 ℓ))) (r₀ : raw_code A) 
+       (r₁ : raw_code B) (pre : precond)
+       (post : postcond (choice.Choice.sort A) (choice.Choice.sort B)),
+     ⊢ ⦃ set_lhs ℓ v pre ⦄ r₀ ≈ r₁ ⦃ post ⦄ ->
+     ⊢ ⦃ pre ⦄ #put ℓ := v ;; r₀ ≈ r₁ ⦃ post ⦄.
+Proof.
+  intros.
+  replace (pre) with (fun '(x, y) => pre (x, y)).
+  apply r_put_lhs.
+  apply H.
+  apply functional_extensionality.
+  intros [].
+  reflexivity.
+Qed.
+
+Corollary better_r_get_remind_lhs : forall {A B : choice.Choice.type} (ℓ : Location)
+       (v : choice.Choice.sort (Value (projT1 ℓ)))
+       (r₀ : choice.Choice.sort (Value (projT1 ℓ)) -> raw_code A) (r₁ : raw_code B)
+       (pre : precond) (post : postcond (choice.Choice.sort A) (choice.Choice.sort B)),
+     Remembers_lhs ℓ v pre ->
+     ⊢ ⦃ pre ⦄ r₀ v ≈ r₁ ⦃ post ⦄ ->
+     ⊢ ⦃ pre ⦄ x ← get ℓ ;; r₀ x ≈ r₁ ⦃ post ⦄.
+Proof.
+  intros.
+  replace (pre) with (fun '(x, y) => pre (x, y)) in *.
+  eapply r_get_remind_lhs.
+  apply H.
+  apply H0.
+  apply functional_extensionality.
+  intros [].
+  reflexivity.
+Qed.
+
+Lemma isolate_mem_sectiongetr_set_lhs : 
+  forall {A B} ℓ v pre post (a : _ -> raw_code A) (b : raw_code B),
+  ⊢ ⦃ set_lhs ℓ v pre ⦄
+     a v
+  ≈
+     b
+  ⦃ post ⦄ ->
+  ⊢ ⦃ set_lhs ℓ v pre ⦄
+     x ← get ℓ ;;
+     a x
+  ≈
+     b
+  ⦃ post ⦄.
+Proof.
+  clear.
+  intros.
+
+  eapply better_r_get_remind_lhs.
+  unfold Remembers_lhs.
+  intros ? ? [? []]. subst.
+  unfold rem_lhs.
+  rewrite get_set_heap_eq.
+  reflexivity.
+  apply H.
+Qed.
+
+Ltac progress_step_code :=    
+  match goal with
+  | [ |- context [ prog (@is_state ?L ?I _ ?x) : both _ _ _ ] ] =>
+      match goal with
+      | [ |- context [ ⊢ ⦃ _ ⦄ _ ≈ ?os ⦃ _ ⦄ ] ] =>
+          let Hx := fresh in
+          set (Hx := x)
+          ; try replace (@is_pure _ _ _ _) with (@is_pure _ _ _ Hx) by reflexivity
+          ; subst Hx
+          ; let H := fresh in
+            set (H := os)
+            ; pattern (@is_pure L I _ x) in H
+            ; set (Hx := x) in *
+            ; subst H
+            ; apply (@r_bind_trans_both) with (b := Hx)
+            ; intros
+      end
+  end
+  || match goal with
+    | [ |- context [ ⊢ ⦃ _ ⦄ (#put ?l := ?x ;; (getr ?l ?a)) ≈ _ ⦃ _ ⦄ ]] =>
+        apply (r_transL (#put l := x ;; a x )) ;
+        [ apply (r_put_get _ l x a) | ]
+    end
+  ||
+  match goal with
+  | [ |- context [ ⊢ ⦃ _ ⦄ (#put ?l := ?x ;; (putr ?l ?y ?a)) ≈ _ ⦃ _ ⦄ ]] =>
+      apply (r_transL (#put l := y ;; a )) ;
+      [ apply contract_put | ]
+  end
+  ||
+  match goal with
+  | [ |- context [ ⊢ ⦃ _ ⦄ (#put ?l := ?x ;; ?a) ≈ ?b ⦃ _ ⦄ ]] =>
+      apply (better_r_put_lhs l x a b (* (fun '(h0, h1) => heap_ignore fset (h0, h1)) *))
+  end
+  ||
+  rewrite bind_ret
+  ||
+  apply r_ret.
+
+Ltac step_code :=
+  repeat (clear_bind || progress_step_code) ; try (intros ; split ; reflexivity).
+
+(* Ltac heap_ignore_remove_ignore := *)
+(*   match goal with *)
+(*   | H : heap_ignore ?L ( ?a , ?b ) |- _ => *)
+(*       match goal with *)
+(*       | [ |- context[ heap_ignore L ( ?c , b ) ] ] => *)
+(*           intros ℓ H_mem *)
+(*           ; specialize (H ℓ H_mem) *)
+(*           ; match goal with *)
+(*             | [ |- context[ get_heap (set_heap ?x ?ℓ' ?v) ℓ = get_heap _ ℓ ] ] => *)
+(*                 destruct (@eqtype.eq_op (@eqtype.tag_eqType choice_type_eqType *)
+(*              (fun _ : choice_type => ssrnat.nat_eqType)) ℓ ℓ') eqn:ℓ_eq_ℓ' *)
+(*                 ; [ exfalso *)
+(*                     ; apply (ssrbool.elimT eqtype.eqP) in ℓ_eq_ℓ' ; subst *)
+(*                     ; apply (ssrbool.elimT ssrbool.negP) in H_mem *)
+(*                     ; apply H_mem *)
+(*                     ; clear H_mem *)
+(*                     ; apply loc_compute *)
+(*                     ; unfold eqtype.val *)
+(*                     ; rewrite simplify_sorted_fset *)
+(*                     ; repeat (reflexivity || (left ; reflexivity) || right) *)
+(*                   | rewrite <- (get_heap_set_heap a ℓ ℓ' v) ; *)
+(*                     [ assumption *)
+(*                     | rewrite ℓ_eq_ℓ' ; reflexivity  *)
+(*                     ] *)
+(*                 ]      *)
+(*             end *)
+(*       end *)
+(*   end . *)
+
+(* Ltac both_bind := *)
+(*   match goal with *)
+(*   | [ |- context[ (?x : both ?L ?T) ] ] =>   *)
+(*       match goal with *)
+(*       | [ |- context[ (bind ?f ?v) ] ] => *)
+(*           eapply (r_transR (bind (@is_state _ _ x) v) (bind (lift_to_code (@is_pure _ _ x)) v)) ; *)
+(*           [  *)
+(*           | eapply r_bind ; [ apply x | ] *)
+(*           ] *)
+(*       end *)
+(*   end. *)
+
+
+Ltac remove_T_ct :=
+  match goal with
+  | [ |- context[ T_ct ?x ] ] =>  
+      replace (T_ct x) with x by reflexivity
+  | H : _ |- context[ T_ct ?x ] =>  
+      replace (T_ct x) with x in H by reflexivity
+  end.
+
+
+
