coq_ssprove/src/Hacspec_Lib.v
@@ -14,8 +14,6 @@ From Coq Require Import ZArith List.
 Import List.ListNotations.
 (* Require Import IntTypes. *)
 
-Require Import ChoiceEquality.
-
 Require Import Lia.
 Require Import Coq.Logic.FunctionalExtensionality.
 
@@ -26,6 +24,8 @@ Declare Scope hacspec_scope.
 From CoqWord Require Import ssrZ word.
 From Jasmin Require Import word.
 
+Require Import ChoiceEquality.
+Require Import LocationUtility.
 Require Import Hacspec_Lib_Comparable.
 Require Import Hacspec_Lib_Pre.
 
@@ -34,39 +34,61 @@ Open Scope hacspec_scope.
 Open Scope nat_scope.
 Open Scope list_scope.
 
-Definition secret : forall {WS : wsize},  (@T (@int WS)) -> code fset.fset0 [interface] (@ct (@int WS)) := fun {WS} x => lift_to_code (secret x).
+Definition secret : forall {WS : wsize},  (@T (@int WS)) -> both fset.fset0 [interface] (@int WS) := fun {WS} x => lift_to_both (secret x).
+
+(* Definition secret {WS : wsize} (x : @int WS) : *)
+(*   both (fset.fset0) (@int WS) := lift_to_both (secret x). *)
 
 Section Uint.
-  
+  Definition uint8_declassify (n : int8) : both fset.fset0 [interface] int8 :=
+    lift_to_both (uint8_declassify n).
+  Definition int8_declassify (n : int8) : both fset.fset0 [interface] int8 :=
+    lift_to_both (int8_declassify n).
+  Definition uint16_declassify (n : int16) : both fset.fset0 [interface] int16 :=
+    lift_to_both (uint16_declassify n).
+  Definition int16_declassify (n : int16) : both fset.fset0 [interface] int16 :=
+    lift_to_both (int16_declassify n).
+  Definition uint32_declassify (n : int32) : both fset.fset0 [interface] int32 :=
+    lift_to_both (uint32_declassify n).
+  Definition int32_declassify (n : int32) : both fset.fset0 [interface] int32 :=
+    lift_to_both (int32_declassify n).
+  Definition uint64_declassify (n : int64) : both fset.fset0 [interface] int64 :=
+    lift_to_both (uint64_declassify n).
+  Definition int64_declassify (n : int64) : both fset.fset0 [interface] int64 :=
+    lift_to_both (int64_declassify n).
+  Definition uint128_declassify (n : int128) : both fset.fset0 [interface] int128 :=
+    lift_to_both (uint128_declassify n).
+  Definition int128_declassify (n : int128) : both fset.fset0 [interface] int128 :=
+    lift_to_both (int128_declassify n).
 
-Definition uint8_declassify (n : int8) : code fset.fset0 [interface] int8 := lift_to_code (uint8_declassify n).
-Definition int8_declassify (n : int8) : code fset.fset0 [interface] int8 := lift_to_code (int8_declassify n).
-Definition uint16_declassify (n : int16) : code fset.fset0 [interface] int16 := lift_to_code (uint16_declassify n).
-Definition int16_declassify (n : int16) : code fset.fset0 [interface] int16 := lift_to_code (int16_declassify n).
-Definition uint32_declassify (n : int32) : code fset.fset0 [interface] int32 := lift_to_code (uint32_declassify n).
-Definition int32_declassify (n : int32) : code fset.fset0 [interface] int32 := lift_to_code (int32_declassify n).
-Definition uint64_declassify (n : int64) : code fset.fset0 [interface] int64 := lift_to_code (uint64_declassify n).
-Definition int64_declassify (n : int64) : code fset.fset0 [interface] int64 := lift_to_code (int64_declassify n).
-Definition uint128_declassify (n : int128) : code fset.fset0 [interface] int128 := lift_to_code (uint128_declassify n).
-Definition int128_declassify (n : int128) : code fset.fset0 [interface] int128 := lift_to_code (int128_declassify n).
+  Definition uint8_classify (n : int8) : both fset.fset0 [interface] int8 :=
+    lift_to_both (uint8_classify n).
+  Definition int8_classify (n : int8) : both fset.fset0 [interface] int8 :=
+    lift_to_both (int8_classify n).
+  Definition uint16_classify (n : int16) : both fset.fset0 [interface] int16 :=
+    lift_to_both (uint16_classify n).
+  Definition int16_classify (n : int16) : both fset.fset0 [interface] int16 :=
+    lift_to_both (int16_classify n).
+  Definition uint32_classify (n : int32) : both fset.fset0 [interface] int32 :=
+    lift_to_both (uint32_classify n).
+  Definition int32_classify (n : int32) : both fset.fset0 [interface] int32 :=
+    lift_to_both (int32_classify n).
+  Definition uint64_classify (n : int64) : both fset.fset0 [interface] int64 :=
+    lift_to_both (uint64_classify n).
+  Definition int64_classify (n : int64) : both fset.fset0 [interface] int64 :=
+    lift_to_both (int64_classify n).
+  Definition uint128_classify (n : int128) : both fset.fset0 [interface] int128 :=
+    lift_to_both (uint128_classify n).
+  Definition int128_classify (n : int128) : both fset.fset0 [interface] int128 :=
+    lift_to_both (int128_classify n).
 
-Definition uint8_classify (n : int8) : code fset.fset0 [interface] int8 := lift_to_code (uint8_classify n).
-Definition int8_classify (n : int8) : code fset.fset0 [interface] int8 := lift_to_code (int8_classify n).
-Definition uint16_classify (n : int16) : code fset.fset0 [interface] int16 := lift_to_code (uint16_classify n).
-Definition int16_classify (n : int16) : code fset.fset0 [interface] int16 := lift_to_code (int16_classify n).
-Definition uint32_classify (n : int32) : code fset.fset0 [interface] int32 := lift_to_code (uint32_classify n).
-Definition int32_classify (n : int32) : code fset.fset0 [interface] int32 := lift_to_code (int32_classify n).
-Definition uint64_classify (n : int64) : code fset.fset0 [interface] int64 := lift_to_code (uint64_classify n).
-Definition int64_classify (n : int64) : code fset.fset0 [interface] int64 := lift_to_code (int64_classify n).
-Definition uint128_classify (n : int128) : code fset.fset0 [interface] int128 := lift_to_code (uint128_classify n).
-Definition int128_classify (n : int128) : code fset.fset0 [interface] int128 := lift_to_code (int128_classify n).
 
-
-(* CompCert integers' signedness is only interpreted through 'signed' and 'unsigned',
+  (* CompCert integers' signedness is only interpreted through 'signed' and 'unsigned',
    and not in the representation. Therefore, uints are just names for their respective ints.
-*)
+   *)
 
-Definition declassify_usize_from_uint8 (n : uint8) : code fset.fset0 [interface] uint_size := lift_to_code (declassify_usize_from_uint8 n).
+  Definition declassify_usize_from_uint8 (n : uint8) : both fset.fset0 [interface] uint_size :=
+    lift_to_both (declassify_usize_from_uint8 n).
 
 (**** Operations *)
 
@@ -98,32 +120,30 @@ Section Loops.
            {acc : ChoiceEquality}
            (fuel : nat)
            (i : @T uint_size)
-           (f: (@T uint_size) -> @T acc -> raw_code (@ct acc))
-           (cur : @T acc) {struct fuel} : raw_code (@ct acc) :=    
+           {L I}
+           (f: (@T uint_size) -> @T acc -> code L I (@ct acc))
+           (cur : @T acc) {struct fuel} : raw_code (@ct acc) :=
     match fuel with
-    | O => pkg_core_definition.ret (T_ct cur)
+    | O => ret cur
     | S n' =>
         cur' ← f i cur ;;
         foldi_ n' (i .+ one) f (ct_T cur')
     end.
 
   Lemma valid_foldi_ :
-    forall {acc : ChoiceEquality} L I n i (f : @T uint_size -> @T acc -> raw_code (@ct acc)) init,
-      (forall i v, ValidCode L I (f i v)) ->
+    forall {acc : ChoiceEquality} L I n i (f : @T uint_size -> @T acc -> code L I (@ct acc)) init,
       ValidCode L I (foldi_ n i f init).
   Proof.
-    induction n ; intros.
-    - cbn.
-      ssprove_valid.
-    - cbn.
-      ssprove_valid.
+    induction n ; intros ; cbn ; ssprove_valid.
+    apply f.
   Qed.
   
   Definition foldi_pre
              {acc: ChoiceEquality}
              (lo: @T uint_size)
              (hi: @T uint_size) (* {lo <= hi} *)
-             (f: (@T uint_size) -> @T acc -> raw_code (@ct acc)) (* {i < hi} *)
+             {I L}
+             (f: (@T uint_size) -> @T acc -> code I L (@ct acc)) (* {i < hi} *)
              (* {fset_init : _} *)
              (init: @T acc) : raw_code (@ct acc) :=
     match Z.sub (unsigned hi) (unsigned lo) with
@@ -160,7 +180,8 @@ Section Loops.
     forall {acc: ChoiceEquality}
       (fuel : nat)
       (i : @T uint_size)
-      (f : @T uint_size -> @T acc -> raw_code (@ct acc))
+      {L I}
+      (f : @T uint_size -> @T acc -> code L I (@ct acc))
       (cur : @T acc),
       (cur' ← f i cur ;; foldi_ fuel (i .+ one) f (ct_T cur')) = foldi_ (S fuel) i f cur.
   Proof. reflexivity. Qed.
@@ -182,7 +203,7 @@ Section Loops.
       (cur : @T acc),
       (cur' ← foldi_nat_ fuel i f (cur) ;; f (i + fuel) (ct_T cur')) = foldi_nat_ (S fuel) i f cur.
   Proof.
-    Set Printing Coercions.
+    (* Set Printing Coercions. *)
     induction fuel ; intros.
     - rewrite <- foldi__nat_move_S.
       unfold foldi_nat_.
@@ -275,8 +296,9 @@ Section Loops.
   Lemma foldi__move_S_fuel :
     forall {acc: ChoiceEquality}
       (fuel : nat)
-      (i : @T uint_size) 
-      (f : @T uint_size -> @T acc -> raw_code (@ct acc))
+      (i : @T uint_size)
+      {L I}
+      (f : @T uint_size -> @T acc -> code L I (@ct acc))
       (cur : @T acc),
       (0 <= Z.of_nat fuel <= @wmax_unsigned U32)%Z ->
       (cur' ← foldi_ fuel i f cur ;;
@@ -301,7 +323,7 @@ Section Loops.
       apply functional_extensionality.
       intros.
 
-      specialize (IHfuel (i .+ one) f (ct_T x)).
+      specialize (IHfuel (i .+ one) L I f (ct_T x)).
 
       replace ((repr (Z.of_nat (S fuel))) .+ i)
         with ((repr (Z.of_nat fuel)) .+ (i .+ one)).
@@ -359,7 +381,8 @@ Section Loops.
     forall {acc: ChoiceEquality}
       (lo: @T uint_size) (* {lo <= hi} *)
       (hi: @T uint_size) (* {lo <= hi} *)
-      (f: (@T uint_size) -> @T acc -> raw_code (@ct acc)) (* {i < hi} *)
+      {L I}
+      (f: (@T uint_size) -> @T acc -> code L I (@ct acc)) (* {i < hi} *)
       (init: @T acc),
       (unsigned lo <= unsigned hi)%Z ->
       foldi_pre lo hi f init = foldi_nat (Z.to_nat (unsigned lo)) (Z.to_nat (unsigned hi)) (fun x => f (repr (Z.of_nat x))) init.
@@ -408,7 +431,11 @@ Section Loops.
           lia.
         * apply functional_extensionality.
           intros.
-          f_equal.
+
+          enough ((@int_add U32 (@repr U32 (Z.of_nat (S n))) (@repr U32 (Z.of_nat lo_n))) = (@repr U32 (Z.of_nat (Init.Nat.add (S n) lo_n)))).
+          rewrite H0. reflexivity.
+          (* f_equal. *)
+          
           apply word_ext.
 
           replace (urepr (repr (Z.of_nat (S n)))) with (@unsigned U32 (repr (Z.of_nat (S n)))) by reflexivity.
@@ -423,11 +450,12 @@ Section Loops.
     forall {acc: ChoiceEquality}
       (lo: nat) (* {lo <= hi} *)
       (hi: nat) (* {lo <= hi} *)
-      (f: nat -> @T acc -> raw_code (@ct acc)) (* {i < hi} *)
+      {L I}
+      (f: nat -> @T acc -> code L I (@ct acc)) (* {i < hi} *)
       (init: @T acc),
       (lo <= hi) ->
       (Z.of_nat hi < @modulus U32)%Z ->
-      f = (fun x => f (from_uint_size (repr (Z.of_nat x)))) ->
+      (forall x, f x = f (from_uint_size (repr (Z.of_nat x)))) ->
       foldi_nat lo hi f init =
         foldi_pre (usize lo) (usize hi) (fun x => f (from_uint_size x)) init.
   Proof.
@@ -450,10 +478,11 @@ Section Loops.
     rewrite Zmod_small by (split ; [ lia | apply Z.le_lt_trans with (m := Z.of_nat hi) ; try apply inj_le ; assumption ]).
     rewrite Zmod_small by (split ; try easy ; lia).
     do 2 rewrite Nat2Z.id.
-
-    f_equal.
-    apply H1.      
     
+    f_equal.
+    apply functional_extensionality. intros.    
+    rewrite <- H1.
+    reflexivity.    
   Qed.
         
   (* folds can be computed by doing one iteration and incrementing the lower bound *)
@@ -558,7 +587,8 @@ Section Loops.
     forall {acc: ChoiceEquality}
       (lo: @T uint_size)
       (hi: @T uint_size) (* {lo <= hi} *)
-      (f: @T uint_size -> @T acc -> raw_code (@ct acc)) (* {i < hi} *)
+      {L I}
+      (f: @T uint_size -> @T acc -> code L I (@ct acc)) (* {i < hi} *)
       (init: @T acc),
     forall {guarantee: (unsigned lo <= unsigned mid <= unsigned hi)%Z},
       foldi_pre lo hi f init = (cur' ← foldi_pre lo mid f init ;; foldi_pre mid hi f (ct_T cur')).
@@ -585,7 +615,6 @@ Section Loops.
 
   Lemma valid_foldi_pre :
     forall {acc : ChoiceEquality} (lo hi : int_type) {L : {fset Location}} {I : Interface} (f : int_type -> T -> code L I ct),
-      (forall (i : int_type) (v : T), ValidCode L I (f i v)) ->
       forall init : T,
         ValidCode L I (foldi_pre lo hi f init).
   Proof.
@@ -594,7 +623,6 @@ Section Loops.
     destruct (unsigned hi - unsigned lo)%Z.
     - ssprove_valid.
     - apply valid_foldi_.
-      assumption.
     - ssprove_valid.
   Qed.
 
@@ -604,16 +632,12 @@ Section Loops.
              (hi: @T uint_size) (* {lo <= hi} *)
              {L}
              {I}
-             (f: (@T uint_size) -> @T acc -> code L I (@ct acc)) (* {i < hi} *)
-             (* `[is_subset : is_true (fsubset L1 L0)] *)
-             (* `[forall i v, ValidCode L1 I (f i v)] *)
+             (f: (@T uint_size) -> @T acc -> code L I (@ct acc))
              (init: @T acc)
     :
     code L I (@ct acc) :=
-    {| prog := (foldi_pre lo hi f init);
-      prog_valid := valid_foldi_pre _ _ _ _ _ |}.
-
-  Definition valid_foldi L I ce := fun lo hi d f => @prog_valid L I (@ct ce) (@foldi ce lo hi L I d f).
+    {| prog := foldi_pre lo hi f init;
+                     prog_valid := @valid_foldi_pre acc lo hi L I f init |}.
 
   (* Global Arguments foldi {_} _ _ {_} {_} {_} _ _ {_} {_}. *)
 
@@ -702,17 +726,19 @@ Section Loops.
     - apply H.
   Qed.
 
-  (* Lemma valid_foldi_subset : *)
-  (*   forall {acc : ChoiceEquality} L1 L2 I lo hi (f : @T uint_size -> @T acc -> code L1 [interface] (@ct acc)) init, *)
-  (*     fset.fsubset L1 L2 = true -> *)
-  (*     (forall i v, ValidCode L1 I (f i v)) -> *)
-  (*     ValidCode L2 I (foldi_pre lo hi f init). *)
-  (* Proof. *)
-  (*   intros. *)
-  (*   apply (@valid_injectLocations) with (L1 := L1). *)
-  (*   - apply H. *)
-  (*   - apply valid_foldi, H0. *)
-  (* Qed.   *)
+  Lemma valid_subset :
+    forall xs ys I {ct} c,
+      List.incl (xs) (ys) ->
+      ValidCode (fset xs) I c ->
+      @ValidCode (fset ys) I ct c.
+  Proof.
+    intros.
+    apply (@valid_injectLocations) with (L1 := fset xs).
+    - apply list_incl_fsubset.
+      apply -> list_incl_remove_fset.
+      apply H.      
+    - apply H0.
+  Qed.
 
 Theorem for_loop_unfold :
   forall c n,
@@ -726,275 +752,7 @@ Theorem for_loop_unfold :
     rewrite IHn.
     rewrite bind_assoc.
     reflexivity.
-Qed.
-
-Lemma for_loop_equality : forall fuel f,
-    for_loop f fuel  =
-    foldi_nat_ (S fuel) 0 (fun x _ => f x) tt.
-Proof.
-  intros.
-
-  replace f with (fun x => f (x + 0)) at 1.
-  2: {
-    apply functional_extensionality.
-    intros.
-    now rewrite Nat.add_0_r.
-  }
-
-  generalize dependent 0.
-  induction fuel ; intros n.
-  - unfold for_loop.
-    unfold foldi_nat_.
-    now rewrite bind_ret.
-  - rewrite for_loop_unfold.
-    rewrite <- foldi__nat_move_S.
-    f_equal.
-    apply functional_extensionality.
-    intros cur'.
-    destruct cur'.    
-    rewrite <- IHfuel.
-    f_equal.
-    apply functional_extensionality.
-    intros.
-    f_equal.
-    lia.
 Qed.    
-    
-Definition for_loop_range
-  (lo: nat)
-  (hi: nat)
-  (f : nat -> raw_code 'unit) : raw_code 'unit :=
-  for_loop (fun n => f (n + lo)) ((hi - lo) - 1).
-
-Definition for_loop_usize (lo hi : uint_size) {L I} (c : uint_size -> code L I 'unit) : raw_code 'unit :=
-  for_loop_range (from_uint_size lo) (from_uint_size hi) (fun n => prog (c (usize n))).
-
-Lemma for_loop_range_eq :
-  forall lo hi f,
-    for_loop_range lo hi f
-    =
-      (t ← f lo ;;
-       foldi_nat (S lo) hi (fun x _ => f x) t).
-Proof.
-  intros.
-  unfold for_loop_range.
-  rewrite for_loop_equality.
-  unfold foldi_nat.
-
-  replace (hi - S lo) with (hi - lo - 1) by lia.
-  
-  destruct (hi - lo - 1).
-  { cbn.
-    rewrite bind_ret.
-    reflexivity. }
-
-  set (f' := (fun (x : nat) (_ : T) => f x)).
-  replace (f lo) with (f' lo tt) by reflexivity.
-  pose foldi__nat_move_S. rewrite e. clear e.
-
-  replace lo with (0 + lo) at 1 by lia.
-  rewrite <- foldi__nat_move_to_function_add.
-  reflexivity.
-Qed.    
-
-
-Lemma foldi_nat_consume_ret_tt :
-  forall {acc : ChoiceEquality} lo hi f (v : acc),
-  (@foldi_nat acc lo hi (fun x a => f x tt ;; ret a) v)
-  =
-  (@foldi_nat unit_ChoiceEquality lo hi f tt ;; ret v).
-Proof.
-  intros.
-  unfold foldi_nat.
-  destruct (hi - lo).
-  - reflexivity.
-  - generalize dependent lo.
-    induction n ; intros.
-    + cbn.
-      rewrite bind_assoc.
-      rewrite bind_assoc.
-      unfold bind at 2.
-      rewrite T_ct_id.
-      reflexivity.
-    + rewrite <- foldi__nat_move_S.
-      rewrite bind_assoc.
-      rewrite <- foldi__nat_move_S.
-      rewrite bind_assoc.
-      f_equal.
-      apply functional_extensionality.
-      intros [].
-      unfold bind at 1.
-      rewrite ct_T_id.     
-      now rewrite IHn.
-Qed.            
-
-(* Lemma foldi_nat_tt_is_ignore : *)
-(*   forall {acc : ChoiceEquality} lo hi f (v : acc), *)
-(*     (@foldi_nat unit_ChoiceEquality lo hi f tt) *)
-(*   = *)
-(*   (@foldi_nat acc lo hi (fun x _ => f x tt) v). *)
-
-Lemma foldi_nat_consume_ret :
-  forall {acc A : ChoiceEquality} lo hi f (a : acc) (v : A),
-    (@foldi_nat (acc '× A) lo hi (fun x a => t ← f x (fst a) ;; @ret (acc '× A) (t, snd a)) (a , v))
-  =
-  (x ← @foldi_nat acc lo hi f a ;; @ret (acc '× A) (x, v)).
-Proof.
-Admitted.
-
-Lemma foldi_nat_is_loop :
-  forall {acc A : ChoiceEquality} lo hi f (k : A),
-  (for_loop_range lo hi (f k) ;; ret k)
-    =
-  (t ← f k lo ;; foldi_nat (S lo) hi (fun (x0 : nat) (a : T) => f k x0 ;; ret (T_ct a)) k).
-Proof.
-  intros.
-
-  rewrite for_loop_range_eq.
-  rewrite bind_assoc.
-  
-  f_equal.
-  apply functional_extensionality.
-  intros [].
-
-  rewrite <- (foldi_nat_consume_ret_tt (S lo) hi _ k).
-  reflexivity.  
-Qed.
-          
-(* Theorem for_loop_nat_equality (lo hi : nat) c : *)
-(*   ⊢ ⦃ fun '(s₀, s₁) => s₀ = s₁ ⦄ *)
-(*      for_loop_range lo hi c tt *)
-(*      ≈ *)
-(*      foldi_nat (lo) (hi) c (tt)    *)
-(*   ⦃ eq ⦄. *)
-(* Proof. *)
-(*   Set Printing Coercions. *)
-
-(*   unfold for_loop_range. *)
-      
-(*   unfold prog.   *)
-(*   unfold foldi_nat. *)
-  
-(*   destruct (hi - lo) eqn:hi_lo. *)
-(*   - (* apply Nat.sub_0_le in hi_lo. *) *)
-(*     (* apply Nat.leb_le in hi_lo. *) *)
-
-(*     (* unfold nat_comparable. *) *)
-(*     (* unfold leb. *) *)
-(*     (* rewrite hi_lo. *) *)
-
-(*     cbn. *)
-(*     rewrite bind_assoc. *)
-(*     unfold bind at 2. *)
-    
-    
-(*     unfold for_loop. *)
-(*     unfold foldi_nat. *)
-
-(*     apply rreflexivity_rule. *)
-(*   - replace (hi <=.? lo) with false by (rewrite leb_correct_conv by (replace hi with (S n + lo) ; lia) ; reflexivity). *)
-(*     clear hi_lo. *)
-
-(*     replace (S n - 1) with n by lia.  *)
-(*     rewrite <- foldi__nat_move_S. *)
-
-(*     generalize dependent lo. *)
-(*     (* generalize dependent P. *) *)
-(*     induction n ; intros. *)
-(*     + unfold for_loop. *)
-(*       rewrite Nat.add_0_l. *)
-(*       unfold foldi_nat_. *)
-(*       rewrite bind_ret. *)
-(*       unfold bind at 1. *)
-(*       rewrite bind_assoc. *)
-(*       unfold bind at 2. *)
-(*       rewrite ct_T_id. *)
-      
-(*       apply rreflexivity_rule. *)
-(*     + rewrite for_loop_unfold. *)
-(*       eapply r_bind. *)
-(*       apply rreflexivity_rule. *)
-(*       intros. *)
-(*       eapply rpre_weaken_rule.       *)
-(*       apply IHn. *)
-(*       intros. *)
-(*       inversion H ; subst. *)
-(*       reflexivity. *)
-(* Qed.     *)
-
-(* Theorem for_loop_nat_equality_better {acc : ChoiceEquality} (lo hi : nat) (c : nat -> acc -> raw_code acc) (v : acc) : *)
-(*   ⊢ ⦃ fun '(s₀, s₁) => s₀ = s₁ ⦄ *)
-(*       i ← ret v ;; *)
-(*   for_loop_range (fun x => (i ← c x (ct_T i) ;; @ret 'unit tt)) lo hi ;; *)
-(*   ret i *)
-(*      ≈ *)
-(*      foldi_nat (lo) (hi) c v    *)
-(*      ⦃ eq ⦄. *)
-(* Proof. *)
-(*   unfold bind at 1. *)
-(*   rewrite ct_T_id. *)
-
-(*   unfold for_loop_range. *)
-      
-(*   unfold prog.   *)
-(*   unfold foldi_nat. *)
-  
-(*   destruct (hi - lo) eqn:hi_lo. *)
-(*   - apply Nat.sub_0_le in hi_lo. *)
-(*     apply Nat.leb_le in hi_lo. *)
-(*     unfold nat_comparable. *)
-(*     unfold leb. *)
-(*     rewrite hi_lo. *)
-
-(*     apply r_ret. intros ; subst ; reflexivity. *)
-(*   - replace (hi <=.? lo) with false by (rewrite leb_correct_conv by (replace hi with (S n + lo) ; lia) ; reflexivity). *)
-(*     clear hi_lo. *)
-
-(*     replace (S n - 1) with n by lia.  *)
-(*     rewrite <- foldi__nat_move_S. *)
-
-(*     generalize dependent lo. *)
-(*     (* generalize dependent P. *) *)
-(*     induction n ; intros. *)
-(*     + unfold for_loop. *)
-(*       rewrite Nat.add_0_l. *)
-(*       unfold foldi_nat_. *)
-(*       rewrite bind_assoc. *)
-(*       unfold bind at 2. *)
-(*       (* unfold bind at 2. *) *)
-(*       replace (fun cur' : choice.Choice.sort (chElement ct) => ret (T_ct (ct_T cur'))) *)
-(*         with *)
-(*         (fun cur' : choice.Choice.sort (chElement ct) => ret cur'). *)
-(*       rewrite bind_ret. *)
-(*       apply rreflexivity_rule. *)
-(*     + rewrite for_loop_unfold. *)
-(*       eapply r_bind. *)
-(*       apply rreflexivity_rule. *)
-(*       intros. *)
-(*       eapply rpre_weaken_rule.       *)
-(*       apply IHn. *)
-(*       intros. *)
-(*       inversion H ; subst. *)
-(*       reflexivity. *)
-
-    
-(*   pose for_loop_nat_equality. *)
-  
-
-(* Theorem for_loop_equality (lo hi : uint_size) {H : (unsigned lo <= unsigned hi)%Z} {L I} (c : uint_size -> code L I 'unit) : *)
-(*   ⊢ ⦃ fun '(s₀, s₁) => s₀ = s₁ ⦄ *)
-(*      for_loop_usize lo hi c *)
-(*      ≈ *)
-(*      foldi (lo) (hi) (fun x a => c x) (tt)    *)
-(*   ⦃ eq ⦄. *)
-(* Proof. *)
-(*   unfold for_loop_usize. *)
-(*   unfold prog. *)
-(*   unfold foldi. *)
-(*   rewrite foldi_to_foldi_nat. *)
-(*   apply for_loop_nat_equality. *)
-(*   apply H. *)
-(* Qed. *)
 
 End Loops.
 
@@ -1004,38 +762,38 @@ Section Seqs.
 
   (**** Unsafe functions *)
 
-  Definition seq_new_ {A: ChoiceEquality} (init : A) (len: nat) : code fset.fset0 [interface] (seq A) :=
-    lift_to_code (seq_new_ init len).
+  Definition seq_new_ {A: ChoiceEquality} (init : A) (len: nat) : both fset.fset0 [interface] (seq A) :=
+    lift_to_both (seq_new_ init len).
 
-  Definition seq_new {A: ChoiceEquality} `{Default A} (len: nat) : code fset.fset0 [interface] (seq A) :=
-    lift_to_code (seq_new len).
+  Definition seq_new {A: ChoiceEquality} `{Default A} (len: nat) : both fset.fset0 [interface] (seq A) :=
+    lift_to_both (seq_new len).
 
-  Definition seq_len {A: ChoiceEquality} (s: @T (seq A)) : code fset.fset0 [interface] (@ct uint_size) := lift_to_code (seq_len s).
+  Definition seq_len {A: ChoiceEquality} (s: @T (seq A)) : both fset.fset0 [interface] (uint_size) := lift_to_both (seq_len s).
 
 (**** Array manipulation *)
 Definition array_new_ {A: ChoiceEquality} (init:@T A) (len: nat) :
-  code fset.fset0 [interface] (@ct (nseq A len)) :=
-  lift_to_code (array_new_ init len).
+  both fset.fset0 [interface] ((nseq A len)) :=
+  lift_to_both (array_new_ init len).
 
-Definition array_index {A: ChoiceEquality} `{Default (@T A)} {len : nat} (s: @T (nseq A len)) (i: nat) : code fset.fset0 [interface] (@ct A) :=
-  lift_to_code (array_index s i).
+Definition array_index {A: ChoiceEquality} `{Default (@T A)} {len : nat} (s: @T (nseq A len)) (i: nat) : both fset.fset0 [interface] (A) :=
+  lift_to_both (array_index s i).
 
-Definition array_upd {A: ChoiceEquality} {len : nat} (s: @T (nseq A len)) (i: nat) (new_v: @T A) : code fset.fset0 [interface] (@ct (nseq A len)) :=
-  lift_to_code (array_upd s i new_v).
+Definition array_upd {A: ChoiceEquality} {len : nat} (s: @T (nseq A len)) (i: nat) (new_v: @T A) : both fset.fset0 [interface] ((nseq A len)) :=
+  lift_to_both (array_upd s i new_v).
 
 (* substitutes a sequence (seq) into an array (nseq), given index interval  *)
 (* Axiom update_sub : forall {A len }, nseq A len -> nat -> nat -> seq A -> t A len. *)
-Definition update_sub {A : ChoiceEquality} {len slen} `{Default (@T A)} (v : @T (nseq A len)) (i : nat) (n : nat) (sub : @T (nseq A slen)) : code fset.fset0 [interface] (@ct (nseq A len)) :=
-  lift_to_code (update_sub v i n sub).
+Definition update_sub {A : ChoiceEquality} {len slen} `{Default (@T A)} (v : @T (nseq A len)) (i : nat) (n : nat) (sub : @T (nseq A slen)) : both fset.fset0 [interface] ((nseq A len)) :=
+  lift_to_both (update_sub v i n sub).
 
-Definition array_from_seq   {a: ChoiceEquality}
+Instance array_from_seq   {a: ChoiceEquality}
  `{Default (@T a)}
   (out_len:nat)
   (input: @T (seq a)) 
-  : code fset.fset0 [interface] (@ct (nseq a out_len)) :=
-  lift_to_code (array_from_seq out_len input : @T (nseq a out_len)).
+  : both fset.fset0 [interface] (nseq a out_len) :=
+  lift_to_both (array_from_seq out_len input). (*  : @T (nseq a out_len) *)
 
-Definition array_to_seq {A : ChoiceEquality} {n} (f : nseq_type A n) : code fset.fset0 [interface] (@ct (seq _)) := @lift_to_code (seq A) _ _ (array_to_seq f).
+Instance array_to_seq {A : ChoiceEquality} {n} (f : nseq_type A n) : both fset.fset0 [interface] (seq _) := @lift_to_both (seq A) _ _ (array_to_seq f).
 
 Definition array_from_slice
   {a: ChoiceEquality}
@@ -1043,9 +801,9 @@ Definition array_from_slice
   (default_value: (@T a))
   (out_len: nat)
   (input: @T (seq a))
-  (start: nat)
-  (slice_len: nat)  : code fset.fset0 [interface] (@ct (nseq a out_len)) :=
-  lift_to_code (array_from_slice default_value out_len input start slice_len).
+  (start: uint_size)
+  (slice_len: uint_size)  : both fset.fset0 [interface] ((nseq a out_len)) :=
+  lift_to_both (array_from_slice default_value out_len input (from_uint_size start) (from_uint_size slice_len)).
 
 Definition array_slice
   {a: ChoiceEquality}
@@ -1053,8 +811,8 @@ Definition array_slice
   (input: @T (seq a))
   (start: nat)
   (slice_len: nat)
-  : code fset.fset0 [interface] (@ct (nseq a slice_len)) :=
-  lift_to_code (array_slice input start slice_len).
+  : both fset.fset0 [interface] ((nseq a slice_len)) :=
+  lift_to_both (array_slice input start slice_len).
 
 Definition array_from_slice_range
   {a: ChoiceEquality}
@@ -1063,8 +821,8 @@ Definition array_from_slice_range
   (out_len: nat)
   (input: @T (seq a))
   (start_fin: (@T uint_size * @T uint_size))
-  : code fset.fset0 [interface] (@ct (nseq a out_len)) :=
-  lift_to_code (array_from_slice_range default_value out_len input start_fin).
+  : both fset.fset0 [interface] ((nseq a out_len)) :=
+  lift_to_both (array_from_slice_range default_value out_len input start_fin).
 
 Definition array_slice_range
   {a: ChoiceEquality}
@@ -1072,8 +830,8 @@ Definition array_slice_range
   {len : nat}
   (input: @T (nseq a len))
   (start_fin:(@T uint_size * @T uint_size))
-    : code fset.fset0 [interface] (@ct (seq a)) :=
-  lift_to_code (array_slice_range input start_fin).
+    : both fset.fset0 [interface] ((seq a)) :=
+  lift_to_both (array_slice_range input start_fin).
 
 Definition array_update
   {a: ChoiceEquality}
@@ -1082,8 +840,8 @@ Definition array_update
   (s: @T (nseq a len))
   (start : nat)
   (start_s: @T (seq a))
-  : code fset.fset0 [interface] (@ct (nseq a len)) :=
-    lift_to_code (array_update s start start_s).
+  : both fset.fset0 [interface] ((nseq a len)) :=
+    lift_to_both (array_update s start start_s).
 
 Definition array_update_start
   {a: ChoiceEquality}
@@ -1091,8 +849,8 @@ Definition array_update_start
   {len: nat}
   (s: @T (nseq a len))
   (start_s: @T (seq a))
-    : code fset.fset0 [interface] (@ct (nseq a len)) :=
-    lift_to_code (array_update_start s start_s).
+    : both fset.fset0 [interface] ((nseq a len)) :=
+    lift_to_both (array_update_start s start_s).
 
 Definition array_len_pre  {a: ChoiceEquality} {len: nat} (s: @T (nseq a len)) := len.
 (* May also come up as 'length' instead of 'len' *)
@@ -1107,16 +865,16 @@ Definition seq_slice
   (s: (@T (seq a)))
   (start: nat)
   (len: nat)
-    : code fset.fset0 [interface] (@ct (nseq a _)) :=
-  lift_to_code (seq_slice s start len).
+    : both fset.fset0 [interface] ((nseq a _)) :=
+  lift_to_both (seq_slice s start len).
 
 Definition seq_slice_range
   {a: ChoiceEquality}
  `{Default (@T (a))}
   (input: (@T (seq a)))
   (start_fin:((@T (uint_size)) * (@T (uint_size))))
-    : code fset.fset0 [interface] (@ct (nseq a _)) :=
-  lift_to_code (seq_slice_range input start_fin).
+    : both fset.fset0 [interface] ((nseq a _)) :=
+  lift_to_both (seq_slice_range input start_fin).
 
 (* updating a subsequence in a sequence *)
 Definition seq_update
@@ -1125,8 +883,8 @@ Definition seq_update
   (s: (@T (seq a)))
   (start: nat)
   (input: (@T (seq a)))
-  : code fset.fset0 [interface] (@ct (seq a)) :=
-  lift_to_code (seq_update s start input).
+  : both fset.fset0 [interface] ((seq a)) :=
+  lift_to_both (seq_update s start input).
 
 (* updating only a single value in a sequence*)
 Definition seq_upd
@@ -1135,16 +893,16 @@ Definition seq_upd
   (s: (@T (seq a)))
   (start: nat)
   (v: (@T (a)))
-  : code fset.fset0 [interface] (@ct (seq a)) :=
-  lift_to_code (seq_upd s start v).
+  : both fset.fset0 [interface] ((seq a)) :=
+  lift_to_both (seq_upd s start v).
 
 Definition seq_update_start
   {a: ChoiceEquality}
  `{Default (@T (a))}
   (s: (@T (seq a)))
   (start_s: (@T (seq a)))
-    : code fset.fset0 [interface] (@ct (seq a)) :=
-    lift_to_code (seq_update_start s start_s).
+    : both fset.fset0 [interface] ((seq a)) :=
+    lift_to_both (seq_update_start s start_s).
 
 Definition array_update_slice
   {a : ChoiceEquality}
@@ -1155,8 +913,8 @@ Definition array_update_slice
   (input: (@T (seq a)))
   (start_in: nat)
   (len: nat)
-  : code fset.fset0 [interface] (@ct (nseq a _)) :=
-  lift_to_code (array_update_slice (l := l) out start_out input start_in len).
+  : both fset.fset0 [interface] ((nseq a _)) :=
+  lift_to_both (array_update_slice (l := l) out start_out input start_in len).
   
 Definition seq_update_slice
   {a : ChoiceEquality}
@@ -1166,45 +924,46 @@ Definition seq_update_slice
   (input: (@T (seq a)))
   (start_in: nat)
   (len: nat)
-    : code fset.fset0 [interface] (@ct (nseq a _)) :=
-  lift_to_code (seq_update_slice out start_out input start_in len).
+    : both fset.fset0 [interface] ((nseq a _)) :=
+  lift_to_both (seq_update_slice out start_out input start_in len).
 
 Definition seq_concat
   {a : ChoiceEquality}
   (s1 :(@T (seq a)))
   (s2: (@T (seq a)))
-  : code fset.fset0 [interface] (@ct (seq a)) :=
-   lift_to_code (seq_concat s1 s2).
+  : both fset.fset0 [interface] ((seq a)) :=
+   lift_to_both (seq_concat s1 s2).
 
 Definition seq_push_pre
   {a : ChoiceEquality}
   (s1 :(@T (seq a)))
   (s2: (@T (a)))
-  : code fset.fset0 [interface] (@ct (seq a)) :=
-  lift_to_code (seq_push s1 s2).
+  : both fset.fset0 [interface] ((seq a)) :=
+  lift_to_both (seq_push s1 s2).
 
 Definition seq_from_slice_range
   {a: ChoiceEquality}
  `{Default (@T (a))}
   (input: (@T (seq a)))
   (start_fin: ((@T (uint_size)) * (@T (uint_size))))
-  : code fset.fset0 [interface] (@ct (seq a)) :=
-  lift_to_code (seq_from_slice_range input start_fin).
+  : both fset.fset0 [interface] ((seq a)) :=
+  lift_to_both (seq_from_slice_range input start_fin).
 
-Definition seq_from_seq {A} (l : @T (seq A)) : code fset.fset0 [interface] (_) := lift_to_code (seq_from_seq l).
+Definition seq_from_seq {A} (l : @T (seq A)) : both fset.fset0 [interface] (seq A) :=
+  lift_to_both (seq_from_seq l).
 
 (**** Chunking *)
 
-Definition seq_num_chunks {a: ChoiceEquality} (s: (@T (seq a))) (chunk_len: nat) : code fset.fset0 [interface] (@ct uint_size) :=
-  lift_to_code (usize (seq_num_chunks s chunk_len)).
+Definition seq_num_chunks {a: ChoiceEquality} (s: (@T (seq a))) (chunk_len: nat) : both fset.fset0 [interface] (uint_size) :=
+  lift_to_both (usize (seq_num_chunks s chunk_len)).
 
 Definition seq_chunk_len
   {a: ChoiceEquality}
   (s: (@T (seq a)))
   (chunk_len: nat)
   (chunk_num: nat)
-    : code fset.fset0 [interface] (@ct (nat_ChoiceEquality)) :=
-  lift_to_code (seq_chunk_len s chunk_len chunk_num).
+    : both fset.fset0 [interface] ((nat_ChoiceEquality)) :=
+  lift_to_both (seq_chunk_len s chunk_len chunk_num).
   
 (* Definition seq_chunk_same_len_same_chunk_len
   {a: Type}
@@ -1221,8 +980,8 @@ Definition seq_get_chunk
   (s: (@T (seq a)))
   (chunk_len: nat)
   (chunk_num: nat)
-  : code fset.fset0 [interface] ((@ct (uint_size '× seq a))) :=
-  lift_to_code (seq_get_chunk s chunk_len chunk_num).
+  : both fset.fset0 [interface] (((uint_size '× seq a))) :=
+  lift_to_both (seq_get_chunk s chunk_len chunk_num).
 
 Definition seq_set_chunk
   {a: ChoiceEquality}
@@ -1230,24 +989,24 @@ Definition seq_set_chunk
   (s: (@T (seq a)))
   (chunk_len: nat)
   (chunk_num: nat)
-  (chunk: (@T (seq a)) ) : code fset.fset0 [interface] (@ct (seq a)) :=
-  lift_to_code (seq_set_chunk s chunk_len chunk_num chunk).
+  (chunk: (@T (seq a)) ) : both fset.fset0 [interface] ((seq a)) :=
+  lift_to_both (seq_set_chunk s chunk_len chunk_num chunk).
 
 
-Definition seq_num_exact_chunks {a} (l : (@T (seq a))) (chunk_size : (@T (uint_size))) : (code fset.fset0 [interface] _) :=
-  lift_to_code (seq_num_exact_chunks l chunk_size).
+Definition seq_num_exact_chunks {a} (l : (@T (seq a))) (chunk_size : (@T (uint_size))) : (both fset.fset0 [interface] uint_size) :=
+  lift_to_both (seq_num_exact_chunks l chunk_size).
 
 
 (* Until #84 is fixed this returns an empty sequence if not enough *)
 Definition seq_get_exact_chunk {a : ChoiceEquality} `{Default (@T (a))} (l : (@T (seq a))) (chunk_size chunk_num: (@T (uint_size))) :
-  code fset.fset0 [interface] (@ct (seq a)) :=
-  lift_to_code (seq_get_exact_chunk l chunk_size chunk_num).
+  both fset.fset0 [interface] ((seq a)) :=
+  lift_to_both (seq_get_exact_chunk l chunk_size chunk_num).
 
 Definition seq_set_exact_chunk {a : ChoiceEquality} `{H : Default (@T (a))} :=
   @seq_set_chunk a H.
 
-Definition seq_get_remainder_chunk {a : ChoiceEquality} `{Default (@T (a))} (l : @T (seq a)) (chunk_size : @T (uint_size)) : code fset.fset0 [interface] (@ct (seq a)) :=
-  lift_to_code (seq_get_remainder_chunk l chunk_size).
+Definition seq_get_remainder_chunk {a : ChoiceEquality} `{Default (@T (a))} (l : @T (seq a)) (chunk_size : @T (uint_size)) : both fset.fset0 [interface] ((seq a)) :=
+  lift_to_both (seq_get_remainder_chunk l chunk_size).
 
 (**** Numeric operations *)
 
@@ -1258,8 +1017,8 @@ Definition array_join_map
   {len: nat}
   (op: (@T (a)) -> (@T (a)) -> (@T (a)))
   (s1: (@T (nseq a len)))
-  (s2 : (@T (nseq a len))) : code fset.fset0 [interface] (@ct (nseq a len)) :=
-  lift_to_code (array_join_map op s1 s2).
+  (s2 : (@T (nseq a len))) : both fset.fset0 [interface] ((nseq a len)) :=
+  lift_to_both (array_join_map op s1 s2).
   
 (* Infix "array_xor" := (array_join_map xor) (at level 33) : hacspec_scope. *)
 (* Infix "array_add" := (array_join_map add) (at level 33) : hacspec_scope. *)
@@ -1296,94 +1055,28 @@ Infix "array_neq" := (fun s1 s2 => negb (array_eq_ eq s1 s2)) (at level 33) : ha
 
 
 (**** Integers to arrays *)
-Axiom uint32_to_le_bytes : @T int32 -> code fset.fset0 [interface] (@ct (nseq int8 4)).
-(* Definition uint32_to_le_bytes (x: uint32) : nseq uint8 4 :=
-  LBSeq.uint_to_bytes_le x. *)
-
-Axiom uint32_to_be_bytes : @T int32 -> code fset.fset0 [interface] (@ct (nseq int8 4)).
-(* Definition uint32_to_be_bytes (x: uint32) : nseq uint8 4 :=
-  LBSeq.uint_to_bytes_be x *)
-
-Axiom uint32_from_le_bytes : @T (nseq int8 4) -> code fset.fset0 [interface] (@ct (int32)).
-(* Definition uint32_from_le_bytes (s: nseq uint8 4) : uint32 :=
-  LBSeq.uint_from_bytes_le s *)
-
-Axiom uint32_from_be_bytes : @T (nseq int8 4) -> code fset.fset0 [interface] (@ct (int32)).
-(* Definition uint32_from_be_bytes (s: nseq uint8 4) : uint32 :=
-  LBSeq.uint_from_bytes_be s *)
-
-Axiom uint64_to_le_bytes : @T int64 -> code fset.fset0 [interface] (@ct (nseq int8 8)).
-(* Definition uint64_to_le_bytes (x: uint64) : nseq uint8 8 :=
-  LBSeq.uint_to_bytes_le x *)
-
-Axiom uint64_to_be_bytes : @T int64 -> code fset.fset0 [interface] (@ct (nseq int8 8)).
-(* Definition uint64_to_be_bytes (x: uint64) : nseq uint8 8 :=
-  LBSeq.uint_to_bytes_be x *)
-
-Axiom uint64_from_le_bytes : @T (nseq int8 8) -> code fset.fset0 [interface] (@ct (int64)).
-(* Definition uint64_from_le_bytes (s: nseq uint8 8) : uint64 :=
-  LBSeq.uint_from_bytes_le s *)
-
-Axiom uint64_from_be_bytes : @T (nseq int8 8) -> code fset.fset0 [interface] (@ct (int64)).
-(* Definition uint64_from_be_bytes (s: nseq uint8 8) : uint64 :=
-  LBSeq.uint_from_bytes_be s *)
-
-Axiom uint128_to_le_bytes : @T int128 -> code fset.fset0 [interface] (@ct (nseq int8 16)).
-(* Definition uint128_to_le_bytes (x: uint128) : nseq uint8 16 :=
-  LBSeq.uint_to_bytes_le x *)
-
-Axiom uint128_to_be_bytes : @T int128 -> code fset.fset0 [interface] (@ct (nseq int8 16)).
-(* Definition uint128_to_be_bytes (x: uint128) : nseq uint8 16 :=
-  LBSeq.uint_to_bytes_be x *)
-
-Definition uint128_from_le_bytes (n : @T (nseq int8 16)) : code fset.fset0 [interface] (@ct (int128)) := lift_to_code (uint128_from_le_bytes n).
-(* Definition uint128_from_le_bytes (input: nseq uint8 16) : uint128 :=
-  LBSeq.uint_from_bytes_le input *)
-
-Axiom uint128_from_be_bytes : @T (nseq int8 16) -> code fset.fset0 [interface] (@ct (int128)).
-(* Definition uint128_from_be_bytes (s: nseq uint8 16) : uint128 :=
-  LBSeq.uint_from_bytes_be s *)
-
-Axiom u32_to_le_bytes : @T int32 -> code fset.fset0 [interface] (@ct (nseq int8 4)).
-(* Definition u32_to_le_bytes (x: pub_uint32) : nseq pub_uint8 4 :=
-  LBSeq.uint_to_bytes_le x *)
-
-Axiom u32_to_be_bytes : @T int32 -> code fset.fset0 [interface] (@ct (nseq int8 4)).
-(* Definition u32_to_be_bytes (x: pub_uint32) : nseq pub_uint8 4 :=
-  LBSeq.uint_to_bytes_be x *)
-
-Axiom u32_from_le_bytes : @T (nseq int8 4) -> code fset.fset0 [interface] (@ct (int32)).
-(* Definition u32_from_le_bytes (s: nseq pub_uint8 4) : pub_uint32 :=
-  LBSeq.uint_from_bytes_le s *)
-
-Axiom u32_from_be_bytes : @T (nseq int8 4) -> code fset.fset0 [interface] (@ct (int32)).
-(* Definition u32_from_be_bytes (s: nseq pub_uint8 4) : pub_uint32 :=
-  LBSeq.uint_from_bytes_be s *)
-
-Axiom u64_to_le_bytes : @T int64 -> code fset.fset0 [interface] (@ct (nseq int8 8)).
-(* Definition u64_to_le_bytes (x: int64) : nseq int8 8 :=
-  LBSeq.uint_to_bytes_le x *)
-
-Axiom u64_from_le_bytes : @T (nseq int8 8) -> code fset.fset0 [interface] (@ct (int64)).
-(* Definition u64_from_le_bytes (s: nseq int8 8) : int64 :=
-  LBSeq.uint_from_bytes_le s *)
-
-Axiom u128_to_le_bytes : @T int128 -> code fset.fset0 [interface] (@ct (nseq int8 16)).
-(* Definition u128_to_le_bytes (x: int128) : nseq int8 16 :=
-  LBSeq.uint_to_bytes_le x *)
-
-Axiom u128_to_be_bytes : @T int128 -> code fset.fset0 [interface] (@ct (nseq int8 16)).
-(* Definition u128_to_be_bytes (x: int128) : nseq int8 16 :=
-  LBSeq.uint_to_bytes_be x *)
-
-Axiom u128_from_le_bytes : @T (nseq int8 16) -> code fset.fset0 [interface] (@ct (int128)).
-(* Definition u128_from_le_bytes (input: nseq int8 16) : int128 :=
-  LBSeq.uint_from_bytes_le input *)
-
-Axiom u128_from_be_bytes : @T (nseq int8 16) -> code fset.fset0 [interface] (@ct (int128)).
-(* Definition u128_from_be_bytes (s: nseq int8 16) : pub_uint128 :=
-  LBSeq.uint_from_bytes_be s *)
-
+Definition uint32_to_le_bytes (n : @T int32) : both fset.fset0 [interface] ((nseq int8 4)) := lift_to_both (uint32_to_le_bytes n).
+Definition uint32_to_be_bytes (n : @T int32) : both fset.fset0 [interface] ((nseq int8 4)) := lift_to_both (uint32_to_be_bytes n).
+Definition uint32_from_le_bytes (n : @T (nseq int8 4)) : both fset.fset0 [interface] ((int32)) := lift_to_both (uint32_from_le_bytes n).
+Definition uint32_from_be_bytes (n : @T (nseq int8 4)) : both fset.fset0 [interface] ((int32)) := lift_to_both (uint32_from_be_bytes n).
+Definition uint64_to_le_bytes (n : @T int64) : both fset.fset0 [interface] ((nseq int8 8)) := lift_to_both (uint64_to_le_bytes n).
+Definition uint64_to_be_bytes (n : @T int64) : both fset.fset0 [interface] ((nseq int8 8)) := lift_to_both (uint64_to_be_bytes n).
+Definition uint64_from_le_bytes (n : @T (nseq int8 8)) : both fset.fset0 [interface] ((int64)) := lift_to_both (uint64_from_le_bytes n).
+Definition uint64_from_be_bytes (n : @T (nseq int8 8)) : both fset.fset0 [interface] ((int64)) := lift_to_both (uint64_from_be_bytes n).
+Definition uint128_to_le_bytes (n : @T int128) : both fset.fset0 [interface] ((nseq int8 16)) := lift_to_both (uint128_to_le_bytes n).
+Definition uint128_to_be_bytes (n : @T int128) : both fset.fset0 [interface] ((nseq int8 16)) := lift_to_both (uint128_to_be_bytes n).
+Definition uint128_from_le_bytes (n : @T (nseq int8 16)) : both fset.fset0 [interface] (int128) := lift_to_both (uint128_from_le_bytes n).
+Definition uint128_from_be_bytes (n : @T (nseq int8 16)) : both fset.fset0 [interface] ((int128)) := lift_to_both (uint128_from_be_bytes n).
+Definition u32_to_le_bytes (n : @T int32) : both fset.fset0 [interface] ((nseq int8 4)) := lift_to_both (u32_to_le_bytes n).
+Definition u32_to_be_bytes (n : @T int32) : both fset.fset0 [interface] ((nseq int8 4)) := lift_to_both (u32_to_be_bytes n).
+Definition u32_from_le_bytes (n : @T (nseq int8 4)) : both fset.fset0 [interface] ((int32)) := lift_to_both (u32_from_le_bytes n).
+Definition u32_from_be_bytes (n : @T (nseq int8 4)) : both fset.fset0 [interface] ((int32)) := lift_to_both (u32_from_be_bytes n).
+Definition u64_to_le_bytes (n : @T int64) : both fset.fset0 [interface] ((nseq int8 8)) := lift_to_both (u64_to_le_bytes n).
+Definition u64_from_le_bytes (n : @T (nseq int8 8)) : both fset.fset0 [interface] ((int64)) := lift_to_both (u64_from_le_bytes n).
+Definition u128_to_le_bytes (n : @T int128) : both fset.fset0 [interface] ((nseq int8 16)) := lift_to_both (u128_to_le_bytes n).
+Definition u128_to_be_bytes (n : @T int128) : both fset.fset0 [interface] ((nseq int8 16)) := lift_to_both (u128_to_be_bytes n).
+Definition u128_from_le_bytes (n : @T (nseq int8 16)) : both fset.fset0 [interface] ((int128)) := lift_to_both (u128_from_le_bytes n).
+Definition u128_from_be_bytes (n : @T (nseq int8 16)) : both fset.fset0 [interface] ((int128)) := lift_to_both (u128_from_be_bytes n).
 
 (*** Nats *)
 
@@ -1400,9 +1093,9 @@ Definition nat_mod_zero_pre {p} : nat_mod p := zmodp.Zp0.
 Definition nat_mod_one_pre {p} : nat_mod p := zmodp.Zp1.
 Definition nat_mod_two_pre {p} : nat_mod p := zmodp.inZp 2.
 
-Definition nat_mod_zero {p} : code fset.fset0 [interface] (@ct (nat_mod p)) := lift_to_code (nat_mod_zero_pre).
-Definition nat_mod_one {p} : code fset.fset0 [interface] (@ct (nat_mod p)) := lift_to_code (nat_mod_one_pre).
-Definition nat_mod_two {p} : code fset.fset0 [interface] (@ct (nat_mod p)) := lift_to_code (nat_mod_two_pre).
+Definition nat_mod_zero {p} : both fset.fset0 [interface] ((nat_mod p)) := lift_to_both (nat_mod_zero_pre).
+Definition nat_mod_one {p} : both fset.fset0 [interface] ((nat_mod p)) := lift_to_both (nat_mod_one_pre).
+Definition nat_mod_two {p} : both fset.fset0 [interface] ((nat_mod p)) := lift_to_both (nat_mod_two_pre).
 
 
 (* convenience coercions from nat_mod to Z and N *)
@@ -1444,15 +1137,15 @@ Close Scope nat_scope.
 (* Definition nat_mod_from_secret_literal_pre {m : Z} (x:int128) : nat_mod m := *)
 (*   @zmodp.inZp (Init.Nat.pred (Z.to_nat m)) (Z.to_nat (unsigned x)). *)
 
-Definition nat_mod_from_secret_literal {m : Z} (x:int128) : code fset.fset0 [interface] (@ct (nat_mod m)) :=
- lift_to_code (@nat_mod_from_secret_literal m x).  
+Definition nat_mod_from_secret_literal {m : Z} (x:int128) : both fset.fset0 [interface] (nat_mod m) :=
+ lift_to_both (@nat_mod_from_secret_literal m x).  
 
-Definition nat_mod_from_literal (m : Z) (x:int128) : code fset.fset0 [interface] (@ct (nat_mod m)) := nat_mod_from_secret_literal x.
+Definition nat_mod_from_literal (m : Z) (x:int128) : both fset.fset0 [interface] ((nat_mod m)) := nat_mod_from_secret_literal x.
 
-Axiom nat_mod_to_byte_seq_le : forall {n : Z}, nat_mod n -> code fset.fset0 [interface] (seq int8).
-Axiom nat_mod_to_byte_seq_be : forall {n : Z}, nat_mod n -> code fset.fset0 [interface] (seq int8).
-Axiom nat_mod_to_public_byte_seq_le : forall (n : Z), nat_mod n -> code fset.fset0 [interface] (seq int8).
-Axiom nat_mod_to_public_byte_seq_be : forall (n : Z), nat_mod n -> code fset.fset0 [interface] (seq int8).
+Definition nat_mod_to_byte_seq_le {n : Z} (m : nat_mod n) : both fset.fset0 [interface] (seq int8) := lift_to_both (nat_mod_to_byte_seq_le m).
+Definition nat_mod_to_byte_seq_be {n : Z} (m : nat_mod n) : both fset.fset0 [interface] (seq int8) := lift_to_both (nat_mod_to_byte_seq_be m).
+Definition nat_mod_to_public_byte_seq_le (n : Z) (m : nat_mod n) : both fset.fset0 [interface] (seq int8) := lift_to_both (nat_mod_to_public_byte_seq_le n m).
+Definition nat_mod_to_public_byte_seq_be (n : Z) (m : nat_mod n) : both fset.fset0 [interface] (seq int8) := lift_to_both (nat_mod_to_public_byte_seq_be n m).
 
 Definition nat_mod_bit_pre {n : Z} (a : nat_mod n) (i : uint_size) : bool :=
   Z.testbit (Z.of_nat (nat_of_ord a)) (from_uint_size i).
@@ -1473,19 +1166,19 @@ Definition nat_mod_to_public_byte_seq_le (n: pos)  (len: uint_size) (x: nat_mod_
   Definition n' := n % (pow2 (8 * len)) in
   Lib.ByteSequence.nat_to_bytes_be len n' *)
 
-Axiom array_declassify_eq : forall  {A l}, nseq A l -> nseq A l -> code fset.fset0 [interface] 'bool.
-Axiom array_to_le_uint32s : forall {A l}, nseq A l -> code fset.fset0 [interface] (nseq uint32 l).
-Axiom array_to_be_uint32s : forall {l}, nseq uint8 l -> code fset.fset0 [interface] (nseq uint32 (l/4)).
-Axiom array_to_le_bytes : forall {A l}, nseq A l -> code fset.fset0 [interface] (seq uint8).
-Axiom array_to_be_bytes : forall {A l}, nseq A l -> code fset.fset0 [interface] (seq uint8).
-Axiom nat_mod_from_byte_seq_le : forall  {A n}, seq A -> code fset.fset0 [interface] (nat_mod n).
-Axiom most_significant_bit : forall {m}, nat_mod m -> uint_size -> code fset.fset0 [interface] (uint_size).
+Axiom array_declassify_eq : forall  {A l}, nseq A l -> nseq A l -> both fset.fset0 [interface] bool_ChoiceEquality.
+Axiom array_to_le_uint32s : forall {A l}, nseq A l -> both fset.fset0 [interface] (nseq uint32 l).
+Axiom array_to_be_uint32s : forall {l}, nseq uint8 l -> both fset.fset0 [interface] (nseq uint32 (l/4)).
+Axiom array_to_le_bytes : forall {A l}, nseq A l -> both fset.fset0 [interface] (seq uint8).
+Axiom array_to_be_bytes : forall {A l}, nseq A l -> both fset.fset0 [interface] (seq uint8).
+Axiom nat_mod_from_byte_seq_le : forall  {A n}, seq A -> both fset.fset0 [interface] (nat_mod n).
+Axiom most_significant_bit : forall {m}, nat_mod m -> uint_size -> both fset.fset0 [interface] (uint_size).
 
 
 (* We assume 2^x < m *)
 
-Definition nat_mod_pow2 (m : Z) (x : N) : code fset.fset0 [interface] (@ct (nat_mod m)) :=
-  lift_to_code (nat_mod_pow2 m x).
+Definition nat_mod_pow2 (m : Z) (x : N) : both fset.fset0 [interface] ((nat_mod m)) :=
+  lift_to_both (nat_mod_pow2 m x).
 
 End Todosection.
 
@@ -1608,69 +1301,6 @@ Definition usize_from_uint128 (n : int128) : uint_size := repr (unsigned n).
 
 
 (* Comparisons, boolean equality, and notation *)
-
-Instance eq_dec_lt_Comparable {A : Type} `{EqDec A} (ltb : A -> A -> bool) : Comparable A := {
-    ltb := ltb;
-    leb a b := if eqb a b then true else ltb a b ;
-    gtb a b := ltb b a;
-    geb a b := if eqb a b then true else ltb b a;
-  }.
-
-Instance eq_dec_le_Comparable {A : Type} `{EqDec A} (leb : A -> A -> bool) : Comparable A := {
-    ltb a b := if eqb a b then false else leb a b;
-    leb := leb ;
-    gtb a b := if eqb a b then false else leb b a;
-    geb a b := leb b a;
-  }.
-
-Theorem eqb_refl : forall {A} {H : EqDec A} (x : A), @eqb A H x x = true.
-Proof.
-  intros.
-  now rewrite eqb_leibniz.
-Qed.
-
-
-Global Program Instance nat_eqdec : EqDec nat := {
-  eqb := Nat.eqb;
-  eqb_leibniz := Nat.eqb_eq ;
-}.
-
-Global Instance nat_comparable : Comparable nat := {
-  ltb := Nat.ltb;
-  leb := Nat.leb;
-  gtb a b := Nat.ltb b a;
-  geb a b := Nat.leb b a;
-}.
-
-Global Instance N_eqdec : EqDec N := {
-  eqb := N.eqb;
-    eqb_leibniz := N.eqb_eq ;
-}.
-
-Global Instance N_comparable : Comparable N := {
-  ltb := N.ltb;
-  leb := N.leb;
-  gtb a b := N.ltb b a;
-  geb a b := N.leb b a;
-}.
-
-Global Instance Z_eqdec : EqDec Z := {
-  eqb := Z.eqb;
-  eqb_leibniz := Z.eqb_eq ;
-}.
-
-Global Instance Z_comparable : Comparable Z := {
-  ltb := Z.ltb;
-  leb := Z.leb;
-  gtb a b := Z.ltb b a;
-  geb a b := Z.leb b a;
-}.
-
-Lemma int_eqb_eq : forall {WS : wsize} (a b : @int WS),
-    eqtype.eq_op a b = true <-> a = b.
-Proof.
-  symmetry ; exact (ssrbool.rwP (@eqtype.eqP _ a b)).
-Qed.
 
 Global Instance int_eqdec `{WS : wsize}: EqDec (@int WS) := {
   eqb := eqtype.eq_op ;
@@ -1829,396 +1459,58 @@ Definition nat_be_range (k : nat) (z : Z) (n : nat) : Z :=
 
 End TodoSection2.
 
-(*** Location *)
-
-Section Location.
-    Fixpoint Inb {A : Type} `{EqDec A} (a:A) (l:list A) : bool :=
-    match l with
-    | nil => false
-    | cons b m => (eqb b a) || Inb a m
-    end.
-  
-
-  Definition location_eqb (ℓ ℓ' : Location) :=
-    (eqb (ssrfun.tagged ℓ) (ssrfun.tagged ℓ')).
-  (* (@eqtype.eq_op *)
-  (* (@eqtype.tag_eqType choice_type_eqType *)
-  (*                     (fun _ : choice_type => ssrnat.nat_eqType)) ℓ ℓ'). *)
-
-  Axiom location_is_types : (forall l1 l2 : Location ,
-                                is_true (eqb (ssrfun.tagged l1) (ssrfun.tagged l2)) ->
-                                is_true (eqtype.eq_op (ssrfun.tag l1) (ssrfun.tag l2))).
-
-  Definition location_eqbP : forall (l1 l2 : Location),
-      @eqb nat _ (ssrfun.tagged l1) (ssrfun.tagged l2)
-      = (@eqtype.eq_op
-           (@eqtype.tag_eqType choice_type_eqType
-                               (fun _ : choice_type => ssrnat.nat_eqType)) l1 l2).
-  Proof.
-    intros.
-    symmetry.
-    pose (location_is_types l1 l2).
-    destruct l1, l2.
-    unfold location_eqb.
-    cbn.
-    unfold eqtype.tag_eq.
-    unfold eqtype.tagged_as, ssrfun.tagged , ssrfun.tag , ".π1" , ".π2" in *.
-
-    destruct ((n =? n0)%nat) eqn:b.
-    - rewrite i by assumption.        
-      destruct eqtype.eqP.
-      + cbn.
-        unfold eq_rect_r , eq_rect ; destruct eq_sym.      
-        assumption.
-      + rewrite eqtype.eq_refl.
-        reflexivity.
-    - destruct eqtype.eqP.
-      + cbn.
-        unfold eq_rect_r , eq_rect ; destruct eq_sym.
-        assumption.
-      + rewrite eqtype.eq_refl.
-        reflexivity.
-  Qed.
-
-  Lemma location_eqb_sound : forall ℓ ℓ' : Location, is_true (location_eqb ℓ ℓ') <-> ℓ = ℓ'.
-  Proof.
-    intros.
-    unfold is_true.
-    replace (location_eqb ℓ ℓ' = true) with (true = location_eqb ℓ ℓ') by
-      (rewrite boolp.propeqE ; split ; symmetry ; assumption).
-    unfold location_eqb. rewrite location_eqbP.
-    split.
-    - symmetry ; apply lookup_hpv_r_obligation_1 ; assumption.
-    - intros ; subst. cbn. symmetry. rewrite eqtype.tag_eqE. apply eqtype.eq_refl.
-  Qed.
-
-  Global Program Instance location_eqdec: EqDec (Location) := {
-      eqb := location_eqb;
-      eqb_leibniz := location_eqb_sound;
-    }.
-
-  Definition location_ltb : Location -> Location -> bool :=
-    (fun l1 l2 : Location =>
-       let (_, n1) := l1 in
-       let (_, n2) := l2 in
-       ltb n1 n2).
-
-  Global Instance location_comparable : Comparable (Location) :=
-    eq_dec_lt_Comparable location_ltb.
-
-  Definition le_is_ord_leq : forall s s0 : nat_ordType,
-      eqtype.eq_op s s0 = false -> ltb s s0 = (s <= s0)%ord.
-  Proof.
-    intros s s0.
-    unfold ltb , nat_comparable , Nat.ltb.
-    intros e.
-    
-    generalize dependent s.
-    induction s0 ; intros.
-    * destruct s ; easy.
-    * destruct s. reflexivity.
-      (* unfold Nat.leb ; fold Nat.leb. *)
-      cbn.
-      cbn in IHs0.
-      rewrite IHs0.
-      reflexivity.
-      assumption.
-  Qed.
-Theorem is_true_split_or : forall a b, is_true (a || b) = (is_true a \/ is_true b).
-Proof.
-  intros.
-  rewrite boolp.propeqE.
-  symmetry.
-  apply (ssrbool.rwP ssrbool.orP).
-Qed.  
-Theorem is_true_split_and : forall a b, is_true (a && b) = (is_true a /\ is_true b).
-Proof.
-  intros.
-  rewrite boolp.propeqE.
-  symmetry.
-  apply (ssrbool.rwP ssrbool.andP).
-Qed.  
-  
-  
-
-    
-Theorem LocsSubset : (forall {A} (L1 L2 : list A) (a : A),
-     List.incl L1 L2 ->
-     List.In a L1 ->
-     List.In a L2).
-  intros.
-  induction L1 as [ | a0 L ] ; cbn in *.
-  - contradiction.
-  - destruct (List.incl_cons_inv H).
-    destruct H0.
-    + subst.
-      assumption.
-    + apply IHL ; assumption.
-Qed.
-Theorem in_bool_iff : forall {A : Type} `{EqDec A} (a:A) (l:list A), is_true (Inb a l) <-> List.In a l.
-  induction l ; cbn.
-  - rewrite boolp.falseE.
-    reflexivity.
-  - cbn.
-    rewrite is_true_split_or.    
-    apply ZifyClasses.or_morph.
-    apply eqb_leibniz.
-    apply IHl.
-Qed.
-
-Theorem loc_compute_b :
-  (forall l : (@sigT choice_type (fun _ : choice_type => nat)),
-    forall n : list (@sigT choice_type (fun _ : choice_type => nat)),
-      Inb l n = ssrbool.in_mem l (@ssrbool.mem _
-          (seq.seq_predType
-             (Ord.eqType
-                (@tag_ordType choice_type_ordType (fun _ : choice_type => nat_ordType))))
-          n)).
-  intros.
-  cbn.
-  unfold ssrbool.in_mem.
-  unfold ssrbool.pred_of_mem.
-  unfold ssrbool.mem ; cbn.
-  
-  induction n.
-  - cbn.
-    reflexivity.
-  - cbn.
-    unfold "||".
-    rewrite eqtype.tag_eqE ; rewrite eqtype.eq_sym ; rewrite <- eqtype.tag_eqE.
-    rewrite IHn.
-    rewrite location_eqbP.
-    reflexivity.
-Qed.
-
-Theorem loc_compute : (forall l : (@sigT choice_type (fun _ : choice_type => nat)), forall n : list (@sigT choice_type (fun _ : choice_type => nat)), List.In l n <-> is_true (ssrbool.in_mem l (@ssrbool.mem _
-          (seq.seq_predType
-             (Ord.eqType
-                (@tag_ordType choice_type_ordType (fun _ : choice_type => nat_ordType))))
-          n))).
-  intros.
-  rewrite <- loc_compute_b.
-  symmetry.
-  apply in_bool_iff.
-Qed.
-
-Lemma valid_injectLocations_b :
-  forall (import : Interface) (A : choice.Choice.type)
-    (L1 L2 : {fset tag_ordType (I:=choice_type_ordType) (fun _ : choice_type => nat_ordType)})
-    (v : raw_code A),
-    List.incl L1 L2 -> ValidCode L1 import v -> ValidCode L2 import v.
-Proof.
-    intros A L1 L2 v h incl p.
-    induction p.
-    all:
-      try solve [ constructor ; eauto ].
-    all: apply loc_compute in H 
-    ; constructor ; [ | eauto ]
-    ; apply loc_compute
-    ; eapply LocsSubset
-    ; eauto.
-Qed.
-
-Theorem in_bool_eq : forall {A : Type} `{EqDec A} (a:A) (l:list A), is_true (Inb a l) = List.In a l.
-  intros.
-  rewrite boolp.propeqE. apply in_bool_iff.
-Qed.
-
-  Definition incl_sort_compute A `{EqDec A} (l1 l2 : list A) : bool.
-  Proof.
-    induction l1.
-    - exact true.
-    - exact (andb (Inb a l2) (IHl1)).      
-  Defined.
-
-  Definition incl_fset_sort_compute (l1 l2 : {fset Location}) : bool.
-  Proof.
-    destruct l1 as [l1].
-    induction l1.
-    - exact true.
-    - assert (is_true (path.sorted Ord.lt l1)).
-      {
-        pose (path.drop_sorted).
-        specialize i0 with (n := 1) (s := a :: l1).
-        rewrite seq.drop1 in i0.
-        unfold seq.behead in i0.
-        apply i0.
-        apply i.
-      }
-      exact (andb (Inb a l2) (IHl1 H)).      
-  Defined.
-
-  Theorem in_remove_fset : forall a (l : list Location), List.In a l <-> List.In a (fset l).
-  Proof.
-    intros.
-    do 2 rewrite loc_compute.
-    unfold fset ; rewrite ssreflect.locked_withE.
-    cbn.
-    rewrite (@path.mem_sort (Ord.eqType
-                (@tag_ordType choice_type_ordType (fun _ : choice_type => nat_ordType))) (tag_leq (I:=choice_type_ordType) (T_:=fun _ : choice_type => nat_ordType)) (@seq.undup
-                (Ord.eqType
-                   (@tag_ordType choice_type_ordType (fun _ : choice_type => nat_ordType)))
-                l)).
-    
-    generalize dependent a.
-    induction l ; intros.
-    + easy.
-    + cbn.
-
-      rewrite (@seq.in_cons (Ord.eqType
-                               (@tag_ordType choice_type_ordType (fun _ : choice_type => nat_ordType))) a l).
-      rewrite is_true_split_or.
-
-      match goal with
-      | [ |- context[match ?x with | true => _ | false => _ end] ] =>
-          destruct x eqn:so
-      end.
-      * rewrite <- IHl.
-        split.
-        -- intros [].
-           ++ apply Couplings.reflection_nonsense in H.
-              subst.
-              apply so.
-           ++ apply H.
-        -- intros.
-           right.
-           apply H.
-      * split.
-        -- intros [].
-           ++ apply Couplings.reflection_nonsense in H.
-              subst.
-              apply seq.mem_head.
-           ++ apply seq.mem_drop with (n0 := 1%nat).
-              cbn.
-              rewrite seq.drop0.
-              apply IHl.
-              apply H.
-        -- intros.
-           destruct (eqtype.eq_op) eqn:so2.
-           ++ left.
-              reflexivity.
-           ++ right.
-              unfold ssrbool.in_mem in H.
-              unfold ssrbool.pred_of_mem in H.
-              unfold ssrbool.mem in H.
-              cbn in H.
-              cbn in so2.
-              rewrite so2 in H.
-              cbn in H.
-
-              apply IHl.
-              apply H.
-  Qed.
-
-  Theorem list_incl_remove_fset {A} `{EqDec A} : forall (l1 l2 : list Location), List.incl l1 l2 <-> List.incl (fset l1) (fset l2).
-  Proof.
-    pose in_bool_eq.
-    pose loc_compute_b.
-    
-    intros. (* [l1] [l2]. *)
-    pose (@incl_sort_compute A H).
-
-    cbn in *.
-    
-    induction l1.
-    - rewrite <- fset0E. easy.
-    - cbn.
-      unfold incl.
-      cbn.
-      split.
-      + intros.
-        rewrite <- in_remove_fset.
-        rewrite <- in_remove_fset in H1.
-        apply H0.
-        apply H1.
-      + intros.        
-        rewrite -> in_remove_fset.
-        apply H0.
-        rewrite <- in_remove_fset.
-        apply H1.
-Qed.        
-
-  Theorem list_incl_compute {A} `{EqDec A} : forall (l1 l2 : list Location), List.incl l1 l2 <-> is_true (incl_sort_compute _ l1 l2).
-    induction l1.
-    - split ; intros.
-      reflexivity.
-      apply incl_nil_l.
-    - intros.
-      
-      assert (forall A (a : A) l1 l2, List.incl (a :: l1) l2 <-> (List.In a l2 /\ List.incl l1 l2)).
-      {
-        split.
-        - pose List.incl_cons_inv.
-          apply List.incl_cons_inv.
-        - intros [].
-          apply List.incl_cons ; assumption.          
-      }
-
-      rewrite H0.
-
-      cbn.
-      rewrite is_true_split_and.
-      rewrite in_bool_eq.
-
-      apply and_iff_compat_l.
-      apply IHl1.
-  Qed.        
-
-  (* Theorem forall l1 l2, incl_sort_compute <-> list_incl_compute  *)
-
-End Location.
 
 (*** Monad / Bind *)
 
-Definition result_unwrap {a b} (x : result a b) : code fset.fset0 [interface] (a) :=
-  lift_to_code (result_unwrap x).
-Definition result_unwrap_safe {a b} (x : result a b) `{match x with @Ok_type _ _ _ => True | @Err_type _ _ _ => False end} : code fset.fset0 [interface] (a) :=
-  lift_to_code (result_unwrap_safe x (H := H)).
+Definition result_unwrap {a b} (x : result a b) : both fset.fset0 [interface] (a) :=
+  lift_to_both (result_unwrap x).
+Definition result_unwrap_safe {a b} (x : result a b) `{match x with @Ok_type _ _ _ => True | @Err_type _ _ _ => False end} : both fset.fset0 [interface] (a) :=
+  lift_to_both (result_unwrap_safe x (H := H)).
 
 Module ChoiceEqualityMonad.
   
-  Class bind_through_code {M} (mon : ChoiceEqualityMonad.CEMonad M) :=
-    {
-      bind_code : forall {A B} {L1 L2 : list Location} `{is_true (incl_sort_compute _ L1 L2)} {I} (y : code (fset L1) I (M A)) (f : A -> code (fset L2) I (M B)) , code (fset L2) I (M B)
-    }.
+  (* Class bind_through_code {M} (mon : ChoiceEqualityMonad.CEMonad M) := *)
+  (*   { *)
+  (*     bind_code : forall {A B} {L1 L2 : list Location} `{is_true (incl_sort_compute _ L1 L2)} {I} (y : code (fset L1) I (M A)) (f : A -> code (fset L2) I (M B)) , code (fset L2) I (M B) *)
+  (*   }. *)
 
 
-  Global Program Instance result_bind_code {C} : bind_through_code (@ChoiceEqualityMonad.result_monad C) :=
-    {|
-      bind_code A B L1 L2 H I y f :=
-      {code
-         z ← y ;;
-         match ct_T z with
-         | @Ok_type _ _ a => f a
-         | @Err_type _ _ b => (@mkprog (fset L2) I _ (pkg_core_definition.ret (Err b)) (valid_ret (fset L2) I (Err b)))
-         end}
-    |}.
-  Next Obligation.
-    intros.
-    apply valid_bind.
-    - apply (@valid_injectLocations_b I _ (fset L1) (fset L2) y).
-      apply (list_incl_remove_fset L1 L2).      
-      apply (proj2 (list_incl_compute L1 L2) H).
-      apply y.
-    - intros.
-      destruct ct_T.
-      + apply (f t).
-      + apply valid_ret.      
-  Qed.
+  (* Global Program Instance result_bind_code {C} : bind_through_code (@ChoiceEqualityMonad.result_monad C) := *)
+  (*   {| *)
+  (*     bind_code A B L1 L2 H I y f := *)
+  (*     {code *)
+  (*        z ← y ;; *)
+  (*        match ct_T z with *)
+  (*        | @Ok_type _ _ a => f a *)
+  (*        | @Err_type _ _ b => (@mkprog (fset L2) I _ (pkg_core_definition.ret (Err b)) (valid_ret (fset L2) I (Err b))) *)
+  (*        end} *)
+  (*   |}. *)
+  (* Next Obligation. *)
+  (*   intros. *)
+  (*   apply valid_bind. *)
+  (*   - apply (@valid_injectLocations_b I _ (fset L1) (fset L2) y). *)
+  (*     apply (list_incl_remove_fset L1 L2).       *)
+  (*     apply (proj2 (list_incl_compute L1 L2) H). *)
+  (*     apply y. *)
+  (*   - intros. *)
+  (*     destruct ct_T. *)
+  (*     + apply (f t). *)
+  (*     + apply valid_ret.       *)
+  (* Qed. *)
   
 End ChoiceEqualityMonad.  
 
 (*** Notation *)
 
-Program Definition if_bind_code {A : ChoiceEquality} `{mnd : ChoiceEqualityMonad.CEMonad} `{@ChoiceEqualityMonad.bind_through_code _ mnd} (b : bool_ChoiceEquality) {Lx Ly L2 : list Location}  `{it1 : is_true (incl_sort_compute _ Lx L2)} `{it2 : is_true (incl_sort_compute _ Ly L2)} {I} (x : code (fset Lx) I (M A)) (y : code (fset Ly) I (M A)) (f : A -> code (fset L2) I (@ct (M A))) : code (fset L2) I (@ct (M A)) :=
-  if b
-  then ChoiceEqualityMonad.bind_code (L1 := Lx) (is_true0 := it1) x f
-  else ChoiceEqualityMonad.bind_code (L1 := Ly) (is_true0 := it2) y f.
+(* Program Definition if_bind_code {A : ChoiceEquality} `{mnd : ChoiceEqualityMonad.CEMonad} `{@ChoiceEqualityMonad.bind_through_code _ mnd} (b : bool_ChoiceEquality) {Lx Ly L2 : list Location}  `{it1 : is_true (incl_sort_compute _ Lx L2)} `{it2 : is_true (incl_sort_compute _ Ly L2)} {I} (x : code (fset Lx) I (M A)) (y : code (fset Ly) I (M A)) (f : A -> code (fset L2) I (@ct (M A))) : code (fset L2) I (@ct (M A)) := *)
+(*   if b *)
+(*   then ChoiceEqualityMonad.bind_code (L1 := Lx) (is_true0 := it1) x f *)
+(*   else ChoiceEqualityMonad.bind_code (L1 := Ly) (is_true0 := it2) y f. *)
 
-Definition foldi_bind_code {A : ChoiceEquality} `{mnd : ChoiceEqualityMonad.CEMonad} `{@ChoiceEqualityMonad.bind_through_code _ mnd} (a : uint_size) (b : uint_size) {L1 L2 : list Location} `{is_true (incl_sort_compute _ L1 L2)} {I}  (init : M A) (f : uint_size -> A -> code (fset L2) I (@ct (M A))) : code (fset L2) I (@ct (M A)) :=
-  foldi a b (fun x y => ChoiceEqualityMonad.bind_code (L1 := L1) (is_true0 := is_true0) (lift_to_code y) (f x)) init.
+(* Definition foldi_bind_code {A : ChoiceEquality} `{mnd : ChoiceEqualityMonad.CEMonad} `{@ChoiceEqualityMonad.bind_through_code _ mnd} (a : uint_size) (b : uint_size) {L1 L2 : list Location} `{is_true (incl_sort_compute _ L1 L2)} {I}  (init : M A) (f : uint_size -> A -> code (fset L2) I (@ct (M A))) : code (fset L2) I (@ct (M A)) := *)
+(*   foldi a b (fun x y => ChoiceEqualityMonad.bind_code (L1 := L1) (is_true0 := is_true0) (lift_to_both y) (f x)) init. *)
 
-Global Notation "'foldibnd' s 'to' e 'for' z '>>' f" := (foldi_bind_code s e (Ok z) f) (at level 50).
+(* Global Notation "'foldibnd' s 'to' e 'for' z '>>' f" := (foldi_bind_code s e (Ok z) f) (at level 50). *)
 
 (* Global Notation "'ifbnd' b 'then' x 'else' y '>>' f" := (if b then f x else f y) (at level 200). *)
 (* Global Notation "'ifbnd' b 'thenbnd' x 'else' y '>>' f" := (if b then (ChoiceEqualityMonad.bind_code x) f else f y) (at level 200). *)
@@ -2267,380 +1559,227 @@ Infix "<=.?" := leb (at level 42) : hacspec_scope.
 Infix ">.?" := gtb (at level 42) : hacspec_scope.
 Infix ">=.?" := geb (at level 42) : hacspec_scope.
 
-(* Ltac ssprove_valid_location := *)
-(*   try repeat (try (apply eqtype.predU1l ; reflexivity) ; try apply eqtype.predU1r). *)
-
-Ltac ssprove_valid_location :=
-  repeat
-    (try reflexivity ;
-     try (rewrite fset_cons ;
-          apply (ssrbool.introT (fsetU1P _ _ _)) ;
-          try (left ; reflexivity) ;
-          right)).
-
-
-Ltac ssprove_valid_program :=
-  try (apply prog_valid) ;
-  try (apply valid_scheme ; apply prog_valid).
-
-Ltac destruct_choice_type_prod :=
-  try match goal with
-  | H : choice.Choice.sort (chElement (loc_type ?p)) |- _ =>
-      unfold p in H ;
-      unfold loc_type in H ;
-      unfold "_ .π1" in H
-  end ;
-  try match goal with
-  | H : @T (prod_ChoiceEquality _ _) |- _ =>
-      destruct H
-  end ;
-  try repeat match goal with
-  | H : choice.Choice.sort
-         (chElement
-            (@ct
-               (prod_ChoiceEquality _ _))) |- _ =>
-      destruct H
-  end ;
-  repeat match goal with
-         | H : prod _ _ |- _ => destruct H
-         end.
-
-Ltac ssprove_valid_2 :=
-  (* destruct_choice_type_prod ; *)
-  ssprove_valid ;
-  ssprove_valid_program ;
-  ssprove_valid_location.
-
-Check ct.
-
-Theorem single_mem : forall m, 
-Datatypes.is_true
-    (@ssrbool.in_mem
-       (Ord.sort (@tag_ordType choice_type_ordType (fun _ : choice_type => nat_ordType)))
-       m
-       (@ssrbool.mem
-          (Ord.sort
-             (@tag_ordType choice_type_ordType (fun _ : choice_type => nat_ordType)))
-          (fset_predType
-             (@tag_ordType choice_type_ordType (fun _ : choice_type => nat_ordType)))
-          (@fset (@tag_ordType choice_type_ordType (fun _ : choice_type => nat_ordType))
-             (@cons (@sigT choice_type (fun _ : choice_type => nat)) m
-                    (@nil (@sigT choice_type (fun _ : choice_type => nat))))))).
+Lemma foldi_nat_both :
+  forall {A : ChoiceEquality} {L : {fset Location}} {I} (lo hi : nat)
+    (b : nat -> A -> both L I A)
+    (* (f_state : nat -> A -> raw_code A) *)
+    (* (f_pure : nat -> A -> A) *)
+    (v : A),
+    (* (lo <= hi)%nat -> *)
+  ⊢ ⦃ true_precond ⦄
+      @foldi_nat _ lo hi (fun n v => @is_state _ _ _ (b n v)) v
+  ≈
+  lift_to_both (L := L) (I := [interface]) (Hacspec_Lib_Pre.foldi_nat lo hi (fun n v => @is_pure _ _ _ (b n v)) v)
+  ⦃ pre_to_post true_precond ⦄.
 Proof.
   intros.
-  rewrite <- (@fset1E (@tag_ordType choice_type_ordType (fun _ : choice_type => nat_ordType))).
-  rewrite (ssrbool.introT (fset1P _ _)) ; reflexivity.
-Qed.
+  unfold prog, lift_to_both.
+
+  unfold foldi_nat.
+  unfold Hacspec_Lib_Pre.foldi_nat.
+
+    destruct (_ - lo).
+  { apply r_ret ; intros ; subst. 
+    split.
+    - easy.
+    - easy.
+  }
   
-(* Notation "ct( x , y , .. , z )" := (pair_ChoiceEquality .. (pair_ChoiceEquality x y) .. z) : hacspec_scope. *)
-
-
-
-(* Locate "=.?". *)
-
-(* Definition le_is_ord_leq2 : forall (s s0 : Location), *)
-(*     eqb (ssrfun.tagged s) (ssrfun.tagged s0) = false ->  *)
-(*     eqtype.eq_op (ssrfun.tag s) (ssrfun.tag s0) = false -> *)
-(*     s <.? s0 = (s <= s0)%ord. *)
-(* Proof. *)
-(*   intros s s0. *)
-(*   unfold "<.?" , location_comparable , eq_dec_lt_Comparable , location_ltb , "<?". *)
-(*   unfold eqtype.tagged_as, ssrfun.tagged , ssrfun.tag , ".π1" , ".π2". *)
-(*   intros e H. *)
-(*   destruct s , s0. *)
-
-(*   replace (((x; n) <= (x0; n0))%ord) with (x < x0)%ord. *)
-(*   2 : {     *)
-(*     cbn. *)
-(*     unfold tag_leq. *)
-(*     cbn. *)
-(*     cbn in H. *)
-(*     replace (choice_type_test x x0) with false by apply H. *)
-(*     cbn. *)
-(*     rewrite Bool.orb_false_r. *)
-(*     reflexivity. *)
-(*   }   *)
-
-  
-  
-(*   replace (eqtype.eq_op (ssrfun.tag (x; n)) (ssrfun.tag (x0; n0))) with false. *)
-  
-(*   rewrite le_is_ord_leq by apply e. *)
-
-  
-  
-(*   generalize dependent n. *)
-(*   induction n0 ; intros. *)
-(*   * destruct s ; easy. *)
-(*   * destruct s. reflexivity. *)
-(*     (* unfold Nat.leb ; fold Nat.leb. *) *)
-(*     cbn. *)
-(*     cbn in IHs0. *)
-(*     rewrite IHs0. *)
-(*     reflexivity. *)
-(*     assumption. *)
-(* Qed. *)
-
-Definition location_lebP : (tag_leq (I:=choice_type_ordType) (T_:=fun _ : choice_type => nat_ordType)) = leb.
-Proof.
-  symmetry.
-  do 2 (apply functional_extensionality ; intro).
-  unfold tag_leq.
-  unfold "<=.?".
-  unfold location_comparable.
-  unfold eq_dec_lt_Comparable.
-  destruct (@eqb Location _ x x0) eqn:x_eq_x0.
-  - cbn in x_eq_x0.
-    rewrite location_is_types by apply x_eq_x0.    
-    unfold eqtype.tagged_as.
-    destruct eqtype.eqP.
-    + rewrite (Couplings.reflection_nonsense _ (ssrfun.tagged x) (ssrfun.tagged x0) x_eq_x0).
-      unfold eq_rect_r , eq_rect ; destruct eq_sym.
-      rewrite Ord.leqxx.
-      rewrite Bool.orb_true_r.
-      reflexivity. 
-    + exfalso.
-      apply n.
-      apply Couplings.reflection_nonsense.
-      apply (location_is_types x x0 x_eq_x0).
-  - unfold location_ltb.
-    pose (location_eqbP x x0).
-    destruct x , x0.
-    cbn in x_eq_x0.
-    cbn in e.
-    rewrite x_eq_x0 in e.
-    symmetry in e.
-    unfold eqtype.tag_eq in e.
-    unfold eqtype.tagged_as, ssrfun.tagged , ssrfun.tag , ".π1" , ".π2" in e.
-    
-    unfold eqtype.tagged_as, ssrfun.tagged , ssrfun.tag , ".π1" , ".π2".
-    destruct eqtype.eqP.
-    + subst.
-      unfold eq_rect_r , eq_rect in * ; destruct eq_sym.
-      rewrite choice_type_refl in e.
-      rewrite Bool.andb_true_l in e.
-
-      rewrite Ord.ltxx.
+  generalize dependent lo.
+  clear.
+  generalize dependent v.
       
-      rewrite Bool.orb_false_l.
-      rewrite Bool.andb_true_l.
-
-      apply le_is_ord_leq.
-      assumption.
-    + exfalso.
-      admit.
-Admitted.
-
-
-
-Ltac ssprove_valid_location' :=
-  apply loc_compute ; repeat (try (left ; reflexivity) ; right) ; try reflexivity.
-
-Fixpoint uniqb {A} `{EqDec A} (s : list A) :=
-  match s with
-  | cons x s' => andb (negb (Inb x s')) (uniqb s')
-  | _ => true
-  end.
-
-Theorem uniq_is_bool : forall (l : list (tag_ordType (I:=choice_type_ordType) (fun _ : choice_type => nat_ordType))), seq.uniq l = uniqb l.
-Proof.
-  cbn ; intros.
-  induction l.
-  - reflexivity.
+  induction n ; intros.
   - cbn.
-    f_equal.
-    + f_equal.
-      rewrite loc_compute_b.
-      reflexivity.
-    + exact IHl.
-Qed.        
+    unfold repr.
     
-Theorem simplify_fset : forall l,
-    is_true
-    (path.sorted leb l) ->
-    is_true (uniqb l) ->
-    (@FSet.fsval (@tag_ordType choice_type_ordType (fun _ : choice_type => nat_ordType))
-       (@fset _
-              l)) = (l).
-  intros l is_sorted  is_unique.
-  unfold fset ; rewrite ssreflect.locked_withE.
-  cbn.
-  rewrite <- uniq_is_bool in is_unique.
-  rewrite seq.undup_id by assumption.
-  rewrite path.sorted_sort.
-  - reflexivity.
-  - destruct (tag_leqP (I:=choice_type_ordType) (fun _ : choice_type => nat_ordType)) as [ _ trans _ _ ].
-    apply trans.
-  - rewrite location_lebP.
-    assumption.  
+    replace (fun cur' : choice.Choice.sort (chElement (@ct A)) =>
+               @ret (chElement (@ct A)) (@T_ct A (@ct_T A cur'))) with (@ret (chElement (@ct A))) by (apply functional_extensionality ; intros ; now rewrite T_ct_id).
+    rewrite bind_ret.
+    apply (@code_eq_proof_statement).
+    
+  - rewrite <- foldi__nat_move_S.
+    rewrite <- Hacspec_Lib_Pre.foldi__nat_move_S.
+
+    pose @r_bind_trans_both.
+    specialize r with (b := (b lo v)).
+
+    rewrite <- (ct_T_id is_pure).
+                            
+    specialize r with (g := fun temp => @ret (chElement (@ct A))
+       (@T_ct A
+          (@Hacspec_Lib_Pre.foldi_nat_ (@T A) (S n) (S lo)
+             (fun (n0 : nat) (v0 : @T A) => @is_pure L I A (b n0 v0))
+             (ct_T temp)))).
+    apply r.
+    intros.
+    apply IHn.
 Qed.
 
-Theorem simplify_sorted_fset : forall l,
-    is_true (uniqb l) ->
-    (@FSet.fsval (@tag_ordType choice_type_ordType (fun _ : choice_type => nat_ordType))
-       (@fset _  (path.sort (leb : Location -> Location -> bool) l))) = (path.sort (leb : Location -> Location -> bool) l).
+Lemma foldi_both :
+  forall {A : ChoiceEquality} {L I} lo hi
+    (b : uint_size -> A -> both L I A)
+     v,
+    (unsigned lo <= unsigned hi)%Z ->
+  ⊢ ⦃ true_precond ⦄
+     @foldi _ lo hi L I (fun x y => @is_state _ _ _ (b x y))  v
+  ≈
+     lift_to_both (L := L) (I := I) (Hacspec_Lib_Pre.foldi lo hi (fun x y => @is_pure _ _ _ (b x y)) v)
+  ⦃ pre_to_post true_precond ⦄. (* fun '(a, _) '(b, _) => a = b *)
 Proof.
   intros.
-  apply simplify_fset.
-  apply path.sort_sorted ; pose location_lebP ; cbn ; cbn in e ; rewrite <- e ; apply Ord.leq_total.
-  rewrite <- uniq_is_bool.
-  rewrite path.sort_uniq.
-  rewrite uniq_is_bool.
+  unfold foldi.
+  unfold prog.
+  rewrite foldi_to_foldi_nat by apply H.
+
+  unfold lift_to_both.
+  rewrite Hacspec_Lib_Pre.foldi_to_foldi_nat by apply H.
+
+  eapply (foldi_nat_both).
+Qed.
+
+(* Class both L I (A : ChoiceEquality) := *)
+(*   { *)
+(*     is_pure : A ; *)
+(*     is_state : code L I (@ct A) ; *)
+(*     code_eq_proof_statement : *)
+(*     ⊢ ⦃ true_precond ⦄ *)
+(*           is_state ≈ lift_to_code (L := L) (I := I) (is_pure) *)
+(*       ⦃ pre_to_post true_precond ⦄ *)
+(*   }. *)
+(* Coercion is_pure : both >-> T. *)
+(* Coercion is_state : both >-> code. *)
+
+Lemma foldi_as_both :
+  forall {A : ChoiceEquality} {L I} lo hi
+    (state : uint_size -> A -> code L I (@ct A))
+    (pure : uint_size -> A -> @T A)
+     v,
+    (unsigned lo <= unsigned hi)%Z ->
+    (forall x y,
+    ⊢ ⦃ true_precond ⦄ 
+        state x y ≈ lift_to_code (L := L) (I := I) (pure x y)
+    ⦃ pre_to_post true_precond ⦄) ->
+  ⊢ ⦃ true_precond ⦄
+     @foldi _ lo hi L I state v
+  ≈
+     lift_to_both (L := L) (I := I) (Hacspec_Lib_Pre.foldi lo hi pure v)
+  ⦃ pre_to_post true_precond ⦄. 
+Proof.
+  intros.
+  apply foldi_both with (b := fun x y => Build_both L I A (pure x y) (state x y) (H0 x y)).
   apply H.
 Qed.
-  
-Theorem tag_leq_simplify :
-  forall (a b : Location),
-    is_true (ssrfun.tag a <= ssrfun.tag b)%ord ->
-    is_true (ssrfun.tagged a <= ssrfun.tagged b)%ord ->
-    is_true (tag_leq (I:=choice_type_ordType) (T_:=fun _ : choice_type => nat_ordType) a b).
+
+(*** For loop again *)
+
+(* SSProve for loop is inclusive upperbound, while hacspec is exclusive upperbound *)
+Definition for_loop_range
+  (lo: nat)
+  (hi: nat)
+  (f : nat -> raw_code 'unit) : raw_code 'unit :=
+  match hi - lo with
+  | O => @ret 'unit tt
+  | S i => for_loop (fun n => f (n + lo)) i
+  end.
+
+Definition ChoiceEqualityLocation := ∑ (t : ChoiceEquality), nat.
+Definition CE_loc_to_loc (x : ChoiceEqualityLocation) : Location :=
+  let (k, n) := x in
+  (@ct k; n).
+Definition CE_loc_to_CE (x : ChoiceEqualityLocation) : ChoiceEquality :=
+  let (k, n) := x in
+  k.
+Coercion CE_loc_to_loc : ChoiceEqualityLocation >-> Location.
+Coercion CE_loc_to_CE : ChoiceEqualityLocation >-> ChoiceEquality.
+
+Fixpoint list_types_ (l : list ChoiceEquality) (init : ChoiceEquality) : ChoiceEquality  :=
+  match l with
+  | (t :: ts) => list_types_ ts t '× init
+  | [] => init
+  end.
+
+Fixpoint list_types (l : list ChoiceEquality) : ChoiceEquality :=
+  match l with
+  | [] => unit_ChoiceEquality
+  | (t :: ts) => list_types_ ts t
+  end.
+
+Program Fixpoint vars_to_tuple (vars : list (∑ (t : ChoiceEquality), t)) {measure (length vars)} : list_types (seq.map (fun '(x ; y) => x) vars)  :=
+  match vars with
+  | [] => @ct_T unit_ChoiceEquality tt
+  | (x :: xs) =>
+      match xs with
+      | [] => _
+      | (s :: xs) => (vars_to_tuple (s :: xs) , _)
+      end
+  end.
+
+Fixpoint for_loop_return_ (ℓ : list ChoiceEqualityLocation) (vars : list (∑ (t : ChoiceEquality), t)) : raw_code (list_types (seq.cat (seq.map (fun '(x ; y) => x) vars) (seq.map (fun '(x ; y) => x) ℓ) )).
+  (* Set Printing Implicit. *)
+  destruct ℓ as [ | l ls ].
+  - rewrite seq.cats0.
+    pose (ret (vars_to_tuple vars)).
+    replace (fun pat : ∑ t : ChoiceEquality, @T t => _) with
+      (fun pat : @sigT ChoiceEquality
+       (fun t : ChoiceEquality => @T t) =>
+         match pat return ChoiceEquality with
+         | @existT _ _ x _ => x
+         end)
+      in r by (apply functional_extensionality ; now intros []).
+    apply r.
+  - apply (getr l).
+    intros x.
+    destruct l.
+    cbn in x.
+    pose (for_loop_return_ ls (vars ++ [(_ ; ct_T x)])).
+    rewrite seq.map_cat in r.
+    cbn in r.
+    rewrite <- seq.catA in r.
+    cbn in r.
+    apply r.
+Defined.    
+Definition for_loop_return (ℓ : list ChoiceEqualityLocation) : raw_code (list_types (seq.map (fun '(x ; y) => x) ℓ)) := for_loop_return_ ℓ [].
+
+Definition for_loop_locations
+           (lo: nat)
+           (hi: nat)
+           (ℓ : list ChoiceEqualityLocation)
+           (f : nat -> raw_code 'unit) :=
+  match hi - lo with
+  | O => @ret 'unit tt
+  | S i => for_loop (fun n => f (n + lo)) i
+  end  ;; for_loop_return ℓ.
+
+Theorem empty_put {B} ℓ v (k h : raw_code B) :
+  ⊢ ⦃ true_precond ⦄ k ≈ h ⦃ pre_to_post true_precond ⦄ ->
+  ⊢ ⦃ true_precond ⦄ #put ℓ := v ;; k ≈ h ⦃ pre_to_post true_precond ⦄.
 Proof.
-  intros [] [].
-  
-  unfold tag_leq.
-  unfold eqtype.tagged_as, ssrfun.tagged , ssrfun.tag , ".π1" , ".π2".
+  intros.
+  step_code.
+  eapply rpre_weaken_rule.
+  apply H.
+  intros.
+  reflexivity.
+Qed.  
 
-  intro.
-  rewrite Ord.leq_eqVlt in H.
-  rewrite is_true_split_or in H.
-  destruct H.
-  - apply Couplings.reflection_nonsense in H ; subst.
-    
-    rewrite Ord.ltxx.
-    rewrite Bool.orb_false_l.
-    rewrite eqtype.eq_refl.
-    rewrite Bool.andb_true_l.
-    
-    destruct eqtype.eqP.
-    + unfold eq_rect_r , eq_rect ; destruct eq_sym.
-      trivial.
-    + contradiction.
-  - rewrite H ; clear H.
-    reflexivity.    
-Qed.
-  
-Theorem tag_leq_inverse :
-  forall a b,
-    tag_leq (I:=choice_type_ordType) (T_:=fun _ : choice_type => nat_ordType) a b
-    =
-      negb (tag_leq (I:=choice_type_ordType) (T_:=fun _ : choice_type => nat_ordType)
-                    b a) ||
-           eqtype.eq_op (ssrfun.tag a) (ssrfun.tag b) &&
-        eqtype.eq_op (ssrfun.tagged a) (ssrfun.tagged b).
+Theorem forget_precond {B} (x y : raw_code B) P Q :
+  ⊢ ⦃ true_precond ⦄ x ≈ y ⦃ Q ⦄ -> 
+  ⊢ ⦃ P ⦄ x ≈ y ⦃ Q ⦄. 
 Proof.
-  intros [a b] [c d].
-  unfold tag_leq.
-  
-  rewrite Bool.negb_orb.
-  rewrite Bool.negb_andb.
-  rewrite Bool.andb_orb_distrib_r.
-
-  unfold eqtype.tagged_as.
-  unfold ssrfun.tagged , ssrfun.tag , ".π1" , ".π2".
-  rewrite <- Bool.orb_assoc.
-  
-  f_equal.
-  - rewrite <- Bool.negb_orb.    
-    rewrite <- Bool.orb_comm.
-    rewrite <- Ord.leq_eqVlt.
-    rewrite <- Ord.ltNge.
-    reflexivity.
-  - destruct (eqtype.eq_op a c) eqn:a_eq_c.
-    + apply Couplings.reflection_nonsense in a_eq_c.
-      subst.
-      do 2 rewrite Bool.andb_true_l.
-
-      destruct eqtype.eqP. 2: contradiction.
-      
-      unfold eq_rect_r , eq_rect.
-      destruct eq_sym.
-
-      rewrite Ord.leq_eqVlt.
-      rewrite Bool.orb_comm.
-
-      f_equal.
-      rewrite <- Ord.ltNge.
-      rewrite Ord.ltxx.
-      reflexivity.
-    + do 2 rewrite Bool.andb_false_l.
-      rewrite Bool.orb_false_r.
-      symmetry.
-
-      destruct eqtype.eqP.
-      { subst. rewrite eqtype.eq_refl in a_eq_c. discriminate a_eq_c. }
-
-      rewrite Ord.eq_leq by reflexivity.
-      rewrite Bool.andb_false_r.
-      reflexivity.
+  intros.
+  eapply rpre_weaken_rule.
+  apply H.
+  intros.
+  reflexivity.
 Qed.
-
-Ltac incl_compute :=
-  now (apply list_incl_compute ; cbn ; reflexivity).
-
-(* Ltac incl_b_compute := *)
-(*   let H := fresh in *)
-(*   intro H ; *)
-(*   repeat rewrite is_true_split_or in H ; *)
-(*   decompose [and or] H ; clear H ; *)
-(*   [ repeat rewrite is_true_split_or ; *)
-(*     repeat (try (left ; assumption) ; right) *)
-(*   | discriminate ]. *)
-
-(* Ltac incl_compute := *)
-(*   now (unfold List.incl ; intros [] ; repeat rewrite <- in_bool_eq ; unfold Inb ; incl_b_compute). *)
-
-(* Lemma valid_inject_loc_b : *)
-(*   forall (import : Interface) (A : choiceType) *)
-(*     (L1 L2 : {fset tag_ordType (I:=choice_type_ordType) (fun _ : choice_type => nat_ordType)}) *)
-(*     (v : raw_code A), *)
-(*     List.incl (path.sort leb L1) (path.sort leb L2). *)
-(* Proof. *)
-(*   intros. *)
-(*   rewrite simplify_sorted_fset by reflexivity. *)
-(*   eapply (valid_injectLocations_b) with (L1 := L1). *)
-(*   [ rewrite simplify_sorted_fset by reflexivity  *)
-(*     ; rewrite simplify_sorted_fset by reflexivity *)
-(*     ; cbn   *)
-(*     ; incl_compute *)
-(*   | .. ]    . *)
-(* Qed. *)
-
-(* eapply (valid_injectLocations_b) with (L1 := _) ; *)
-
-Ltac valid_sorted_incl :=
-  rewrite simplify_sorted_fset by reflexivity 
-    ; rewrite simplify_sorted_fset by reflexivity
-    ; cbn  
-    ; incl_compute.
-
-Ltac valid_program :=
-  (* match goal with *)
-  (* | |- (ValidCode _ _ (@prog _ _ _ (?program))) => apply program *)
-  (* end. *)
-  match goal with
-  | |- (ValidCode _ _ (@prog _ _ _ ?program)) =>
-      pose program ;
-      match goal with
-      | H : (code ?fset _ _) |- _ =>          
-          eapply (valid_injectLocations_b) with (L1 := fset) ;
-          [ | apply program ]
-      end           
-  end ; valid_sorted_incl .
 
 Ltac ssprove_valid' :=
-  repeat (valid_program
-          || (apply valid_bind ; [apply valid_scheme ; apply prog_valid | intros])
-          || (apply valid_bind ; [ | intros ; ssprove_valid' ])
-          || (apply ChoiceEqualityMonad.bind_code) 
+  repeat ((apply valid_bind ; [apply valid_scheme ; apply prog_valid | intros])
+          || (apply valid_bind ; [valid_program | intros])
+          (* || (apply ChoiceEqualityMonad.bind_code)  *)
           || (apply valid_putr ; [ cbn ; ssprove_valid_location | ])
           || (apply valid_getr ; [ cbn ; ssprove_valid_location | intros])
-          (* || (apply valid_foldi ; intros) *)
-          || (unfold for_loop_usize, for_loop_range ;
-             (* match goal with *)
-            (* | [ |- context[match ?x with | true => _ | false => _ end] ] => *)
-                (* destruct x ; [ |  *)apply valid_for_loop ; intros (* ] *)
-            (* end *)
-             )
           || match goal with
             | [ |- context[match ?x with | true => _ | false => _ end] ] =>
                 destruct x
@@ -2653,210 +1792,132 @@ Ltac ssprove_valid' :=
             | [ |- context[let _ := ct_T ?x in _] ] =>
                 destruct ct_T
             end
-          || apply valid_ret).
+          || apply valid_ret
+          (* || (match goal with *)
+          (*    | [ |- context [ValidCode (fset ?xs) _ (@prog _ _ _ (@foldi _ ?lo ?hi (fset ?xs) _ ?f ?v))] ] => *)
+          (*        apply valid_foldi_pre *)
+          (*    end) *)
+          || (match goal with
+             | [ |- context [ValidCode (fset ?ys) _ (@prog _ _ _ (@foldi _ ?lo ?hi (fset ?xs) _ ?f ?v))] ] =>
+                 eapply (valid_subset xs ys) ; [ | apply valid_foldi_pre ] ; incl_compute
+             end)
+             ).
 
-Ltac ssprove_valid'_2 :=
-  destruct_choice_type_prod ;
-  ssprove_valid' ;
-  ssprove_valid_program ;
-  ssprove_valid_location.
+Check path.merge_sort_rec.
 
-Definition heap_ignore_post fset {A} : postcond A A :=
-  fun '(a, h₀) '(b, h₁) => a = b /\ heap_ignore fset (h₀ , h₁).
-
-Class both fset (A : ChoiceEquality) :=
-  {
-    is_pure : A ;
-    is_state : code fset [interface] (@ct A) ;
-    code_eq_proof_statement : ⊢ ⦃ (fun '(h0, h1) => heap_ignore fset (h0, h1)) ⦄  is_state ≈ lift_to_code (L := fset.fset0) (I := [interface]) (is_pure) ⦃ heap_ignore_post fset ⦄
-  }.
-Coercion is_pure : both >-> T.
-Coercion is_state : both >-> code.
-
-(* Class CodeEqProofStatement  {fset} {A : ChoiceEquality} `(b : @both fset A) := *)
-(*   code_eq_proof_statement : ⊢ ⦃ (fun '(h0, h1) => heap_ignore fset (h0, h1)) ⦄  is_state ≈ lift_to_code (L := fset.fset0) (I := [interface]) (is_pure) ⦃ heap_ignore_post fset ⦄. *)
-
-Theorem bind_both {A B : ChoiceEquality} {fset}  `{b : @both fset A} (* `{code_bind : @CodeEqProofStatement fset A b } *)
-    (k : choice.Choice.sort A -> raw_code B) :
-    (forall a₀ a₁ : choice.Choice.sort A, ⊢ ⦃ fun '(s₀, s₁) => heap_ignore_post fset (a₀, s₀) (a₁, s₁) ⦄ k a₀ ≈ k a₁ ⦃ heap_ignore_post fset ⦄) ->
-    ⊢ ⦃ (fun '(h₀, h₁) => heap_ignore fset (h₀ , h₁)) ⦄
-        (@bind A B is_state k)
-        ≈
-        (@bind A B (lift_to_code (L := fset.fset0) (I := [interface]) is_pure) k)
-    ⦃ heap_ignore_post fset ⦄.
-Proof. exact (r_bind (is_state) ((lift_to_code (L := fset.fset0) (I := [interface]) is_pure)) k k (heap_ignore fset) (heap_ignore_post fset) (heap_ignore_post fset) code_eq_proof_statement). Qed.
-
-Ltac bind_both_function :=
-  match goal with
-  | [ |- context [ ⊢ ⦃ ?P ⦄ (@bind _ _ (_ (_ ?code_fun) ) ?k) ≈ _ ⦃ ?Q ⦄ ]] =>
-      apply (@bind_both _ _ _ Q (code_eq_proof_statement code_fun) k)
-  end.
-     (* match goal with *)
-  (* | [ |- context [ ⊢ ⦃ ?P ⦄ (@bind _ _ (_ (?proj_fun ?code_fun) ) ?k) ≈ _ ⦃ ?Q ⦄ ]] => *)
-  (*     apply (r_bind  (proj_fun code_fun) (prog (lift_to_code (L := fset.fset0) (I := [interface]) code_fun)) k k P (fun '(a, _) '(b, _) => a = b) Q) ; [apply code_eq_proof_statement | intros ..] *)
-  (* end. *)
-
-Theorem bind_rewrite : forall (A B : ChoiceEquality) x f, @bind A B (ret x) f = f x.
-Proof ltac:(reflexivity).
-
-Ltac clear_bind :=
-  rewrite bind_rewrite
-  ||
-  bind_both_function.
-
-Ltac progress_step_code :=
-  match goal with
-  | [ |- context [ ⊢ ⦃ _ ⦄ (#put ?l := ?x ;; (getr ?l ?a)) ≈ _ ⦃ _ ⦄ ]] =>
-      apply (r_transL (#put l := x ;; a x )) ;
-      [ apply (r_put_get _ l x a) | ]
-  end
-  ||
-  match goal with
-  | [ |- context [ ⊢ ⦃ _ ⦄ (#put ?l := ?x ;; (putr ?l ?y ?a)) ≈ _ ⦃ _ ⦄ ]] =>
-      apply (r_transL (#put l := y ;; a )) ;
-      [ apply contract_put | ]
-  end
-  ||
-  match goal with
-  | [ |- context [ ⊢ ⦃ _ ⦄ (#put ?l := ?x ;; ?a) ≈ ?b ⦃ _ ⦄ ]] =>
-      apply (r_put_lhs l x a b (* (fun '(h0, h1) => heap_ignore fset (h0, h1)) *))
-  end
-  ||
-  apply r_ret.
-
-Ltac step_code :=
-  repeat (clear_bind || progress_step_code).
-
-Lemma foldi_both :
-  forall {A : ChoiceEquality} {L} lo hi
-    (f_state : uint_size -> A -> code L [interface] A)
-    (f_pure : uint_size -> A -> A) v,
-    (unsigned lo <= unsigned hi)%Z ->
-    forall (P : precond), (forall x, P (x , x)) ->
-    (forall (i : uint_size) (v : A),
-        ⊢ ⦃ fun '(s₀, s₁) => P (s₀, s₁) /\ s₀ = s₁ ⦄
-            f_state i v
-          ≈
-            ret (f_pure i v)
-          ⦃ eq ⦄) ->
-  ⊢ ⦃ fun '(s₀, s₁) => s₀ = s₁ ⦄
-     @foldi _ lo hi L [interface] f_state v 
-  ≈
-     lift_to_code (L := L) (I := [interface]) (Hacspec_Lib_Pre.foldi lo hi f_pure v) 
-  ⦃ eq ⦄. (* fun '(a, _) '(b, _) => a = b *)
+Theorem length_merge_sort_pop : forall {A} leb (l1 : list (list A)) (l2 : list A),
+    length (path.merge_sort_pop leb l2 l1) = length (seq.cat (seq.flatten l1) l2).
 Proof.
   intros.
-  unfold foldi.
-  unfold prog.
-  rewrite foldi_to_foldi_nat by apply H.
-
-  unfold lift_to_code.
-  rewrite Hacspec_Lib_Pre.foldi_to_foldi_nat by apply H.
-
-  unfold foldi_nat.  
-  unfold Hacspec_Lib_Pre.foldi_nat.
-
-  set (r := Z.to_nat (unsigned lo)).
-  destruct (_ - r) ; [ apply r_ret ; intros ; subst ; reflexivity | ].
-
-  generalize dependent r.
-  clear -H0 H1.
-  generalize dependent v.
-  
-  induction n ; intros.
+  generalize dependent l2.
+  induction l1 ; intros.
   - cbn.
-    unfold repr.
-    
-    replace (fun cur' : choice.Choice.sort (chElement (@ct A)) =>
-               @ret (chElement (@ct A)) (@T_ct A (@ct_T A cur'))) with (@ret (chElement (@ct A))) by (apply functional_extensionality ; intros ; now rewrite T_ct_id).
-    rewrite bind_ret.
-    eapply rpre_weaken_rule.
-    apply H1. intros ; subst ; split ; easy.
-  - rewrite <- foldi__nat_move_S.
-    rewrite <- Hacspec_Lib_Pre.foldi__nat_move_S.
-
-    replace (ret
-       (T_ct
-          (Hacspec_Lib_Pre.foldi_nat_ (S n) (S r)
-                                      (fun x : nat => f_pure (repr (Z.of_nat x))) (f_pure (repr (Z.of_nat r)) v)))) with
-      (pu ← lift_to_code (L := L) (I := [interface]) (f_pure (repr (Z.of_nat r)) v) ;;
-        ret
-       (T_ct
-          (Hacspec_Lib_Pre.foldi_nat_ (S n) (S r)
-                                      (fun x : nat => f_pure (repr (Z.of_nat x))) (ct_T pu)))).
-
-    pose (@r_bind).
-    eapply (@r_bind) with (mid := eq).    
-    eapply rpre_weaken_rule.
-    apply H1. intros ; subst ; split ; easy.
-    intros.
-    specialize IHn with (v := (ct_T a₁)) (r := S r).
-    apply (r_transR _ (foldi_nat_ (S n) (S r)
-       (fun (x : nat) (x0 : T) => prog (f_state (repr (Z.of_nat x)) x0)) 
-       (ct_T a₁))).
-    apply IHn.
-    apply rpre_hypothesis_rule.
-    intros ; inversion H ; subst.
-    eapply rpre_weaken_rule.    
-    apply @rreflexivity_rule.
-    intros sa sb [].
-    cbn in *.
-    subst.
     reflexivity.
-
-    unfold prog.
-    unfold lift_to_code.
-    rewrite bind_rewrite.
-    rewrite ct_T_id.
+  - cbn.
+    rewrite IHl1.
+    rewrite seq.size_cat.    
+    rewrite seq.size_cat.
+    rewrite seq.size_cat.        
+    rewrite path.size_merge.    
+    rewrite seq.size_cat.    
+    rewrite ssrnat.addnA.    
+    f_equal.
+    rewrite ssrnat.addnC.
     reflexivity.
 Qed.
 
-Ltac heap_ignore_remove_ignore :=
-  match goal with
-  | H : heap_ignore ?L ( ?a , ?b ) |- _ =>
-      match goal with
-      | [ |- context[ heap_ignore L ( ?c , b ) ] ] =>
-          intros ℓ H_mem
-          ; specialize (H ℓ H_mem)
-          ; match goal with
-            | [ |- context[ get_heap (set_heap ?x ?ℓ' ?v) ℓ = get_heap _ ℓ ] ] =>
-                destruct (@eqtype.eq_op (@eqtype.tag_eqType choice_type_eqType
-             (fun _ : choice_type => ssrnat.nat_eqType)) ℓ ℓ') eqn:ℓ_eq_ℓ'
-                ; [ exfalso
-                    ; apply (ssrbool.elimT eqtype.eqP) in ℓ_eq_ℓ' ; subst
-                    ; apply (ssrbool.elimT ssrbool.negP) in H_mem
-                    ; apply H_mem
-                    ; clear H_mem
-                    ; apply loc_compute
-                    ; unfold eqtype.val
-                    ; rewrite simplify_sorted_fset
-                    ; repeat (reflexivity || (left ; reflexivity) || right)
-                  | rewrite <- (get_heap_set_heap a ℓ ℓ' v) ;
-                    [ assumption
-                    | rewrite ℓ_eq_ℓ' ; reflexivity 
-                    ]
-                ]     
-            end
-      end
-  end .
+Theorem length_sort_even : forall {A} leb a x (l1 : list (list A)) (l2 : list A),
+    length (path.merge_sort_rec leb l1 (a :: x :: l2)) =
+    length (path.merge_sort_rec leb
+        (path.merge_sort_push leb (if leb a x then [a; x] else [x; a]) l1) l2).
+Proof.
+  reflexivity.
+Qed.
 
-Ltac both_bind :=
-  match goal with
-  | [ |- context[ (?x : both ?L ?T) ] ] =>  
-      match goal with
-      | [ |- context[ (bind ?f ?v) ] ] =>
-          eapply (r_transR (bind (@is_state _ _ x) v) (bind (lift_to_code (@is_pure _ _ x)) v)) ;
-          [ 
-          | eapply r_bind ; [ apply x | ]
-          ]
-      end
-  end.
+Theorem length_sort_is_length' : forall {A} leb (l1 : list (list A)),
+    length (path.merge_sort_rec leb l1 []) = length (seq.flatten l1).
+Proof.
+  destruct l1.
+  + cbn.
+    reflexivity.
+  + cbn.
+    rewrite length_merge_sort_pop.
+    rewrite seq.size_cat.
+    rewrite seq.size_cat.
+    rewrite path.size_merge.
+    rewrite seq.cats0.
+    rewrite ssrnat.addnC.
+    reflexivity.
+Qed.
+
+(* Theorem length_sort_is_length'' : forall {A} leb (l1 : list (list A)) (l2 : list A), *)
+(*     length (path.merge_sort_rec leb l1 l2) = length (seq.cat (seq.flatten l1) l2 ) \/ *)
+(*     (forall x, length (path.merge_sort_rec leb l1 (x :: l2)) = S (length (seq.cat l2 (seq.flatten l1)))). *)
+(* Proof. *)
+(*   intros. *)
+(*   generalize dependent l1. *)
+(*   induction l2. *)
+(*   - intros. left. *)
+(*     rewrite length_sort_is_length'. *)
+(*     rewrite seq.cats0. *)
+(*     reflexivity. *)
+(*   - intros. *)
+(*     cbn. *)
+(*     right. intros. *)
+(*     specialize (IHl2 (path.merge_sort_push leb [x; a] l1)). *)
+(*     destruct IHl2. *)
+(* Admitted. *)
+    
+(* Theorem length_sort_is_length : forall {A} leb (l1 : list (list A)) (l2 : list A), *)
+(*     length (path.merge_sort_rec leb l1 l2) = length (seq.cat l2 (seq.flatten l1)). *)
+(* Proof. *)
+(*   intros. *)
+(* Admitted. *)
+  
+(* Theorem fset_sort_cons : *)
+(*   forall leb (l1 l2 : list Location)  (a : Location), *)
+(*     path.sort leb l1 = path.sort leb l2 <-> *)
+(*     path.sort leb (a :: l1) = path.sort leb (a :: l2). *)
+(* Proof. *)
+(*   unfold path.sort. *)
+(*   set (n := []). *)
+(*   generalize dependent n. *)
+
+(*   assert (forall {A} {l1 l2 : list A}, l1 = l2 -> length l1 = length l2). *)
+(*   { intros. apply f_equal with (f := @length _) in H. apply H. } *)
+(* Admitted. *)
 
 
-Ltac remove_T_ct :=
-  match goal with
-  | [ |- context[ T_ct ?x ] ] =>  
-      replace (T_ct x) with x by reflexivity
-  | H : _ |- context[ T_ct ?x ] =>  
-      replace (T_ct x) with x in H by reflexivity
-  end.
+(* Theorem fset_sort_is_list_in : *)
+(*   forall leb (l1 l2 : list Location), *)
+(*     (forall a, List.In a l1 <-> List.In a l2) <-> *)
+(*     path.sort leb (@seq.undup loc_eqType l1) = path.sort leb (@seq.undup loc_eqType l2). *)
+(* Proof. *)
+(*   induction l1 ; intros. *)
+(*   - destruct l2. *)
+(*     + split ; intros. *)
+(*       * reflexivity. *)
+(*       * reflexivity. *)
+(*     + split ; intros. *)
+(*       * specialize (H l). *)
+(*         exfalso. *)
+(*         apply H. *)
+(*         left. *)
+(*         reflexivity. *)
+(*       * apply f_equal with (f := @length _) in H. *)
+(*         do 2 rewrite path.size_sort in H. *)
+(*         admit. *)
+(*   - split. intros. *)
+(* Admitted. *)
+
+(* Theorem fset_any_sort : *)
+(*   forall leb (l : list Location), *)
+(*     (fset (path.sort leb l)) = (fset l). *)
+(* Proof.   *)
+(* Admitted.   *)
+  
+Ltac ssprove_valid'_2 :=
+  destruct_choice_type_prod
+  ; ssprove_valid'
+  ; ssprove_valid_program
+  ; ssprove_valid_location.
