coq_ssprove/src/Hacspec_Lib_Comparable.v
@@ -1,3 +1,5 @@
+From Coq Require Import ZArith List.
+From Crypt Require Import Package.
 
 Class EqDec (A : Type) :=
   { eqb : A -> A -> bool ;
@@ -24,8 +26,45 @@ Instance eq_dec_lt_Comparable {A : Type} `{EqDec A} (ltb : A -> A -> bool) : Com
     geb a b := if eqb a b then true else ltb b a;
   }.
 
-Theorem eqb_refl : forall {A} {H : EqDec A} (x : A), @eqb A H x x = true.
+Instance eq_dec_le_Comparable {A : Type} `{EqDec A} (leb : A -> A -> bool) : Comparable A := {
+    ltb a b := if eqb a b then false else leb a b;
+    leb := leb ;
+    gtb a b := if eqb a b then false else leb b a;
+    geb a b := leb b a;
+  }.
+
+Theorem eqb_refl : forall {A} {H : EqDec A} (x : A), (@eqb A H x x) = true.
 Proof.
   intros.
   now apply eqb_leibniz.
 Qed.
+
+Theorem eqbP : forall {A} {H : EqDec A} (x y : A), ssrbool.reflect (x = y) (@eqb A H x y).
+Proof.
+  intros.
+  apply Bool.iff_reflect.
+  rewrite <- eqb_leibniz.
+  reflexivity.
+Qed.
+
+Theorem neqb_leibniz : forall {A} {H : EqDec A} x y, eqb x y = false <-> x <> y .
+Proof.
+  intros.
+  rewrite (ssrbool.rwP ssrbool.negPf).  
+  rewrite <- (ssrbool.rwP (@ssrbool.negP (eqb x y))).
+  apply not_iff_compat.
+  apply eqb_leibniz.
+Qed.
+
+
+Global Program Instance nat_eqdec : EqDec nat := {
+  eqb := Nat.eqb;
+  eqb_leibniz := Nat.eqb_eq ;
+}.
+
+Global Instance nat_comparable : Comparable nat := {
+  ltb := Nat.ltb;
+  leb := Nat.leb;
+  gtb a b := Nat.ltb b a;
+  geb a b := Nat.leb b a;
+}.
