coq_ssprove/src/Hacspec_Poly1305.v
@@ -4,7 +4,6 @@ Import PackageNotation.
 From extructures Require Import ord fset.
 From CoqWord Require Import ssrZ word.
 From Jasmin Require Import word.
-Require Import ChoiceEquality.
 
 From Coq Require Import ZArith.
 Import List.ListNotations.
@@ -12,6 +11,9 @@ Open Scope list_scope.
 Open Scope Z_scope.
 Open Scope bool_scope.
 
+
+Require Import ChoiceEquality.
+Require Import LocationUtility.
 Require Import Hacspec_Lib_Comparable.
 Require Import Hacspec_Lib_Pre.
 Require Import Hacspec_Lib.
@@ -46,7 +48,6 @@ Notation "'poly_state_t'" := ((
   poly_key_t
 )) : hacspec_scope.
 
-Import Hacspec_Lib_Pre.
 Definition poly1305_encode_r_pure (b_2 : poly_block_t) : field_element_t :=
   let n_0 : uint128 :=
     uint128_from_le_bytes (array_from_seq (16) (array_to_seq (b_2))) in 
@@ -59,14 +60,12 @@ Definition poly1305_encode_r_pure_code
   : code fset.fset0 [interface] (@ct field_element_t) :=
   {code pkg_core_definition.ret (T_ct (poly1305_encode_r_pure b_2))}.
 
-Import Hacspec_Lib.
 Definition n_0_loc : Location :=
   (uint128 : choice_type ; 8%nat).
 Program Definition poly1305_encode_r_state
   (b_2 : poly_block_t)
-  : code (fset (path.sort leb [ n_0_loc])) [interface] (@ct (
-      field_element_t)) :=
-  (({code  temp_3 ←
+  : code (fset ([ n_0_loc])) [interface] (@ct (field_element_t)) :=
+  (({| prog :=  temp_3 ←
         (array_to_seq (b_2)) ;;
       let temp_3 : seq uint8 :=
         (temp_3) in
@@ -83,52 +82,33 @@ Program Definition poly1305_encode_r_state
         (secret (@repr U128 21267647620597763993911028882763415551)) ;;
       let temp_6 : int128 :=
         (temp_6) in
-      n_0 ← get n_0_loc ;;
-      
       #put n_0_loc := 
         ((n_0) .& (temp_6)) ;;
       n_0 ← get n_0_loc ;;
       
        temp_7 ←
         (nat_mod_from_secret_literal (n_0)) ;;
-      @pkg_core_definition.ret (field_element_t) ( (temp_7)) } : code (fset (
-          path.sort leb [ n_0_loc])) [interface] _)).
+      @pkg_core_definition.ret (field_element_t) ( (
+        temp_7)) ; prog_valid := ltac:(ssprove_valid'_2) |}: code (fset (
+          [ n_0_loc])) [interface] _)).
 Fail Next Obligation.
 
 Program Definition poly1305_encode_r
   (b_2 : poly_block_t)
-  : both (fset (path.sort leb [ n_0_loc])) field_element_t :=
+  : both (fset ([ n_0_loc])) [interface] field_element_t :=
   {|
-  is_pure := poly1305_encode_r_pure(b_2 : poly_block_t);
-  is_state := poly1305_encode_r_state(b_2 : poly_block_t);
+  is_pure := poly1305_encode_r_pure (b_2 : poly_block_t);
+  is_state := poly1305_encode_r_state (b_2 : poly_block_t);
   |}.
 Next Obligation.
-  unfold poly1305_encode_r_pure.
-  unfold poly1305_encode_r_state.
-  unfold is_pure.
-  unfold is_state.
+intros.
+unfold poly1305_encode_r_pure.
+unfold poly1305_encode_r_state.
 
-  unfold prog.
-
-  unfold array_to_seq.
-  unfold array_from_seq.
-  unfold uint128_from_le_bytes.
-  unfold secret.
-  unfold nat_mod_from_secret_literal.
-
-  unfold lift_to_code.
-
-  step_code.
-  intros.
-
-  split ; [reflexivity | ].
-  destruct H.
-  decompose [and or] H ; clear H ; subst.
-  
-  heap_ignore_remove_ignore.
+unfold prog.
+step_code.
 Qed.
 
-Import Hacspec_Lib_Pre.
 Definition poly1305_encode_block_pure (b_9 : poly_block_t) : field_element_t :=
   let n_10 : uint128 :=
     uint128_from_le_bytes (array_from_seq (16) (array_to_seq (b_9))) in 
@@ -141,12 +121,11 @@ Definition poly1305_encode_block_pure_code
   : code fset.fset0 [interface] (@ct field_element_t) :=
   {code pkg_core_definition.ret (T_ct (poly1305_encode_block_pure b_9))}.
 
-Import Hacspec_Lib.
 
 Program Definition poly1305_encode_block_state
   (b_9 : poly_block_t)
   : code (fset.fset0) [interface] (@ct (field_element_t)) :=
-  (({code  temp_12 ←
+  (({| prog :=  temp_12 ←
         (array_to_seq (b_9)) ;;
       let temp_12 : seq uint8 :=
         (temp_12) in
@@ -165,35 +144,26 @@ Program Definition poly1305_encode_block_state
       let temp_16 : field_element_t :=
         (temp_16) in
       @pkg_core_definition.ret (field_element_t) ( ((f_11) +% (
-          temp_16))) } : code (fset.fset0) [interface] _)).
+          temp_16))) ; prog_valid := ltac:(ssprove_valid'_2) |}: code (
+        fset.fset0) [interface] _)).
 Fail Next Obligation.
 
 Program Definition poly1305_encode_block
   (b_9 : poly_block_t)
-  : both (fset.fset0) field_element_t :=
+  : both (fset.fset0) [interface] field_element_t :=
   {|
-  is_pure := poly1305_encode_block_pure(b_9 : poly_block_t);
-  is_state := poly1305_encode_block_state(b_9 : poly_block_t);
+  is_pure := poly1305_encode_block_pure (b_9 : poly_block_t);
+  is_state := poly1305_encode_block_state (b_9 : poly_block_t);
   |}.
 Next Obligation.
-  unfold poly1305_encode_block_pure.
-  unfold poly1305_encode_block_state.
+intros.
+unfold poly1305_encode_block_pure.
+unfold poly1305_encode_block_state.
 
-  unfold prog.
-
-  unfold array_to_seq.
-  unfold array_from_seq.
-  unfold uint128_from_le_bytes.
-  unfold nat_mod_from_secret_literal.
-  unfold nat_mod_pow2.
-
-  unfold lift_to_code.
-
-  step_code.
-  split ; easy.
+unfold prog.
+step_code.
 Qed.
 
-Import Hacspec_Lib_Pre.
 Definition poly1305_encode_last_pure
   (pad_len_17 : block_index_t)
   (b_18 : sub_block_t)
@@ -212,13 +182,12 @@ Definition poly1305_encode_last_pure_code
   {code pkg_core_definition.ret (T_ct (poly1305_encode_last_pure pad_len_17
     b_18))}.
 
-Import Hacspec_Lib.
 
 Program Definition poly1305_encode_last_state
   (pad_len_17 : block_index_t)
   (b_18 : sub_block_t)
   : code (fset.fset0) [interface] (@ct (field_element_t)) :=
-  (({code  temp_21 ←
+  (({| prog :=  temp_21 ←
         (seq_len (b_18)) ;;
        temp_22 ←
         (array_from_slice (default) (16) (b_18) (usize 0) (temp_21)) ;;
@@ -236,38 +205,29 @@ Program Definition poly1305_encode_last_state
       let temp_25 : field_element_t :=
         (temp_25) in
       @pkg_core_definition.ret (field_element_t) ( ((f_20) +% (
-          temp_25))) } : code (fset.fset0) [interface] _)).
+          temp_25))) ; prog_valid := ltac:(ssprove_valid'_2) |}: code (
+        fset.fset0) [interface] _)).
 Fail Next Obligation.
 
 Program Definition poly1305_encode_last
   (pad_len_17 : block_index_t)
   (b_18 : sub_block_t)
-  : both (fset.fset0) field_element_t :=
+  : both (fset.fset0) [interface] field_element_t :=
   {|
-  is_pure := poly1305_encode_last_pure(pad_len_17 : block_index_t)
+  is_pure := poly1305_encode_last_pure (pad_len_17 : block_index_t)
   (b_18 : sub_block_t);
-  is_state := poly1305_encode_last_state(pad_len_17 : block_index_t)
+  is_state := poly1305_encode_last_state (pad_len_17 : block_index_t)
   (b_18 : sub_block_t);
   |}.
 Next Obligation.
-  unfold poly1305_encode_last_pure.
-  unfold poly1305_encode_last_state.
+intros.
+unfold poly1305_encode_last_pure.
+unfold poly1305_encode_last_state.
 
-  unfold prog.
-
-  unfold seq_len.
-  unfold array_from_slice.
-  unfold uint128_from_le_bytes.
-  unfold nat_mod_from_secret_literal.
-  unfold nat_mod_pow2.
-
-  unfold lift_to_code.
-
-  step_code.
-  split ; easy.
+unfold prog.
+step_code.
 Qed.
 
-Import Hacspec_Lib_Pre.
 Definition poly1305_init_pure (k_26 : poly_key_t) : poly_state_t :=
   let r_27 : field_element_t :=
     poly1305_encode_r (array_from_slice (default) (16) (array_to_seq (k_26)) (
@@ -278,12 +238,11 @@ Definition poly1305_init_pure_code
   : code fset.fset0 [interface] (@ct poly_state_t) :=
   {code pkg_core_definition.ret (T_ct (poly1305_init_pure k_26))}.
 
-Import Hacspec_Lib.
 
 Program Definition poly1305_init_state
   (k_26 : poly_key_t)
-  : code (fset (path.sort leb [ n_0_loc])) [interface] (@ct (poly_state_t)) :=
-  (({code  temp_28 ←
+  : code (fset ([ n_0_loc])) [interface] (@ct (poly_state_t)) :=
+  (({| prog :=  temp_28 ←
         (array_to_seq (k_26)) ;;
       let temp_28 : seq uint8 :=
         (temp_28) in
@@ -299,43 +258,26 @@ Program Definition poly1305_init_state
           field_element_t '×
           field_element_t '×
           poly_key_t
-        )) ( ((temp_31, r_27, k_26))) } : code (fset (
-          path.sort leb [ n_0_loc])) [interface] _)).
+        )) ( ((temp_31, r_27, k_26
+        ))) ; prog_valid := ltac:(ssprove_valid'_2) |}: code (fset (
+          [ n_0_loc])) [interface] _)).
 Fail Next Obligation.
 
 Program Definition poly1305_init
   (k_26 : poly_key_t)
-  : both (fset (path.sort leb [ n_0_loc])) poly_state_t :=
+  : both (fset ([ n_0_loc])) [interface] poly_state_t :=
   {|
-  is_pure := poly1305_init_pure(k_26 : poly_key_t);
-  is_state := poly1305_init_state(k_26 : poly_key_t);
+  is_pure := poly1305_init_pure (k_26 : poly_key_t);
+  is_state := poly1305_init_state (k_26 : poly_key_t);
   |}.
 Next Obligation.
-  unfold poly1305_init_pure.
-  unfold poly1305_init_state.
+intros.
+unfold poly1305_init_pure.
+unfold poly1305_init_state.
 
-  unfold prog.
+unfold prog.
+Admitted.
 
-  unfold array_to_seq.
-  unfold array_from_slice.
-  unfold nat_mod_zero.
-
-  unfold lift_to_code.
-
-  step_code.
-  both_bind.
-    
-  apply r_ret.
-  intros ; subst.
-  reflexivity.
-
-  intros.
-  step_code.
-  intros ? ? [] ; subst.
-  split ; easy.
-Qed.
-
-Import Hacspec_Lib_Pre.
 Definition poly1305_update_block_pure
   (b_32 : poly_block_t)
   (st_33 : poly_state_t)
@@ -349,13 +291,12 @@ Definition poly1305_update_block_pure_code
   : code fset.fset0 [interface] (@ct poly_state_t) :=
   {code pkg_core_definition.ret (T_ct (poly1305_update_block_pure b_32 st_33))}.
 
-Import Hacspec_Lib.
 
 Program Definition poly1305_update_block_state
   (b_32 : poly_block_t)
   (st_33 : poly_state_t)
   : code (fset.fset0) [interface] (@ct (poly_state_t)) :=
-  (({code let '(acc_34, r_35, k_36) :=
+  (({| prog := let '(acc_34, r_35, k_36) :=
         (st_33) : (field_element_t '× field_element_t '× poly_key_t) in
        temp_37 ←
         (poly1305_encode_block (b_32)) ;;
@@ -363,41 +304,30 @@ Program Definition poly1305_update_block_state
           field_element_t '×
           field_element_t '×
           poly_key_t
-        )) ( ((((temp_37) +% (acc_34)) *% (r_35), r_35, k_36))) } : code (
+        )) ( ((((temp_37) +% (acc_34)) *% (r_35), r_35, k_36
+        ))) ; prog_valid := ltac:(ssprove_valid'_2) |}: code (
         fset.fset0) [interface] _)).
 Fail Next Obligation.
 
 Program Definition poly1305_update_block
   (b_32 : poly_block_t)
   (st_33 : poly_state_t)
-  : both (fset.fset0) poly_state_t :=
+  : both (fset.fset0) [interface] poly_state_t :=
   {|
-  is_pure := poly1305_update_block_pure(b_32 : poly_block_t)
+  is_pure := poly1305_update_block_pure (b_32 : poly_block_t)
   (st_33 : poly_state_t);
-  is_state := poly1305_update_block_state(b_32 : poly_block_t)
+  is_state := poly1305_update_block_state (b_32 : poly_block_t)
   (st_33 : poly_state_t);
   |}.
 Next Obligation.
+intros.
 unfold poly1305_update_block_pure.
 unfold poly1305_update_block_state.
-unfold is_pure.
-unfold is_state.
 
 unfold prog.
-
-both_bind.
-
 step_code.
-intros ; subst.
-reflexivity.
-
-intros.
-step_code.
-intros ? ? [] ; subst.
-split ; easy.
 Qed.
 
-Import Hacspec_Lib_Pre.
 Definition poly1305_update_blocks_pure
   (m_40 : byte_seq)
   (st_41 : poly_state_t)
@@ -407,7 +337,7 @@ Definition poly1305_update_blocks_pure
   let n_blocks_42 : uint_size :=
     (seq_len (m_40)) ./ (blocksize_v) in 
   let st_38 :=
-    foldi (usize 0) (n_blocks_42) (fun i_43 st_38 =>
+    Hacspec_Lib_Pre.foldi (usize 0) (n_blocks_42) (fun i_43 st_38 =>
       let block_44 : poly_block_t :=
         array_from_seq (16) (seq_get_exact_chunk (m_40) (blocksize_v) (
             i_43)) in 
@@ -423,14 +353,13 @@ Definition poly1305_update_blocks_pure_code
   {code pkg_core_definition.ret (T_ct (poly1305_update_blocks_pure m_40
     st_41))}.
 
-Import Hacspec_Lib.
 Definition st_38_loc : Location :=
   ((field_element_t '× field_element_t '× poly_key_t) : choice_type ; 49%nat).
 Program Definition poly1305_update_blocks_state
   (m_40 : byte_seq)
   (st_41 : poly_state_t)
-  : code (fset (path.sort leb [ st_38_loc])) [interface] (@ct (poly_state_t)) :=
-  (({code #put st_38_loc := 
+  : code (fset ([ st_38_loc])) [interface] (@ct (poly_state_t)) :=
+  (({| prog := #put st_38_loc := 
         (st_41) ;;
       st_38 ← get st_38_loc ;;
       let st_38 : (field_element_t '× field_element_t '× poly_key_t) :=
@@ -439,572 +368,63 @@ Program Definition poly1305_update_blocks_state
         (seq_len (m_40)) ;;
       let n_blocks_42 : uint_size :=
         ((temp_45) ./ (blocksize_v)) in
-      for_loop_usize (usize 0) (n_blocks_42) (fun i_43 =>
-        ({code  temp_46 ←
-            (seq_get_exact_chunk (m_40) (blocksize_v) (i_43)) ;;
-           temp_47 ←
-            (array_from_seq (16) (temp_46 : seq int8)) ;;
-          let block_44 : poly_block_t :=
-            (temp_47) in
-           temp_48 ←
-            (poly1305_update_block (block_44) (st_38)) ;;
-          st_38 ← get st_38_loc ;;
-          
-          #put st_38_loc := 
-            (temp_48) ;;
-          st_38 ← get st_38_loc ;;
-          
-          @pkg_core_definition.ret (unit_ChoiceEquality) ( (tt)) } : code (
-            fset (path.sort leb [ st_38_loc])) [interface] _)) ;;
+       st_38 ←
+        (foldi (usize 0) (n_blocks_42) (fun i_43 (st_38 : _) =>
+            ({| prog :=  temp_46 ←
+                (seq_get_exact_chunk (m_40) (blocksize_v) (i_43)) ;;
+               temp_47 ←
+                (array_from_seq (16) (temp_46 : seq int8)) ;;
+              let block_44 : poly_block_t :=
+                (temp_47) in
+               temp_48 ←
+                (poly1305_update_block (block_44) (st_38)) ;;
+              #put st_38_loc := 
+                (temp_48) ;;
+              st_38 ← get st_38_loc ;;
+              
+              @pkg_core_definition.ret (_) ( ((st_38
+                ))) ; prog_valid := ltac:(ssprove_valid'_2) |}: code (fset (
+                  [ st_38_loc])) [interface] _)) st_38) ;;
+      
       @pkg_core_definition.ret ((
           field_element_t '×
           field_element_t '×
           poly_key_t
-        )) ( (st_38)) } : code (fset (
-                                    path.sort leb [ st_38_loc])) [interface] _)).
+        )) ( (st_38)) ; prog_valid := ltac:(ssprove_valid'_2) |}: code (fset (
+          [ st_38_loc])) [interface] _)).
 Fail Next Obligation.
 
 Program Definition poly1305_update_blocks
   (m_40 : byte_seq)
   (st_41 : poly_state_t)
-  : both (fset (path.sort leb [ st_38_loc])) poly_state_t :=
+  : both (fset ([ st_38_loc])) [interface] poly_state_t :=
   {|
-  is_pure := poly1305_update_blocks_pure(m_40 : byte_seq)
+  is_pure := poly1305_update_blocks_pure (m_40 : byte_seq)
   (st_41 : poly_state_t);
-  is_state := poly1305_update_blocks_state(m_40 : byte_seq)
+  is_state := poly1305_update_blocks_state (m_40 : byte_seq)
   (st_41 : poly_state_t);
   |}.
 Next Obligation.
+intros.
 unfold poly1305_update_blocks_pure.
 unfold poly1305_update_blocks_state.
-unfold is_pure.
-unfold is_state.
 
 unfold prog.
-
-unfold seq_len.
-unfold lift_to_code.
 
 step_code.
 
+apply foldi_as_both.
+set (hi := (a ./ blocksize_v)).
+destruct_uint_size_as_nat hi.
+- reflexivity.
+- rewrite H2.  
+  apply Nat2Z.is_nonneg.
 
-enough (unsigned (usize 0%nat) <=
-          unsigned (Hacspec_Lib_Pre.seq_len m_40 ./ blocksize_v))%Z.
-
-unfold for_loop_usize.
-replace (from_uint_size (usize 0)) with 0 by reflexivity.
-
-set (f := fun n : nat => _).
-set (k := (_ , _)).
-pose (foldi_nat_is_loop 0 (from_uint_size (Hacspec_Lib_Pre.seq_len m_40 ./ blocksize_v)) (fun (_ : poly_state_t) => f) k).
-hnf in e.
-
-Set Printing Coercions.
-
-set (tct := T_ct _) in *.
-replace tct with k in e by reflexivity. 
-remove_T_ct.
-rewrite e.
-  
-pose @Build_both.
-epose (fun x y => @Build_both _ _ (d x y) (c x)) .
-
-
-both_bind.
-
-unfold c at 1.
-
-unfold poly1305_update_block.
-unfold poly1305_update_block_state.
-unfold poly1305_update_block_pure.
-destruct st_41 as [[]].
-
-unfold poly1305_encode_block.
-unfold is_pure.
-unfold is_state.
-unfold poly1305_encode_block_state.
-unfold poly1305_encode_block_pure.
-
-unfold prog.
-unfold seq_get_exact_chunk.
-unfold array_from_seq.
-unfold array_to_seq.
-unfold uint128_from_le_bytes.
-unfold nat_mod_from_secret_literal.
-unfold nat_mod_pow2.
-
-unfold lift_to_code.
+intros.
 
 step_code.
+Qed.
 
-
-
-apply r_restore_lhs.
-intros.
-subst.
-
-apply r_get_remember_lhs. intros.
-apply r_put_lhs.
-apply r_get_remember_lhs. intros.
-fold (@bind 'unit).
-step_code.
-
-
-set (lo := S (from_uint_size _)).
-set (hi := (from_uint_size (_ ./ _))).
-set (f := fun _ _ => _ ).
-set (v := (@pair (@T (prod_ChoiceEquality field_element_t field_element_t))
-                (@T poly_key_t) (@pair (@T field_element_t) (@T field_element_t) t t0) t1) : poly_state_t).
-
-replace (foldi_nat lo hi f tt ;; ret _) with (foldi_nat lo hi (fun (x : nat) (a : poly_state_t) => f x tt ;; ret a) v) by apply (@foldi_nat_consume_ret (prod_ChoiceEquality _ _) lo hi f v).
-
-(* replace (S (from_uint_size (usize 0))) with (from_uint_size (usize (S 0))) in lo. *)
-pose (foldi_to_foldi_nat (usize (S 0)) (Hacspec_Lib_Pre.seq_len m_40 ./ blocksize_v)).
-
-rewrite foldi_nat_to_foldi.
-
-epose (@foldi
-       (prod_ChoiceEquality (prod_ChoiceEquality field_element_t field_element_t)
-                            poly_key_t) (@usize nat nat_uint_sizable lo) (@usize nat nat_uint_sizable hi)
-       _ _
-       (fun (x1 : @T uint_size)
-          (a : @T
-                 (prod_ChoiceEquality
-                    (prod_ChoiceEquality field_element_t field_element_t) poly_key_t)) =>
-        {code (@bind (chElement (@ct unit_ChoiceEquality))
-          (chElement
-             (@ct
-                (prod_ChoiceEquality (prod_ChoiceEquality field_element_t field_element_t)
-                   poly_key_t))) (f (@from_uint_size nat nat_uint_sizable x1) tt)
-          (fun _ : choice.Choice.sort (chElement (@ct unit_ChoiceEquality)) =>
-           @ret
-             (chElement
-                (@ct
-                   (prod_ChoiceEquality
-                      (prod_ChoiceEquality field_element_t field_element_t) poly_key_t)))
-             (@T_ct
-                (prod_ChoiceEquality (prod_ChoiceEquality field_element_t field_element_t)
-                                     poly_key_t) a)))}) v).
-
-replace (@foldi_pre
-       (prod_ChoiceEquality (prod_ChoiceEquality field_element_t field_element_t)
-          poly_key_t) (@usize nat nat_uint_sizable lo) (@usize nat nat_uint_sizable hi)
-       (fun (x1 : @T uint_size)
-          (a : @T
-                 (prod_ChoiceEquality
-                    (prod_ChoiceEquality field_element_t field_element_t) poly_key_t)) =>
-        @bind (chElement (@ct unit_ChoiceEquality))
-          (chElement
-             (@ct
-                (prod_ChoiceEquality (prod_ChoiceEquality field_element_t field_element_t)
-                   poly_key_t))) (f (@from_uint_size nat nat_uint_sizable x1) tt)
-          (fun _ : choice.Choice.sort (chElement (@ct unit_ChoiceEquality)) =>
-           @ret
-             (chElement
-                (@ct
-                   (prod_ChoiceEquality
-                      (prod_ChoiceEquality field_element_t field_element_t) poly_key_t)))
-             (@T_ct
-                (prod_ChoiceEquality (prod_ChoiceEquality field_element_t field_element_t)
-                   poly_key_t) a))) v) with (prog c0).
-unfold c0.
-
-unfold prog.
-(* eapply rpre_weaken_rule. *)
-
-set (f_state := (fun (x1 : block_index_t) (a : poly_state_t) =>
-        {code f (from_uint_size x1) tt ;;
-        ret a })).
-
-set (f_pure := (fun (i_43 : block_index_t) => _)).
-
-unfold hi in *. clear hi. set (hi := (Hacspec_Lib_Pre.seq_len m_40 ./ blocksize_v)).
-unfold lo in *. clear lo.
-unfold nat_uint_sizable.
-unfold usize at 3.
-unfold from_uint_size at 3.
-
-set (lo := usize 0%Z).
-set (P := _ ⋊ _).
-assert (forall x , P (x , x)).
-clear.
-intros.
-unfold P.
-unfold set_lhs.
-hnf.
-esplit.
-exists (set_heap x1 st_38_loc v).
-split.
-hnf.
-split.
-exists x1.
-split.
-reflexivity.
-reflexivity.
-
-hnf.
-rewrite get_set_heap_eq.
-
-exists x1.
-cbn.
-
-pose (@foldi_both _ _ lo (hi) f_state f_pure v H P).
-
-Set Printing Coercions.
-
-pose @r_transR.
-specialize r0 with (P := P).
-              (set_lhs st_38_loc v (fun '(h₀, h₁) => h₀ = h₁) ⋊ rem_lhs st_38_loc x)). 
-                                                                                  (c₁' := ret (Hacspec_Lib_Pre.foldi lo hi f_pure v)).
-
-(((T_ct
-              (Hacspec_Lib_Pre.nat_mod_from_secret_literal
-                 (T_ct
-                    (Hacspec_Lib_Pre.uint128_from_le_bytes
-                       (T_ct
-                          (Hacspec_Lib_Pre.array_from_seq 16
-                             (T_ct
-                                (Hacspec_Lib_Pre.array_to_seq
-                                   (T_ct
-                                      (Hacspec_Lib_Pre.array_from_seq 16
-                                         (T_ct
-                                            (Hacspec_Lib_Pre.seq_get_exact_chunk m_40
-                                               blocksize_v
-                                               (usize (from_uint_size (repr (Z.of_nat 0))))))))))))))) +%
-            T_ct
-              (Hacspec_Lib_Pre.nat_mod_pow2 1361129467683753853853498429727072845819
-                 (N.of_nat (uint_size_to_nat (Z_to_uint_size (toword (usize 128))))))) +%
-           t) *% t0, t0, t1)
-
-  eapply r_transR.
-apply r.
-assumption.
-intros.
-unfold f_state.
-unfold f_pure.
-unfold prog.
-unfold f.
-unfold c.
-
-
-unfold poly1305_update_block.
-unfold poly1305_update_block_state.
-unfold poly1305_update_block_pure.
-(* destruct st_41 as [[]]. *)
-
-unfold poly1305_encode_block.
-unfold is_pure.
-unfold is_state.
-unfold poly1305_encode_block_state.
-unfold poly1305_encode_block_pure.
-
-unfold prog.
-unfold seq_get_exact_chunk.
-unfold array_from_seq.
-unfold array_to_seq.
-unfold uint128_from_le_bytes.
-unfold nat_mod_from_secret_literal.
-unfold nat_mod_pow2.
-
-unfold lift_to_code.
-
-step_code.
-
-
-
-
-unfold lo.
-unfold hi.
-unfold nat_uint_sizable.
-unfold from_uint_size.
-unfold usize.
-
-
-
-
-
-rewrite  Z2Nat.id.
-rewrite Nat2Z.id.
-
-eapply r.
-
-Print foldi.
-rewrite <- foldi_to_foldi_nat.
-
-apply foldi_both.
-
-
-  
-
-Set Printing All.
-
-rewrite <- e.
-rewrite <- foldi_nat_consume_ret.
-
-
-
-
-(@bind (chElement chUnit)
-       (chElement
-          (@ct
-             (prod_ChoiceEquality (prod_ChoiceEquality field_element_t field_element_t)
-                poly_key_t))) (@foldi_nat unit_ChoiceEquality lo hi f tt)
-       (fun _ : choice.Choice.sort (chElement chUnit) =>
-        @ret
-          (chElement
-             (@ct
-                (prod_ChoiceEquality (prod_ChoiceEquality field_element_t field_element_t)
-                   poly_key_t)))
-          (@pair (@T (prod_ChoiceEquality field_element_t field_element_t))
-                 (@T poly_key_t) t2 t3)))
-
-(@bind (chElement chUnit)
-          (chElement
-             (@ct
-                (prod_ChoiceEquality (prod_ChoiceEquality field_element_t field_element_t)
-                   poly_key_t))) (@foldi_nat unit_ChoiceEquality lo hi f tt)
-          (fun _ : choice.Choice.sort (chElement (@ct unit_ChoiceEquality)) =>
-           @ret
-             (chElement
-                (@ct
-                   (prod_ChoiceEquality
-                      (prod_ChoiceEquality field_element_t field_element_t) poly_key_t)))
-             (@T_ct
-                (prod_ChoiceEquality (prod_ChoiceEquality field_element_t field_element_t)
-                   poly_key_t)
-                (@pair (@T (prod_ChoiceEquality field_element_t field_element_t))
-                   (@T poly_key_t) t2 t3))))
-
-set (v := (t, t0, t1) ).
-
-
-rewrite <- foldi_nat_consume_ret.
-
-
-apply rreflexivity_rule.
-
-reflexivity.
-
-
-fold bind.
-
-Check r_get_remind_lhs.
-apply r_get_remind_lhs.
-
-apply r_restore_lhs.
-intros. subst.  admit. 
-
-
-rewrite <- bind_assoc.
-unfold bind at 1.
-
-
-
-replace (S
-          (from_uint_size (Hacspec_Lib_Pre.seq_len m_40 ./ blocksize_v) -
-             from_uint_size (usize 0) - 1)) with
-  (S (from_uint_size ((Hacspec_Lib_Pre.seq_len m_40 ./ blocksize_v) .- repr 1) -
-      from_uint_size (usize 0))).
-
-pose (foldi_nat (usize 0) ((Hacspec_Lib_Pre.seq_len m_40 ./ blocksize_v) - 1)).
-remember r.
-
-inversion Heqr0.
-unfold r in Heqr0.
-unfold foldi_nat in r.
-destruct ((Hacspec_Lib_Pre.seq_len m_40 ./ blocksize_v) - 1 - usize 0) eqn:ro in r.
-
-
-replace 
-
-
-
-fold foldi_nat.
-
-rewrite <- foldi__nat_move_S_append.
-unfold c.
-unfold prog.
-unfold seq_get_exact_chunk.
-unfold array_from_seq.
-
-rewrite forc;
-
-
-
-
-eapply (r_transL
-          (foldi_nat_
-       (S
-          (from_uint_size (Hacspec_Lib_Pre.seq_len m_40 ./ blocksize_v) -
-           from_uint_size (usize 0) - 1)) 0
-       (fun (x : nat) (_ : unit_ChoiceEquality) =>
-        c (usize (x + from_uint_size (usize 0)))) tt ;; ret st_41)) .
-eapply r_bind.
-apply rsymmetry.
-apply rsym_pre. intros ; subst ; reflexivity.
-eapply rpost_weaken_rule.
-rewrite for_loop_equality.
-reflexivity.
-
-
-apply for_loop_equality. apply H.
-intros. subst. destruct a₁. reflexivity.
-intros. apply r_ret. intros. inversion H0. subst. reflexivity.
-Set Printing Coercions.
-
-eapply (r_transL
-          (lift_to_code (Hacspec_Lib_Pre.foldi (usize 0) (Hacspec_Lib_Pre.seq_len m_40 ./ blocksize_v) (fun i_43 st_38 : T =>
-              let (is_pure, _) :=
-                poly1305_update_block
-                  (Hacspec_Lib_Pre.array_from_seq 16
-                     (Hacspec_Lib_Pre.seq_get_exact_chunk m_40 blocksize_v i_43)) st_38 in
-              is_pure) _) ;; ret st_41)).
-eapply r_bind.
-apply rsymmetry.
-apply rsym_pre. intros ; subst ; reflexivity.
-eapply rpost_weaken_rule.
-pose @foldi_both.
-apply foldi_both.
-intros [h₀  h₁]. apply (h₀ = h₁).
-apply H.
-intros.
-
-
-
-
-
-(* unfold prog. *)
-(* unfold foldi. *)
-
-(* assert (forall lo hi {L I} f v (H : (unsigned lo <= unsigned hi)%Z), *)
-(*            (foldi lo hi (fun x _ => f x) tt ;; ret v) = *)
-(*            (foldi lo hi (L := L) (I := I) (fun x v => {code f x ;; ret v}) (ct_T v)) *)
-(*        ). *)
-(* clear. *)
-(* intros. *)
-(* unfold prog. *)
-(* unfold foldi. *)
-(* rewrite foldi_to_foldi_nat by apply H. *)
-(* rewrite foldi_to_foldi_nat by apply H. *)
-(* unfold prog. *)
-(* unfold foldi_nat. *)
-(* destruct (Z.to_nat (unsigned hi) - Z.to_nat (unsigned lo)) ; [ reflexivity | .. ]. *)
-(* rewrite <- foldi__nat_move_S. *)
-(* rewrite <- foldi__nat_move_S. *)
-(* f_equal. *)
-(* induction n. *)
-(* - cbn. *)
-(*   rewrite bind_ret. *)
-
-apply 
-
-unfold prog.
-unfold foldi.
-rewrite foldi_to_foldi_nat.
-
-  
-
-pose (foldi_both (usize 0) (Hacspec_Lib_Pre.seq_len m_40 ./ blocksize_v) (fun (x : block_index_t) (_ : unit_ChoiceEquality) => c x)).
-
-apply H.
-
-unfold nat_uint_sizable in r.
-unfold usize in r.
-rewrite unsigned_repr_alt in r.
-
-
-
-
-specialize r with ()
-apply r.
-
-unfold for_loop_usize.
-unfold for_loop_range.
-
-unfold prog.
-
-unfold poly1305_update_block.
-unfold poly1305_update_block_pure.
-unfold poly1305_update_block_state.
-unfold is_pure.
-unfold is_state.
-destruct st_41 as [[]].
-
-unfold poly1305_encode_block.
-unfold poly1305_encode_block_pure.
-unfold poly1305_encode_block_state.
-unfold is_pure.
-unfold is_state.
-unfold prog.
-
-unfold seq_get_exact_chunk.
-unfold array_from_seq.
-
-unfold array_to_seq.
-unfold array_from_seq.
-unfold uint128_from_le_bytes.
-unfold nat_mod_from_secret_literal.
-unfold nat_mod_pow2.
-
-unfold lift_to_code.
-
-
-unfold from_uint_size.
-unfold nat_uint_sizable.
-unfold usize.
-Set Printing Coercions.
-
-rewrite unsigned_repr_alt.
-rewrite Nat2Z.id.
-rewrite Nat.sub_0_r.
-
-unfold for_loop.
-destruct (Z.to_nat (unsigned (T_ct (Hacspec_Lib_Pre.seq_len m_40) ./ blocksize_v))).
-
-
-
-
-
-repeat rewrite unsigned_repr_alt.
-
-
-rewrite unsigned_repr.
-
-apply (for_loop_rule (fun i => fun '(s₀, s₁) => set_lhs st_38_loc st_41 (fun '(h₀, h₁) => h₀ = h₁) (s₀, s₁))).
-
-unfold poly1305_update_block.
-unfold poly1305_update_block_pure.
-unfold poly1305_update_block_state.
-unfold is_pure.
-unfold is_state.
-
-unfold prog.
-
-destruct st_38 as [[]].
-
-unfold poly1305_encode_block.
-unfold poly1305_encode_block_pure.
-unfold poly1305_encode_block_state.
-unfold is_pure.
-unfold is_state.
-unfold prog.
-
-unfold seq_get_exact_chunk.
-unfold array_from_seq.
-
-
-
-unfold array_to_seq.
-  unfold array_from_seq.
-  unfold uint128_from_le_bytes.
-  unfold nat_mod_from_secret_literal.
-  unfold nat_mod_pow2.
-
-  unfold lift_to_code.
-
-Admitted.
-
-Import Hacspec_Lib_Pre.
 Definition poly1305_update_last_pure
   (pad_len_52 : uint_size)
   (b_53 : sub_block_t)
@@ -1013,7 +433,7 @@ Definition poly1305_update_last_pure
   let st_50 : (field_element_t '× field_element_t '× poly_key_t) :=
     st_54 in 
   let '(st_50) :=
-    if (seq_len (b_53)) !=.? (usize 0):bool then (let '(acc_55, r_56, k_57) :=
+    if (seq_len (b_53) : T) !=.? (usize 0):bool then (let '(acc_55, r_56, k_57) :=
         st_50 in 
       let st_50 :=
         (
@@ -1032,15 +452,14 @@ Definition poly1305_update_last_pure_code
     b_53
     st_54))}.
 
-Import Hacspec_Lib.
 Definition st_50_loc : Location :=
   ((field_element_t '× field_element_t '× poly_key_t) : choice_type ; 60%nat).
 Program Definition poly1305_update_last_state
   (pad_len_52 : uint_size)
   (b_53 : sub_block_t)
   (st_54 : poly_state_t)
-  : code (fset (path.sort leb [ st_50_loc])) [interface] (@ct (poly_state_t)) :=
-  (({code #put st_50_loc := 
+  : code (fset ([ st_50_loc])) [interface] (@ct (poly_state_t)) :=
+  (({| prog := #put st_50_loc := 
         (st_54) ;;
       st_50 ← get st_50_loc ;;
       let st_50 : (field_element_t '× field_element_t '× poly_key_t) :=
@@ -1048,68 +467,54 @@ Program Definition poly1305_update_last_state
        temp_58 ←
         (seq_len (b_53)) ;;
        '(st_50) ←
-        (if (temp_58) !=.? (usize 0):bool_ChoiceEquality then (({code let '(
-                  acc_55,
-                  r_56,
-                  k_57
-                ) :=
+        (if (temp_58) !=.? (usize 0):bool_ChoiceEquality then ((
+              {| prog := let '(acc_55, r_56, k_57) :=
                 (st_50) : (field_element_t '× field_element_t '× poly_key_t
               ) in
                temp_59 ←
                 (poly1305_encode_last (pad_len_52) (b_53)) ;;
-              st_50 ← get st_50_loc ;;
-              
               #put st_50_loc := 
                 ((((temp_59) +% (acc_55)) *% (r_56), r_56, k_57)) ;;
               st_50 ← get st_50_loc ;;
               
-              @pkg_core_definition.ret (_) ( ((st_50))) } : code (fset (
-                  path.sort leb [ st_50_loc])) [interface] _)) else (
+              @pkg_core_definition.ret (_) ( ((st_50
+                ))) ; prog_valid := ltac:(ssprove_valid'_2) |}: code (fset (
+                  [ st_50_loc])) [interface] _)) else (
             @pkg_core_definition.ret (_) ( ((st_50))))) ;;
       
       @pkg_core_definition.ret ((
           field_element_t '×
           field_element_t '×
           poly_key_t
-        )) ( (st_50)) } : code (fset (
-          path.sort leb [ st_50_loc])) [interface] _)).
+        )) ( (st_50)) ; prog_valid := ltac:(ssprove_valid'_2) |}: code (fset (
+          [ st_50_loc])) [interface] _)).
 Fail Next Obligation.
 
-Definition poly1305_update_last
+Program Definition poly1305_update_last
   (pad_len_52 : uint_size)
   (b_53 : sub_block_t)
   (st_54 : poly_state_t)
-  : both (fset (path.sort leb [ st_50_loc])) poly_state_t :=
+  : both (fset ([ st_50_loc])) [interface] poly_state_t :=
   {|
-  is_pure := poly1305_update_last_pure(pad_len_52 : uint_size)
+  is_pure := poly1305_update_last_pure (pad_len_52 : uint_size)
   (b_53 : sub_block_t)
   (st_54 : poly_state_t);
-  is_state := poly1305_update_last_state(pad_len_52 : uint_size)
+  is_state := poly1305_update_last_state (pad_len_52 : uint_size)
   (b_53 : sub_block_t)
   (st_54 : poly_state_t);
   |}.
-
-Instance poly1305_update_last_eq :
-forall (pad_len_52 : uint_size)
-(b_53 : sub_block_t)
-(st_54 : poly_state_t),
-CodeEqProofStatement (poly1305_update_last(pad_len_52 : uint_size)
-  (b_53 : sub_block_t)
-  (st_54 : poly_state_t)).
-Proof.
+Next Obligation.
 intros.
-unfold CodeEqProofStatement.
-
-unfold poly1305_update_last.
 unfold poly1305_update_last_pure.
 unfold poly1305_update_last_state.
-unfold is_pure.
-unfold is_state.
 
 unfold prog.
-Admitted.
+step_code.
+destruct negb.
+- step_code.
+- step_code.
+Qed.
 
-Import Hacspec_Lib_Pre.
 Definition poly1305_update_pure
   (m_61 : byte_seq)
   (st_62 : poly_state_t)
@@ -1125,14 +530,12 @@ Definition poly1305_update_pure_code
   : code fset.fset0 [interface] (@ct poly_state_t) :=
   {code pkg_core_definition.ret (T_ct (poly1305_update_pure m_61 st_62))}.
 
-Import Hacspec_Lib.
 
 Program Definition poly1305_update_state
   (m_61 : byte_seq)
   (st_62 : poly_state_t)
-  : code (fset (path.sort leb [ st_38_loc ; st_50_loc])) [interface] (@ct (
-      poly_state_t)) :=
-  (({code  temp_65 ←
+  : code (fset ([ st_50_loc ; st_38_loc])) [interface] (@ct (poly_state_t)) :=
+  (({| prog :=  temp_65 ←
         (poly1305_update_blocks (m_61) (st_62)) ;;
       let st_63 : (field_element_t '× field_element_t '× poly_key_t) :=
         (temp_65) in
@@ -1144,39 +547,30 @@ Program Definition poly1305_update_state
         (seq_len (last_64)) ;;
        temp_68 ←
         (poly1305_update_last (temp_67) (last_64) (st_63)) ;;
-      @pkg_core_definition.ret (poly_state_t) ( (temp_68)) } : code (fset (
-          path.sort leb [ st_38_loc ; st_50_loc])) [interface] _)).
+      @pkg_core_definition.ret (poly_state_t) ( (
+        temp_68)) ; prog_valid := ltac:(ssprove_valid'_2) |}: code (fset (
+          [ st_50_loc ; st_38_loc])) [interface] _)).
 Fail Next Obligation.
 
-Definition poly1305_update
+Program Definition poly1305_update
   (m_61 : byte_seq)
   (st_62 : poly_state_t)
-  : both (fset (path.sort leb [ st_38_loc ; st_50_loc])) poly_state_t :=
+  : both (fset ([ st_50_loc ; st_38_loc])) [interface] poly_state_t :=
   {|
-  is_pure := poly1305_update_pure(m_61 : byte_seq)
+  is_pure := poly1305_update_pure (m_61 : byte_seq)
   (st_62 : poly_state_t);
-  is_state := poly1305_update_state(m_61 : byte_seq)
+  is_state := poly1305_update_state (m_61 : byte_seq)
   (st_62 : poly_state_t);
   |}.
-
-Instance poly1305_update_eq :
-forall (m_61 : byte_seq)
-(st_62 : poly_state_t),
-CodeEqProofStatement (poly1305_update(m_61 : byte_seq) (st_62 : poly_state_t)).
-Proof.
+Next Obligation.
 intros.
-unfold CodeEqProofStatement.
-
-unfold poly1305_update.
 unfold poly1305_update_pure.
 unfold poly1305_update_state.
-unfold is_pure.
-unfold is_state.
 
 unfold prog.
-Admitted.
+step_code.
+Qed.
 
-Import Hacspec_Lib_Pre.
 Definition poly1305_finish_pure (st_69 : poly_state_t) : poly1305_tag_t :=
   let '(acc_70, _, k_71) :=
     st_69 in 
@@ -1188,18 +582,17 @@ Definition poly1305_finish_pure (st_69 : poly_state_t) : poly1305_tag_t :=
   let a_74 : uint128 :=
     uint128_from_le_bytes (array_from_slice (default) (16) (aby_73) (usize 0) (
         usize 16)) in 
-  array_from_seq (16) (array_to_seq (uint128_to_le_bytes ((a_74) .+ (n_72)))).
+  array_from_seq (16) (array_to_seq (uint128_to_le_bytes ((a_74) .+ (n_72)) : nseq _ _)).
 Definition poly1305_finish_pure_code
   (st_69 : poly_state_t)
   : code fset.fset0 [interface] (@ct poly1305_tag_t) :=
   {code pkg_core_definition.ret (T_ct (poly1305_finish_pure st_69))}.
 
-Import Hacspec_Lib.
 
 Program Definition poly1305_finish_state
   (st_69 : poly_state_t)
   : code (fset.fset0) [interface] (@ct (poly1305_tag_t)) :=
-  (({code let '(acc_70, _, k_71) :=
+  (({| prog := let '(acc_70, _, k_71) :=
         (st_69) : (field_element_t '× field_element_t '× poly_key_t) in
        temp_75 ←
         (array_to_seq (k_71)) ;;
@@ -1224,40 +617,32 @@ Program Definition poly1305_finish_state
        temp_81 ←
         (uint128_to_le_bytes ((a_74) .+ (n_72))) ;;
        temp_82 ←
-        (array_to_seq (temp_81)) ;;
+        (array_to_seq (temp_81 : nseq int8 16 )) ;;
       let temp_82 : seq uint8 :=
         (temp_82) in
        temp_83 ←
         (array_from_seq (16) (temp_82)) ;;
-      @pkg_core_definition.ret (poly1305_tag_t) ( (temp_83)) } : code (
+      @pkg_core_definition.ret (poly1305_tag_t) ( (
+        temp_83)) ; prog_valid := ltac:(ssprove_valid'_2) |}: code (
         fset.fset0) [interface] _)).
 Fail Next Obligation.
 
-Definition poly1305_finish
+Program Definition poly1305_finish
   (st_69 : poly_state_t)
-  : both (fset.fset0) poly1305_tag_t :=
+  : both (fset.fset0) [interface] poly1305_tag_t :=
   {|
-  is_pure := poly1305_finish_pure(st_69 : poly_state_t);
-  is_state := poly1305_finish_state(st_69 : poly_state_t);
+  is_pure := poly1305_finish_pure (st_69 : poly_state_t);
+  is_state := poly1305_finish_state (st_69 : poly_state_t);
   |}.
-
-Instance poly1305_finish_eq :
-forall (st_69 : poly_state_t),
-CodeEqProofStatement (poly1305_finish(st_69 : poly_state_t)).
-Proof.
+Next Obligation.
 intros.
-unfold CodeEqProofStatement.
-
-unfold poly1305_finish.
 unfold poly1305_finish_pure.
 unfold poly1305_finish_state.
-unfold is_pure.
-unfold is_state.
 
 unfold prog.
-Admitted.
+step_code.
+Qed.
 
-Import Hacspec_Lib_Pre.
 Definition poly1305_pure
   (m_86 : byte_seq)
   (key_87 : poly_key_t)
@@ -1273,16 +658,14 @@ Definition poly1305_pure_code
   : code fset.fset0 [interface] (@ct poly1305_tag_t) :=
   {code pkg_core_definition.ret (T_ct (poly1305_pure m_86 key_87))}.
 
-Import Hacspec_Lib.
 Definition st_84_loc : Location :=
   ((field_element_t '× field_element_t '× poly_key_t) : choice_type ; 91%nat).
 Program Definition poly1305_state
   (m_86 : byte_seq)
   (key_87 : poly_key_t)
-  : code (fset (
-      path.sort leb [ st_50_loc ; n_0_loc ; st_84_loc ; st_38_loc])) [interface] (
+  : code (fset ([ st_50_loc ; n_0_loc ; st_84_loc ; st_38_loc])) [interface] (
     @ct (poly1305_tag_t)) :=
-  (({code  temp_88 ←
+  (({| prog :=  temp_88 ←
         (poly1305_init (key_87)) ;;
       #put st_84_loc := 
         (temp_88) ;;
@@ -1291,44 +674,34 @@ Program Definition poly1305_state
         (st_84) in
        temp_89 ←
         (poly1305_update (m_86) (st_84)) ;;
-      st_84 ← get st_84_loc ;;
-      
       #put st_84_loc := 
         (temp_89) ;;
       st_84 ← get st_84_loc ;;
       
        temp_90 ←
         (poly1305_finish (st_84)) ;;
-      @pkg_core_definition.ret (poly1305_tag_t) ( (temp_90)) } : code (fset (
-          path.sort leb [ st_50_loc ; n_0_loc ; st_84_loc ; st_38_loc])) [interface] _)).
+      @pkg_core_definition.ret (poly1305_tag_t) ( (
+        temp_90)) ; prog_valid := ltac:(ssprove_valid'_2) |}: code (fset (
+          [ st_50_loc ; n_0_loc ; st_84_loc ; st_38_loc])) [interface] _)).
 Fail Next Obligation.
 
-Definition poly1305
+Program Definition poly1305
   (m_86 : byte_seq)
   (key_87 : poly_key_t)
   : both (fset (
-      path.sort leb [ st_50_loc ; n_0_loc ; st_84_loc ; st_38_loc])) poly1305_tag_t :=
+      [ st_50_loc ; n_0_loc ; st_84_loc ; st_38_loc])) [interface] poly1305_tag_t :=
   {|
-  is_pure := poly1305_pure(m_86 : byte_seq)
+  is_pure := poly1305_pure (m_86 : byte_seq)
   (key_87 : poly_key_t);
-  is_state := poly1305_state(m_86 : byte_seq)
+  is_state := poly1305_state (m_86 : byte_seq)
   (key_87 : poly_key_t);
   |}.
-
-Instance poly1305_eq :
-forall (m_86 : byte_seq)
-(key_87 : poly_key_t),
-CodeEqProofStatement (poly1305(m_86 : byte_seq) (key_87 : poly_key_t)).
-Proof.
+Next Obligation.
 intros.
-unfold CodeEqProofStatement.
-
-unfold poly1305.
 unfold poly1305_pure.
 unfold poly1305_state.
-unfold is_pure.
-unfold is_state.
 
 unfold prog.
-Admitted.
+step_code.
+Qed.
 
