coq_ssprove/src/LocationUtility.v
@@ -1,0 +1,597 @@
+From Coq Require Import ZArith List.
+From Crypt Require Import choice_type Package.
+Import PackageNotation.
+From Crypt Require Import pkg_interpreter.
+From extructures Require Import ord fset fmap.
+Require Import Hacspec_Lib_Comparable.
+
+Require Import Coq.Logic.FunctionalExtensionality.
+
+(*** Location *)
+
+(* Fixpoint Inb {A : Type} `{EqDec A} (a:A) (l:list A) : bool := *)
+(*   match l with *)
+(*   | nil => false *)
+(*   | cons b m => (eqb b a) || Inb a m *)
+(*   end. *)
+
+Definition loc_eqType :=
+  (@eqtype.tag_eqType choice_type_eqType (fun _ : choice_type => ssrnat.nat_eqType)).
+
+Definition location_eqb (ℓ ℓ' : Location) :=
+  andb (@eqtype.eq_op ssrnat.nat_eqType (projT2 ℓ) (projT2 ℓ'))
+       (@eqtype.eq_op _ (projT1 ℓ) (projT1 ℓ')).
+       (* (@eqtype.eq_op loc_eqType ℓ ℓ'). *)
+
+(* Axiom location_is_types : (forall l1 l2 : Location , *)
+(*                               is_true (eqb (ssrfun.tagged l1) (ssrfun.tagged l2)) -> *)
+(*                               is_true (eqtype.eq_op (ssrfun.tag l1) (ssrfun.tag l2))). *)
+
+
+Definition location_eqbP : forall (l1 l2 : Location),
+    @location_eqb (l1) (l2)
+    = (@eqtype.eq_op
+         (@eqtype.tag_eqType choice_type_eqType
+                             (fun _ : choice_type => ssrnat.nat_eqType)) l1 l2).
+Proof.
+  intros.
+
+  unfold location_eqb.
+  unfold eqtype.eq_op.
+
+  cbn.
+  rewrite ssrnat.eqnE.
+  unfold eqtype.tag_eq.
+  unfold eqtype.tagged_as.
+  unfold ssrfun.tag.
+  unfold ssrfun.tagged.
+
+  rewrite Bool.andb_comm.
+  
+  unfold eq_rect_r, eq_rect.
+
+  set (eqtype.eq_op _ _) at 2.
+  replace (choice_type_eq _ _) with b by reflexivity.
+  
+  destruct b eqn:b_eq ; subst b.
+  - f_equal.
+    case eqtype.eqP ; intros.
+    + rewrite e in *.
+      unfold eq_sym.
+      reflexivity.
+    + exfalso.
+      apply (ssrbool.elimT eqtype.eqP) in b_eq.
+      apply n.
+      eapply b_eq.
+  - reflexivity.
+Qed.
+
+Theorem is_true_split_or : forall a b, is_true (a || b) = (is_true a \/ is_true b).
+Proof.
+  intros.
+  rewrite boolp.propeqE.
+  symmetry.
+  apply (ssrbool.rwP ssrbool.orP).
+Qed.  
+Theorem is_true_split_and : forall a b, is_true (a && b) = (is_true a /\ is_true b).
+Proof.
+  intros.
+  rewrite boolp.propeqE.
+  symmetry.
+  apply (ssrbool.rwP ssrbool.andP).
+Qed.  
+
+
+
+
+Theorem LocsSubset : (forall {A} (L1 L2 : list A) (a : A),
+                         List.incl L1 L2 ->
+                         List.In a L1 ->
+                         List.In a L2).
+  intros.
+  induction L1 as [ | a0 L ] ; cbn in *.
+  - contradiction.
+  - destruct (List.incl_cons_inv H).
+    destruct H0.
+    + subst.
+      assumption.
+    + apply IHL ; assumption.
+Qed.
+
+(* Theorem in_bool_iff : forall {A : Type} `{EqDec A} (a:A) (l:list A), is_true (Inb a l) <-> List.In a l. *)
+(*   induction l ; cbn. *)
+(*   - rewrite boolp.falseE. *)
+(*     reflexivity. *)
+(*   - cbn. *)
+(*     rewrite is_true_split_or.     *)
+(*     apply ZifyClasses.or_morph. *)
+(*     apply eqb_leibniz. *)
+(*     apply IHl. *)
+(* Qed. *)
+
+
+Lemma location_eqb_sound : forall ℓ ℓ' : Location, is_true (location_eqb ℓ ℓ') <-> ℓ = ℓ'.
+Proof.
+  intros.
+  rewrite location_eqbP.
+  (* unfold location_eqb. *)
+  (* Set Printing All. *)
+  pose (@eqtype.eqP loc_eqType).
+  unfold eqtype.Equality.axiom in a.
+  pose (ssrbool.elimT).
+  pose (@eqtype.tag_eqP ).
+
+  split.
+  
+  pose (Couplings.reflection_nonsense (@eqtype.tag_eqType choice_type_eqType (fun _ : choice_type => ssrnat.nat_eqType)) ℓ ℓ').
+
+  
+  (* rewrite is_true_split_and. *)
+  (* intros [_].   *)
+  apply e.  
+  (* apply H. *)
+  intros. subst.
+  (* rewrite eqb_refl. *)
+  apply eqtype.eq_refl.
+Qed.
+
+Global Program Instance location_eqdec: EqDec (Location) := {
+    eqb := location_eqb;
+    eqb_leibniz := location_eqb_sound;
+  }.
+
+Definition location_ltb : Location -> Location -> bool :=
+  (tag_leq (I:=choice_type_ordType) (T_:=fun _ : choice_type => nat_ordType)).
+
+Definition location_ltb_simple : Location -> Location -> bool :=
+  fun x y => ltb (projT2 x) (projT2 y).
+
+Global Instance location_comparable : Comparable (Location) :=
+  eq_dec_lt_Comparable location_ltb.
+
+Definition le_is_ord_leq : forall s s0 : nat_ordType,
+    eqtype.eq_op s s0 = false -> ltb s s0 = (s <= s0)%ord.
+Proof.
+  intros s s0.
+  unfold ltb , nat_comparable , Nat.ltb.
+  intros e.
+  
+  generalize dependent s.
+  induction s0 ; intros.
+  * destruct s ; easy.
+  * destruct s. reflexivity.
+    (* unfold Nat.leb ; fold Nat.leb. *)
+    cbn.
+    cbn in IHs0.
+    rewrite IHs0.
+    reflexivity.
+    assumption.
+Qed.
+
+(* Theorem loc_compute_b : *)
+(*   (forall l : (@sigT choice_type (fun _ : choice_type => nat)), *)
+(*     forall n : list (@sigT choice_type (fun _ : choice_type => nat)), *)
+(*       Inb l n = ssrbool.in_mem l (@ssrbool.mem _ *)
+(*                                                (seq.seq_predType *)
+(*                                                   (Ord.eqType *)
+(*                                                      (@tag_ordType choice_type_ordType (fun _ : choice_type => nat_ordType)))) *)
+(*                                                n)). *)
+(*   intros. *)
+(*   cbn. *)
+(*   unfold ssrbool.in_mem. *)
+(*   unfold ssrbool.pred_of_mem. *)
+(*   unfold ssrbool.mem ; cbn. *)
+  
+(*   induction n. *)
+(*   - cbn. *)
+(*     reflexivity. *)
+(*   - cbn. *)
+
+(*     rewrite location_eqbP. *)
+    
+(*     unfold "||". *)
+(*     rewrite eqtype.tag_eqE ; rewrite eqtype.eq_sym ; rewrite <- eqtype.tag_eqE. *)
+(*     rewrite IHn. *)
+(*     reflexivity. *)
+(* Qed. *)
+
+Theorem loc_compute : (forall l : (@sigT choice_type (fun _ : choice_type => nat)), forall n : list (@sigT choice_type (fun _ : choice_type => nat)), List.In l n <-> is_true (ssrbool.in_mem l (@ssrbool.mem _ (seq.seq_predType (Ord.eqType (@tag_ordType choice_type_ordType (fun _ : choice_type => nat_ordType)))) n))).
+Proof.
+  intros.
+  cbn.
+  unfold ssrbool.in_mem.
+  unfold ssrbool.pred_of_mem.
+  unfold ssrbool.mem ; cbn.
+  
+  induction n.
+  - cbn. split ; easy.
+  - cbn.
+
+    rewrite is_true_split_or.
+    (* rewrite eqtype.tag_eqE. *)
+    
+    (* rewrite (ssrbool.introT eqtype.eqP). *)
+    
+    (* rewrite location_eqbP. *)
+    
+    (* unfold "||". *)
+    rewrite eqtype.tag_eqE ; rewrite eqtype.eq_sym ; rewrite <- eqtype.tag_eqE.
+    rewrite IHn.
+
+    apply or_iff_compat_r.
+    apply (ssrbool.rwP (@eqtype.eqP loc_eqType a l)).
+Qed.
+
+(* Theorem in_bool_eq : forall {A : Type} `{EqDec A} (a:A) (l:list A), is_true (Inb a l) = List.In a l. *)
+(*   intros. *)
+(*   rewrite boolp.propeqE. apply in_bool_iff. *)
+(* Qed. *)
+
+(* Fixpoint incl_sort_compute A `{EqDec A} (l1 l2 : list A) : bool := *)
+(*   match l1 with *)
+(*   | nil => true *)
+(*   | (x :: xs) => (andb (Inb x l2) (incl_sort_compute A xs l2)) *)
+(*   end. *)
+
+Fixpoint incl_expand A `{EqDec A} (l1 l2 : list A) : Prop :=
+  match l1 with
+  | nil => True
+  | (x :: xs) => In x l2 /\ incl_expand A xs l2
+  end.
+
+(* Proof. *)
+(*   induction l1. *)
+(*   - exact true. *)
+(*   - exact (andb (Inb a l2) (IHl1)).       *)
+(* Defined. *)
+ 
+(* Definition incl_fset_sort_compute (l1 l2 : {fset Location}) : bool. *)
+(* Proof. *)
+(*   destruct l1 as [l1]. *)
+(*   induction l1. *)
+(*   - exact true. *)
+(*   - assert (is_true (path.sorted Ord.lt l1)). *)
+(*     { *)
+(*       pose (path.drop_sorted). *)
+(*       specialize i0 with (n := 1) (s := a :: l1). *)
+(*       rewrite seq.drop1 in i0. *)
+(*       unfold seq.behead in i0. *)
+(*       apply i0. *)
+(*       apply i. *)
+(*     } *)
+(*     exact (andb (Inb a l2) (IHl1 H)).       *)
+(* Defined. *)
+
+Theorem in_remove_fset : forall a (l : list Location), List.In a l <-> List.In a (fset l).
+Proof.
+  intros.
+  do 2 rewrite loc_compute.
+  unfold fset ; rewrite ssreflect.locked_withE.
+  cbn.
+  rewrite (@path.mem_sort (Ord.eqType
+                             (@tag_ordType choice_type_ordType (fun _ : choice_type => nat_ordType))) (tag_leq (I:=choice_type_ordType) (T_:=fun _ : choice_type => nat_ordType)) (@seq.undup
+                                                                                                                                                                                     (Ord.eqType
+                                                                                                                                                                                        (@tag_ordType choice_type_ordType (fun _ : choice_type => nat_ordType)))
+                                                                                                                                                                                     l)).
+  
+  generalize dependent a.
+  induction l ; intros.
+  + easy.
+  + cbn.
+
+    rewrite (@seq.in_cons (Ord.eqType
+                             (@tag_ordType choice_type_ordType (fun _ : choice_type => nat_ordType))) a l).
+    rewrite is_true_split_or.
+
+    match goal with
+    | [ |- context[match ?x with | true => _ | false => _ end] ] =>
+        destruct x eqn:so
+    end.
+    * rewrite <- IHl.
+      split.
+      -- intros [].
+         ++ apply Couplings.reflection_nonsense in H.
+            subst.
+            apply so.
+         ++ apply H.
+      -- intros.
+         right.
+         apply H.
+    * split.
+      -- intros [].
+         ++ apply Couplings.reflection_nonsense in H.
+            subst.
+            apply seq.mem_head.
+         ++ apply seq.mem_drop with (n0 := 1%nat).
+            cbn.
+            rewrite seq.drop0.
+            apply IHl.
+            apply H.
+      -- intros.
+         destruct (eqtype.eq_op) eqn:so2.
+         ++ left.
+            reflexivity.
+         ++ right.
+            unfold ssrbool.in_mem in H.
+            unfold ssrbool.pred_of_mem in H.
+            unfold ssrbool.mem in H.
+            cbn in H.
+            cbn in so2.
+            rewrite so2 in H.
+            cbn in H.
+
+            apply IHl.
+            apply H.
+Qed.
+
+Theorem in_split_cat : forall a (l0 l1 : list Location), List.In a (seq.cat l0 l1) <-> List.In a l0 \/ List.In a l1.
+Proof.
+  split ; intros.
+  - induction l0.
+    + right. apply H.
+    + destruct H.
+      * left. left. assumption.
+      * destruct (IHl0 H).
+        -- left. right. assumption.
+        -- right. assumption.
+  - destruct H.
+    + induction l0.
+      * contradiction.
+      * destruct H.
+        -- left. assumption.
+        -- right.
+           apply IHl0.
+           assumption.
+    + induction l0.
+      * assumption.
+      * right.
+        assumption.
+Qed.
+
+Theorem in_split_fset_cat : forall a (l0 l1 : {fset tag_ordType (I:=choice_type_ordType) (fun _ : choice_type => nat_ordType)}), List.In a (l0 :|: l1) <-> List.In a l0 \/ List.In a l1.
+Proof.
+  intros.
+  transitivity (In a (seq.cat (eqtype.val l0) (eqtype.val l1))).
+  symmetry.
+  apply in_remove_fset.
+  apply in_split_cat.
+Qed.
+
+Theorem list_incl_fsubset : forall (l0 l1 : {fset tag_ordType (I:=choice_type_ordType) (fun _ : choice_type => nat_ordType)}), is_true (fsubset l0 l1) <-> List.incl l0 l1.
+Proof.
+  intros.
+  rewrite <- (ssrbool.rwP (@fsubsetP _ l0 l1)).
+  
+  unfold ssrbool.sub_mem.
+  unfold incl.
+
+  assert (forall {A} (P Q : A -> Prop), (forall x, P x <-> Q x) -> (forall x, P x) <-> (forall x, Q x)).
+  { split ; intros ; apply H ; apply H0. }
+  apply H. clear H.
+  intros x. cbn in *.
+
+  rewrite loc_compute.
+  rewrite loc_compute.
+
+  reflexivity.
+Qed.
+
+
+Lemma valid_injectLocations_b :
+  forall (import : Interface) (A : choice.Choice.type)
+         (L1 L2 : {fset tag_ordType (I:=choice_type_ordType) (fun _ : choice_type => nat_ordType)})
+         (v : raw_code A),
+    List.incl L1 L2 -> ValidCode L1 import v -> ValidCode L2 import v.
+Proof.  
+  intros I A L1 L2 v incl.
+  apply valid_injectLocations.
+  apply list_incl_fsubset.
+  apply incl.
+Qed.
+
+Theorem list_incl_remove_fset {A} `{EqDec A} : forall (l1 l2 : list Location), List.incl l1 l2 <-> List.incl (fset l1) (fset l2).
+Proof.
+  intros.
+
+  cbn in *.
+  
+  induction l1.
+  - rewrite <- fset0E. easy.
+  - cbn.
+    unfold incl.
+    cbn.
+    split.
+    + intros.
+      rewrite <- in_remove_fset.
+      rewrite <- in_remove_fset in H1.
+      apply H0.
+      apply H1.
+    + intros.        
+      rewrite -> in_remove_fset.
+      apply H0.
+      rewrite <- in_remove_fset.
+      apply H1.
+Qed.        
+
+Theorem list_incl_cons_iff : (forall A (a : A) l1 l2, List.incl (a :: l1) l2 <-> (List.In a l2 /\ List.incl l1 l2)).
+Proof.
+  split.
+  - pose List.incl_cons_inv.
+    apply List.incl_cons_inv.
+  - intros [].
+    apply List.incl_cons ; assumption.          
+Qed.
+
+(* Theorem list_incl_compute {A} `{EqDec A} : forall (l1 l2 : list Location), *)
+(*     List.incl l1 l2 <-> is_true (incl_sort_compute _ l1 l2). *)
+(* Proof. *)
+(*   induction l1. *)
+(*   - split ; intros. *)
+(*     reflexivity. *)
+(*     apply incl_nil_l. *)
+(*   - intros. *)
+    
+(*     rewrite list_incl_cons_iff. *)
+
+(*     cbn. *)
+(*     rewrite is_true_split_and. *)
+(*     rewrite in_bool_eq. *)
+
+(*     apply and_iff_compat_l. *)
+(*     apply IHl1. *)
+(* Qed.         *)
+
+Theorem list_incl_expand {A} `{EqDec A} : forall (l1 l2 : list Location),
+    List.incl l1 l2 <-> incl_expand _ l1 l2.
+Proof.
+  induction l1.
+  - split ; intros.
+    reflexivity.
+    apply incl_nil_l.
+  - intros.
+    rewrite list_incl_cons_iff.
+    cbn.
+    apply and_iff_compat_l.
+    apply IHl1.
+Qed.
+
+(* Theorem forall l1 l2, incl_sort_compute <-> list_incl_compute  *)
+
+Definition location_lebP : (tag_leq (I:=choice_type_ordType) (T_:=fun _ : choice_type => nat_ordType)) = leb.
+Proof.
+  intros.
+  do 2 (apply (@functional_extensionality Location) ; intros []).
+  cbn.
+  
+  unfold tag_leq.
+  unfold eqtype.tag_eq.
+
+  unfold location_ltb.
+  unfold tag_leq.
+  
+  (* set (_ && _)%bool. *)
+  (* set (_ && _)%bool. *)
+
+  unfold location_eqb.
+  
+  unfold ssrfun.tag , ssrfun.tagged , projT1 , projT2 in *.
+
+  rewrite (Bool.andb_comm _ (eqtype.eq_op _ _)).
+  
+  destruct (eqtype.eq_op x _) eqn:x_eq_x0.
+  2: reflexivity.
+  apply Couplings.reflection_nonsense in x_eq_x0.
+  subst.
+  rewrite eqtype.eq_refl.
+  rewrite Bool.andb_true_l.
+  rewrite Bool.andb_true_l.
+  rewrite Ord.ltxx.
+  rewrite Bool.orb_false_l.
+
+  destruct (eqtype.eq_op _ _) eqn:n_eq_n0.
+  2: reflexivity.
+
+  unfold eqtype.tagged_as in *.
+  unfold ssrfun.tagged ,  projT2 in *.
+  unfold eq_rect_r , eq_rect in *.
+  
+  destruct eqtype.eqP in *.
+  2: contradiction.
+  cbn in n_eq_n0.
+  destruct eq_sym in *.
+  rewrite ssrnat.eqnE in n_eq_n0.
+  apply Couplings.reflection_nonsense in n_eq_n0.
+  apply Ord.eq_leq. assumption.
+Qed.
+
+Lemma iff_extensionality : forall {A} (P Q : A -> Prop), (forall a, P a <-> Q a) -> ((forall a, P a) <-> (forall a, Q a)).
+Proof.
+  intros. split ; intuition.
+Qed.
+
+Lemma iff_eq_sym : forall {A} (x y : A), (x = y) <-> (y = x).
+Proof.
+  intros. split ; intuition.
+Qed.
+
+Definition loc_seq_has (a : Location) := seq.has (ssrbool.fun_of_rel (@eqtype.eq_op loc_eqType) a).
+
+Theorem loc_seq_has_remove_sort {A} `{EqDec A} : forall (l : list Location) (a : Location) leb,
+    is_true (loc_seq_has a l) <->
+    is_true (loc_seq_has a (path.sort leb l)).
+Proof.
+  intros.
+  rewrite <- (Bool.negb_involutive (loc_seq_has a (path.sort leb l))).
+
+  unfold loc_seq_has.
+  
+  rewrite <- seq.all_predC.
+  rewrite path.all_sort.
+  rewrite seq.all_predC.
+
+  rewrite Bool.negb_involutive.
+
+  reflexivity.
+Qed.  
+
+Theorem list_in_iff_seq_has {A} `{EqDec A} : forall (l : list Location) (a : Location),
+    is_true (loc_seq_has a l) <-> List.In a l.
+Proof.
+  induction l ; intros.
+  - split ; intros ; easy. 
+  - cbn.
+    rewrite is_true_split_or.
+    apply ZifyClasses.or_morph.
+    + rewrite <- (ssrbool.rwP (@eqtype.eqP loc_eqType a0 a)).      
+      apply iff_eq_sym.
+    + apply IHl.
+Qed.    
+
+Theorem list_in_iff_list_in_sort {A} `{EqDec A} : forall (l : list Location) (a : Location) leb,
+    List.In a l <-> List.In a (path.sort leb l).
+Proof.
+  intros.
+  rewrite <- (list_in_iff_seq_has (path.sort leb l)).
+  rewrite <- loc_seq_has_remove_sort.
+  rewrite list_in_iff_seq_has.
+  reflexivity.
+Qed.    
+
+Theorem list_in_sort_order_ignorant_compute {A} `{EqDec A} : forall (l : list Location) leb1 leb2 a,
+    (List.In a (path.sort leb1 l)) <-> List.In a (path.sort leb2 l).
+Proof.
+  intros.
+  rewrite <- list_in_iff_list_in_sort.
+  rewrite <- list_in_iff_list_in_sort.
+  reflexivity.
+Qed.
+  
+Theorem list_incl_sort_order_ignorant_compute {A} `{EqDec A} : forall (l1 l2 : list Location) leb1 leb2,
+    List.incl (path.sort leb1 l1) (path.sort leb1 l2) <-> List.incl (path.sort leb2 l1) (path.sort leb2 l2).
+Proof.
+  intros.
+  apply iff_extensionality.
+  intros a.
+
+  rewrite list_in_sort_order_ignorant_compute with (leb1 := leb1) (leb2 := leb2).
+  rewrite list_in_sort_order_ignorant_compute with (leb1 := leb1) (leb2 := leb2).
+  reflexivity.
+Qed.    
+
+Theorem list_incl_sort {A} `{EqDec A} : forall (l1 l2 : list Location) leb,
+    List.incl l1 l2 <-> List.incl (path.sort leb l1) (path.sort leb l2).
+Proof.
+  intros.
+  apply iff_extensionality.
+  intros a.
+  rewrite <- list_in_iff_list_in_sort.
+  rewrite <- list_in_iff_list_in_sort.
+  reflexivity.
+Qed.  
+
+Theorem choice_type_test_refl : forall x , is_true (choice_type_test x x).
+Proof.
+  intros.
+  replace (choice_type_test _ _) with (eqtype.eq_op x x) by reflexivity.
+  apply eqtype.eq_refl.
+Qed.
